@base          <http://sweetontology.net/humanEnvirControl> .
@prefix com:   <http://sweetontology.net/humanCommerce/> .
@prefix con:   <http://sweetontology.net/humanEnvirControl/> .
@prefix dec:   <http://sweetontology.net/humanDecision/> .
@prefix rdf:   <http://www.w3.org/1999/02/22-rdf-syntax-ns#> .
@prefix owl:   <http://www.w3.org/2002/07/owl#> .
@prefix xsd:   <http://www.w3.org/2001/XMLSchema#> .
@prefix land:  <http://sweetontology.net/realmLandform/> .
@prefix rdfs:  <http://www.w3.org/2000/01/rdf-schema#> .

con:EnvironmentalControlStrategy
        a                owl:Class ;
        rdfs:subClassOf  dec:ControlStrategy .

con:CarbonOffset  a      owl:Class ;
        rdfs:subClassOf  con:EnvironmentalControlStrategy .

con:WellInjection  a     owl:Class ;
        rdfs:comment     "The subsurface emplacement of \"fluids\" through a bored, drilled, or driven \"well\", or through a dug well, where the depth of the dug well is greater than the largest surface dimension."@en ;
        rdfs:subClassOf  con:EnvironmentalControlStrategy .

con:CloudSeeding  a      owl:Class ;
        rdfs:subClassOf  con:EnvironmentalControlStrategy .

con:Reforestation  a     owl:Class ;
        rdfs:subClassOf  con:Revegetation .

con:SecondaryTreatment
        a                owl:Class ;
        rdfs:comment     "In wastewater treatment, a combination of step processes, usually biochemical in nature, that are designed to remove primarily organic material. Examples of process steps are aeration and trickling filters."@en ;
        rdfs:subClassOf  con:WaterTreatmentProcess .

con:DryScrubbing  a      owl:Class ;
        rdfs:subClassOf  con:Scrubbing .

con:BestAvailablControlTechnology
        a                    owl:Class ;
        rdfs:subClassOf      con:EnvironmentalControlStrategy ;
        owl:equivalentClass  con:BACT .

con:Reclamation  a       owl:Class ;
        rdfs:subClassOf  con:EnvironmentalControlStrategy .

con:Afforestation  a     owl:Class ;
        rdfs:subClassOf  con:EnvironmentalControlStrategy .

con:Pretreatment  a      owl:Class ;
        rdfs:subClassOf  con:EnvironmentalControlStrategy .

con:TertiaryTreatment
        a                owl:Class ;
        rdfs:comment     "Post-secondary treatment of wastewater designed to improve the quality of the water to the point where it can be put to a particular beneficial use. Generally, tertiary treatment steps remove nutrients (e.g., nitrogen and phosphorus) which are poorly removed by secondary treatment. Commonly used steps include coagulation and clarification."@en ;
        rdfs:subClassOf  con:WaterTreatmentProcess .

con:Sequester  a         owl:Class ;
        rdfs:subClassOf  con:EnvironmentalControlStrategy .

con:Restoration  a       owl:Class ;
        rdfs:subClassOf  con:EnvironmentalControlStrategy .

con:Scrubbing  a         owl:Class ;
        rdfs:subClassOf  con:AirTreatmentProcess .

con:PrimaryTreatment  a  owl:Class ;
        rdfs:comment     "In wastewater treatment, a combination of step processes, usually physical in nature, that are designed to remove floating and settleable solids. Examples of process steps are screening and sedimentation."@en ;
        rdfs:subClassOf  con:WaterTreatmentProcess .

<>      a                owl:Ontology ;
        rdfs:label       "SWEET Ontology" ;
        owl:imports      <humanDecision> , <humanCommerce> , <realmLandform> ;
        owl:versionInfo  "3.1.0" .

con:Distillation  a      owl:Class ;
        rdfs:subClassOf  con:WaterTreatmentProcess .

con:CarbonSequestration
        a                owl:Class ;
        rdfs:subClassOf  con:Sequester .

con:Treatment  a         owl:Class ;
        rdfs:subClassOf  con:EnvironmentalControlStrategy .

con:Biosequestration  a  owl:Class ;
        rdfs:subClassOf  con:CarbonSequestration .

con:CapAndTrade  a       owl:Class ;
        rdfs:subClassOf  con:EnvironmentalControlStrategy .

con:MaximumAchievableControlTechnology
        a                    owl:Class ;
        rdfs:subClassOf      con:EnvironmentalControlStrategy ;
        owl:equivalentClass  con:MACT .

con:Abatement  a         owl:Class ;
        rdfs:subClassOf  con:EnvironmentalControlStrategy .

con:BACT  a     owl:Class .

con:WetScrubbing  a      owl:Class ;
        rdfs:subClassOf  con:Scrubbing .

con:Remediation  a       owl:Class ;
        rdfs:subClassOf  con:EnvironmentalControlStrategy .

con:ControlledBurn  a    owl:Class ;
        rdfs:subClassOf  con:EnvironmentalControlStrategy .

con:Revegetation  a      owl:Class ;
        rdfs:subClassOf  con:EnvironmentalControlStrategy .

con:WaterManagement  a   owl:Class ;
        rdfs:subClassOf  com:Management .

con:Flocculation  a      owl:Class ;
        rdfs:subClassOf  con:WaterTreatmentProcess .

con:MACT  a     owl:Class .

con:WaterTreatmentProcess
        a                owl:Class ;
        rdfs:subClassOf  con:EnvironmentalControlStrategy , con:Treatment .

con:StateImplementationPlan
        a                owl:Class ;
        rdfs:subClassOf  con:EnvironmentalControlStrategy .

con:AirTreatmentProcess
        a                owl:Class ;
        rdfs:subClassOf  con:EnvironmentalControlStrategy , con:Treatment .

con:Compliance  a        owl:Class ;
        rdfs:subClassOf  con:EnvironmentalControlStrategy .

con:WastewaterTreatment
        a                owl:Class ;
        rdfs:subClassOf  con:Treatment .
