@base          <http://sweetontology.net/matr> .
@prefix role:  <http://sweetontology.net/stateRole/> .
@prefix chem:  <http://sweetontology.net/matr/> .
@prefix rdf:   <http://www.w3.org/1999/02/22-rdf-syntax-ns#> .
@prefix owl:   <http://www.w3.org/2002/07/owl#> .
@prefix pstate: <http://sweetontology.net/statePhysical/> .
@prefix xsd:   <http://www.w3.org/2001/XMLSchema#> .
@prefix rdfs:  <http://www.w3.org/2000/01/rdf-schema#> .
@prefix state: <http://sweetontology.net/state/> .
@prefix rela:  <http://sweetontology.net/rela/> .

chem:TraceSubstance  a   owl:Class ;
        rdfs:subClassOf  chem:Substance ;
        rdfs:subClassOf  [ a               owl:Restriction ;
                           owl:hasValue    role:Trace ;
                           owl:onProperty  rela:hasRole
                         ] .

chem:NeutralGas  a       owl:Class ;
        rdfs:subClassOf  chem:ChemicalSubstance ;
        rdfs:subClassOf  [ a               owl:Restriction ;
                           owl:hasValue    pstate:Gas ;
                           owl:onProperty  rela:hasState
                         ] ;
        rdfs:subClassOf  [ a               owl:Restriction ;
                           owl:hasValue    pstate:Neutral ;
                           owl:onProperty  rela:hasState
                         ] .

chem:DissolvedSolid  a   owl:Class ;
        rdfs:subClassOf  chem:SolidSubstance , chem:DissolvedSubstance .

chem:TraceGas  a         owl:Class ;
        rdfs:subClassOf  chem:TraceSubstance ;
        rdfs:subClassOf  [ a               owl:Restriction ;
                           owl:hasValue    pstate:Gas ;
                           owl:onProperty  rela:hasState
                         ] .

chem:ChemicalSubstance
        a       owl:Class .

chem:DissolvedSubstance
        a                owl:Class ;
        rdfs:subClassOf  chem:Substance ;
        rdfs:subClassOf  [ a               owl:Restriction ;
                           owl:hasValue    pstate:Dissolved ;
                           owl:onProperty  rela:hasState
                         ] .

chem:GreenhouseGas  a    owl:Class ;
        rdfs:subClassOf  chem:ChemicalSubstance ;
        rdfs:subClassOf  [ a               owl:Restriction ;
                           owl:hasValue    pstate:Gas ;
                           owl:onProperty  rela:hasState
                         ] .

chem:SolidSubstance  a   owl:Class ;
        rdfs:subClassOf  chem:Substance ;
        rdfs:subClassOf  [ a               owl:Restriction ;
                           owl:hasValue    pstate:Solid ;
                           owl:onProperty  rela:hasState
                         ] .

chem:InorganicSubstance
        a       owl:Class .

chem:DO  a      owl:Class .

<>      a                owl:Ontology ;
        rdfs:label       "SWEET Ontology" ;
        owl:imports      <state> , <statePhysical> , <rela> , <stateRole> ;
        owl:versionInfo  "3.1.0" .

chem:SuspendedGas  a     owl:Class ;
        rdfs:subClassOf  chem:SuspendedSubstance ;
        rdfs:subClassOf  [ a               owl:Restriction ;
                           owl:hasValue    pstate:Gas ;
                           owl:onProperty  rela:hasState
                         ] .

chem:DOC  a     owl:Class .

chem:Solution  a         owl:Class ;
        rdfs:comment     "In chemistry, a solution is a homogeneous mixture composed of two or more substances. In such a mixture, a solute is dissolved in another substance, known as a solvent. All solutions are characterized by interactions between the solvent phase and solute molecules or ions that result in a net decrease in free energy. [Wikipedia]"@en ;
        rdfs:subClassOf  chem:Mixture .

chem:BDOC  a    owl:Class .

chem:SuspendedSolid  a   owl:Class ;
        rdfs:subClassOf  chem:SuspendedSubstance , chem:SolidSubstance .

chem:Substance  a  owl:Class .

chem:Air  a              owl:Class ;
        rdfs:subClassOf  chem:Mixture .

chem:Mixture  a              owl:Class ;
        rdfs:comment         "In chemistry, a mixture is when two or more different substances are mixed together but not combined chemically. The molecules of two or more different substances are mixed in the form of solutions, suspensions, and colloids. [Wikipedia]"@en ;
        rdfs:subClassOf      chem:ChemicalSubstance ;
        owl:equivalentClass  chem:MixedChemicalSubstance .

chem:Chemical  a             owl:Class ;
        rdfs:comment         "Chemical substance, in chemistry, are material objects that can undergo various transformations related to artificial or natural phenomena [Wikipedia]"@en ;
        rdfs:subClassOf      chem:Substance ;
        owl:equivalentClass  chem:ChemicalSubstance .

chem:BiodegradableDissolvedOrganicCarbon
        a                    owl:Class ;
        rdfs:subClassOf      chem:DissolvedOrganicCarbon ;
        owl:equivalentClass  chem:BDOC .

chem:Inorganic  a            owl:Class ;
        rdfs:subClassOf      chem:ChemicalSubstance ;
        owl:equivalentClass  chem:InorganicSubstance .

chem:DissolvedOrganicCarbon
        a                    owl:Class ;
        rdfs:subClassOf      chem:DissolvedSubstance ;
        owl:equivalentClass  chem:DOC .

chem:SuspendedSubstance
        a                owl:Class ;
        rdfs:subClassOf  chem:Substance ;
        rdfs:subClassOf  [ a               owl:Restriction ;
                           owl:hasValue    pstate:Suspended ;
                           owl:onProperty  rela:hasState
                         ] .

chem:Medium  a           owl:Class ;
        rdfs:subClassOf  chem:Substance .

chem:OrganicLoading  a   owl:Class ;
        rdfs:subClassOf  chem:DissolvedSubstance .

chem:MixedChemicalSubstance
        a       owl:Class .

chem:DissolvedOxygen  a      owl:Class ;
        rdfs:subClassOf      chem:DissolvedSubstance ;
        owl:equivalentClass  chem:DO .

chem:DissolvedGas  a     owl:Class ;
        rdfs:subClassOf  chem:DissolvedSubstance ;
        rdfs:subClassOf  [ a               owl:Restriction ;
                           owl:hasValue    pstate:Gas ;
                           owl:onProperty  rela:hasState
                         ] .
