@base          <http://sweetontology.net/matrEquipment> .
@prefix infr:  <http://sweetontology.net/matrEquipment/> .
@prefix hum:   <http://sweetontology.net/human/> .
@prefix rdf:   <http://www.w3.org/1999/02/22-rdf-syntax-ns#> .
@prefix subs:  <http://sweetontology.net/matr/> .
@prefix owl:   <http://www.w3.org/2002/07/owl#> .
@prefix xsd:   <http://www.w3.org/2001/XMLSchema#> .
@prefix realm: <http://sweetontology.net/realm/> .
@prefix rdfs:  <http://www.w3.org/2000/01/rdf-schema#> .
@prefix body:  <http://sweetontology.net/realmAstroBody/> .
@prefix tran:  <http://sweetontology.net/humanTransportation/> .
@prefix rela:  <http://sweetontology.net/rela/> .
@prefix hrela: <http://sweetontology.net/relaHuman/> .

infr:MaterialThing  a    owl:Class ;
        rdfs:subClassOf  subs:Substance .

infr:InjectionWell  a    owl:Class ;
        rdfs:subClassOf  infr:Well .

<>      a                owl:Ontology ;
        rdfs:label       "SWEET Ontology" ;
        owl:imports      <realm> , <relaHuman> , <rela> , <realmAstroBody> , <matr> , <humanTransportation> ;
        owl:versionInfo  "3.1.0" .

infr:Wireless  a         owl:Class ;
        rdfs:subClassOf  infr:CommunicationMethod .

infr:NavigationEquipment
        a                owl:Class ;
        rdfs:subClassOf  infr:Equipment ;
        rdfs:subClassOf  [ a                  owl:Restriction ;
                           owl:allValuesFrom  infr:Navigation ;
                           owl:onProperty     hrela:hasHumanActivity
                         ] .

infr:CommunicationsEquipment
        a                owl:Class ;
        rdfs:subClassOf  infr:Equipment ;
        rdfs:subClassOf  [ a                  owl:Restriction ;
                           owl:allValuesFrom  infr:Communications ;
                           owl:onProperty     hrela:hasHumanActivity
                         ] .

infr:DrainageWell  a     owl:Class ;
        rdfs:subClassOf  infr:Well .

infr:UnconfinedWell  a   owl:Class ;
        rdfs:subClassOf  infr:Well .

infr:Rocket  a           owl:Class ;
        rdfs:subClassOf  infr:Spacecraft .

infr:Satellite  a        owl:Class ;
        rdfs:subClassOf  infr:Spacecraft .

infr:SpaceShuttle  a     owl:Class ;
        rdfs:subClassOf  infr:Spacecraft .

infr:Transmission  a  owl:Class .

infr:Train  a            owl:Class ;
        rdfs:subClassOf  infr:Vehicle .

infr:Receiver  a         owl:Class ;
        rdfs:subClassOf  infr:CommunicationsEquipment ;
        rdfs:subClassOf  [ a                  owl:Restriction ;
                           owl:allValuesFrom  infr:Reception ;
                           owl:onProperty     rela:hasRole
                         ] .

infr:Reception  a  owl:Class .

infr:CommunicationMethod
        a                owl:Class ;
        rdfs:subClassOf  infr:Communication .

infr:Helicopter  a       owl:Class ;
        rdfs:subClassOf  infr:Aircraft .

infr:Ship  a             owl:Class ;
        rdfs:subClassOf  infr:Vehicle .

infr:Well  a             owl:Class ;
        rdfs:comment     "A bored, drilled or driven shaft, or a dug hole, whose depth is greater than the largest surface dimension."@en ;
        rdfs:subClassOf  infr:Equipment .

infr:DisposalWell  a     owl:Class ;
        rdfs:subClassOf  infr:Well .

infr:Radio  a            owl:Class ;
        rdfs:subClassOf  infr:CommunicationMethod , infr:CommunicationsEquipment .

infr:Car  a              owl:Class ;
        rdfs:subClassOf  infr:Vehicle .

infr:EmergencyVehicle
        a                owl:Class ;
        rdfs:subClassOf  infr:Vehicle .

infr:Trailer  a          owl:Class ;
        rdfs:subClassOf  infr:Vehicle .

infr:Airplane  a         owl:Class ;
        rdfs:subClassOf  infr:Aircraft .

infr:PumpingWell  a      owl:Class ;
        rdfs:subClassOf  infr:Well .

infr:MonitoringWell  a   owl:Class ;
        rdfs:subClassOf  infr:Well .

infr:Transmit  a             owl:Class ;
        rdfs:subClassOf      infr:Communication ;
        owl:equivalentClass  infr:Transmission .

infr:ArtesianWell  a     owl:Class ;
        rdfs:subClassOf  infr:ConfinedWell .

infr:Spacecraft  a       owl:Class ;
        rdfs:subClassOf  infr:TransportationEquipment ;
        rdfs:subClassOf  [ a                  owl:Restriction ;
                           owl:allValuesFrom  body:OuterSpace ;
                           owl:onProperty     rela:hasRealm
                         ] .

infr:Antenna  a          owl:Class ;
        rdfs:subClassOf  infr:CommunicationsEquipment .

infr:Navigation  a       owl:Class ;
        rdfs:subClassOf  hum:HumanActivity .

infr:Pipeline  a         owl:Class ;
        rdfs:subClassOf  infr:TransportationEquipment .

infr:Vehicle  a          owl:Class ;
        rdfs:subClassOf  infr:TransportationEquipment .

infr:Communications  a  owl:Class .

infr:Borehole  a         owl:Class ;
        rdfs:comment     "A borehole is the generalised term for any narrow shaft drilled in the ground, either vertically or horizontally. A borehole may be constructed for many different purposes including the extraction of water or fluid (such as oil) or gases (such as natural gas or methane), as part of a geotechnical investigation or environmental site assessment, for mineral exploration, or as a pilot hole for installing piers or underground utilities." ;
        rdfs:subClassOf  infr:Equipment .

infr:Rover  a            owl:Class ;
        rdfs:subClassOf  infr:Vehicle .

infr:Truck  a            owl:Class ;
        rdfs:subClassOf  infr:Vehicle .

infr:Aircraft  a         owl:Class ;
        rdfs:comment     "An aircraft is a vehicle which is able to fly through the air (or through any other atmosphere). All the human activity which surrounds aircraft is called aviation. (Most rocket vehicles are not aircraft because they are not supported by the surrounding air)." ;
        rdfs:subClassOf  infr:Equipment ;
        rdfs:subClassOf  [ a                  owl:Restriction ;
                           owl:allValuesFrom  realm:Atmosphere ;
                           owl:onProperty     rela:hasRealm
                         ] .

infr:ConfinedWell  a     owl:Class ;
        rdfs:subClassOf  infr:Well .

infr:Internet  a         owl:Class ;
        rdfs:subClassOf  infr:CommunicationMethod .

infr:Communication  a        owl:Class ;
        rdfs:subClassOf      hum:HumanActivity ;
        owl:equivalentClass  infr:Communications .

infr:Phone  a            owl:Class ;
        rdfs:subClassOf  infr:CommunicationMethod , infr:CommunicationsEquipment .

infr:Signal  a           owl:Class ;
        rdfs:subClassOf  infr:Communication .

infr:Infrastructure  a   owl:Class ;
        rdfs:subClassOf  infr:MaterialThing .

infr:LandLine  a         owl:Class ;
        rdfs:subClassOf  infr:Phone .

infr:Receive  a              owl:Class ;
        rdfs:subClassOf      infr:Communication ;
        owl:equivalentClass  infr:Reception .

infr:RechargeWell  a     owl:Class ;
        rdfs:subClassOf  infr:Well .

infr:Sink  a             owl:Class ;
        rdfs:subClassOf  infr:Equipment .

infr:TransportationEquipment
        a                owl:Class ;
        rdfs:subClassOf  infr:Equipment ;
        rdfs:subClassOf  [ a                  owl:Restriction ;
                           owl:allValuesFrom  tran:Transportation ;
                           owl:onProperty     hrela:hasHumanActivity
                         ] .

infr:Equipment  a        owl:Class ;
        rdfs:subClassOf  infr:Infrastructure .

infr:MobilePhone  a      owl:Class ;
        rdfs:subClassOf  infr:Phone .

infr:Jet  a              owl:Class ;
        rdfs:subClassOf  infr:Aircraft .

infr:ComputerHardware
        a                owl:Class ;
        rdfs:subClassOf  infr:Equipment .

infr:Transmitter  a      owl:Class ;
        rdfs:subClassOf  infr:CommunicationsEquipment ;
        rdfs:subClassOf  [ a                  owl:Restriction ;
                           owl:allValuesFrom  infr:Transmission ;
                           owl:onProperty     rela:hasRole
                         ] .
