@base          <http://sweetontology.net/matrIon> .
@prefix elem:  <http://sweetontology.net/matrElement/> .
@prefix comp:  <http://sweetontology.net/matrCompound/> .
@prefix allo:  <http://sweetontology.net/matrElementalMolecule/> .
@prefix crela: <http://sweetontology.net/relaChemical/> .
@prefix chem:  <http://sweetontology.net/matr/> .
@prefix owl:   <http://www.w3.org/2002/07/owl#> .
@prefix prela: <http://sweetontology.net/relaPhysical/> .
@prefix pstate: <http://sweetontology.net/statePhysical/> .
@prefix xsd:   <http://www.w3.org/2001/XMLSchema#> .
@prefix ion:   <http://sweetontology.net/matrIon/> .
@prefix rdfs:  <http://www.w3.org/2000/01/rdf-schema#> .
@prefix rdf:   <http://www.w3.org/1999/02/22-rdf-syntax-ns#> .
@prefix state: <http://sweetontology.net/state/> .
@prefix rela:  <http://sweetontology.net/rela/> .

ion:Nitrite  a  ion:Ion .

ion:NH4plus  a               comp:InorganicCompound , ion:Ion ;
        crela:hasChemical_1  elem:N ;
        crela:hasChemical_2  ion:H4plus ;
        owl:sameAs           ion:Ammonium .

ion:Ammonium  a  ion:Ion .

ion:O3minus  a             ion:Ion ;
        crela:hasChemical  allo:O3 ;
        prela:hasCharge    -1 .

ion:Nitrate  a  ion:Ion .

<>      a                owl:Ontology ;
        rdfs:label       "SWEET Ontology" ;
        owl:imports      <state> , <matrCompound> , <rela> , <relaPhysical> , <matrElementalMolecule> , <matrElement> , <statePhysical> , <relaChemical> , <matr> ;
        owl:versionInfo  "3.1.0" .

ion:O3minusminus  a        ion:Ion ;
        crela:hasChemical  allo:O3 ;
        prela:hasCharge    -2 .

ion:SaltIon  a           owl:Class ;
        rdfs:subClassOf  ion:Ion .

ion:NO2minus  a              comp:InorganicCompound , ion:Ion ;
        crela:hasChemical_1  elem:N ;
        crela:hasChemical_2  ion:O2minus ;
        owl:sameAs           ion:Nitrite .

ion:Cation  a            owl:Class ;
        rdfs:comment     "An cation is an ion that has more protons than electrons such that the atom or molecule is positively charged. [Wikipedia]"@en ;
        rdfs:subClassOf  ion:Ion .

ion:Oplus  a               ion:Ion ;
        crela:hasChemical  elem:O ;
        prela:hasCharge    1 .

ion:Bicarbonite  a  ion:Ion .

ion:HydrogenCarbonate
        a       ion:Ion .

ion:Ion  a               owl:Class ;
        rdfs:comment     "An ion is an atom or molecule where the total number of electrons is not equal to the total number of protons, giving it a net positive or negative electrical charge. [Wikipedia]"@en ;
        rdfs:subClassOf  chem:Substance ;
        rdfs:subClassOf  [ a               owl:Restriction ;
                           owl:hasValue    pstate:Ionized ;
                           owl:onProperty  rela:hasState
                         ] .

ion:HeavyIon  a          owl:Class ;
        rdfs:subClassOf  ion:Ion .

ion:Carbonate  a  ion:Ion .

ion:CO3minusminus  a         comp:InorganicCompound , ion:Ion ;
        crela:hasChemical_1  elem:C ;
        crela:hasChemical_2  ion:O3minusminus ;
        owl:sameAs           ion:Carbonate .

ion:O2minus  a             ion:Ion ;
        crela:hasChemical  allo:O2 ;
        prela:hasCharge    -1 .

ion:NO3minus  a              comp:InorganicCompound , ion:Ion ;
        crela:hasChemical_1  elem:N ;
        crela:hasChemical_2  ion:O3minus ;
        owl:sameAs           ion:Nitrate .

ion:H4plus  a              ion:Ion ;
        crela:hasChemical  allo:H4 ;
        prela:hasCharge    1 .

ion:Anion  a             owl:Class ;
        rdfs:comment     "An anion is an ion that has more electrons than protons such that the atom or molecule is negatively charged. [Wikipedia]"@en ;
        rdfs:subClassOf  ion:Ion .

ion:Hplus  a               ion:Ion ;
        crela:hasChemical  elem:H ;
        prela:hasCharge    1 .

ion:HCO3minus  a             comp:InorganicCompound , ion:Ion ;
        crela:hasChemical_1  elem:H ;
        crela:hasChemical_2  elem:C ;
        crela:hasChemical_3  ion:O3minus ;
        owl:sameAs           ion:HydrogenCarbonate , ion:Bicarbonite .

ion:Ominus  a              ion:Ion ;
        crela:hasChemical  elem:O ;
        prela:hasCharge    -1 .
