@prefix : <http://sweetontology.net/matrRockIgneous/> .
@prefix owl: <http://www.w3.org/2002/07/owl#> .
@prefix rdf: <http://www.w3.org/1999/02/22-rdf-syntax-ns#> .
@prefix xml: <http://www.w3.org/XML/1998/namespace> .
@prefix xsd: <http://www.w3.org/2001/XMLSchema#> .
@prefix rdfs: <http://www.w3.org/2000/01/rdf-schema#> .
@base <http://sweetontology.net/matrRockIgneous> .

<http://sweetontology.net/matrRockIgneous> rdf:type owl:Ontology ;
                                            owl:imports <http://sweetontology.net/matr> ,
                                                        <http://sweetontology.net/matrRock> ,
                                                        <http://sweetontology.net/phenGeol> ,
                                                        <http://sweetontology.net/rela> ,
                                                        <http://sweetontology.net/relaProvenance> ,
                                                        <http://sweetontology.net/state> ,
                                                        <http://sweetontology.net/stateSolid> ;
                                            rdfs:label "SWEET Ontology" ;
                                            owl:versionInfo "3.1.0" .

#################################################################
#    Classes
#################################################################

###  http://sweetontology.net/matrRockIgneous/Aa
:Aa rdf:type owl:Class ;
    rdfs:subClassOf :ExtrusiveRock ,
                    :Lava ;
    rdfs:comment "One of three basic types of flow lava. Aa is basaltic lava characterized by a rough or rubbly surface composed of broken lava blocks called clinker. [Wikipedia]"@en .


###  http://sweetontology.net/matrRockIgneous/Andesite
:Andesite rdf:type owl:Class ;
          rdfs:subClassOf :VolcanicRock ;
          rdfs:comment "Volcanic rock (or lava) characteristically medium dark in color and containing 54 to 62 percent silica and moderate amounts of iron and magnesium."@en .


###  http://sweetontology.net/matrRockIgneous/AnorogenicIgneousRock
:AnorogenicIgneousRock rdf:type owl:Class ;
                       rdfs:subClassOf :IntrusiveRock ;
                       rdfs:comment "Anorogenic granites are formed above volcanic \"hot spot\" activity and have peculiar mineralogy and geochemistry. These granites are formed by melting of the lower crust under conditions that are usually extremely dry. The rhyolites of the Yellowstone caldera are examples of volcanic equivalents of A-type granite. [Wikipedia]"@en .


###  http://sweetontology.net/matrRockIgneous/Anorthosite
:Anorthosite rdf:type owl:Class ;
             rdfs:subClassOf :IgneousRock .


###  http://sweetontology.net/matrRockIgneous/Aphanite
:Aphanite rdf:type owl:Class ;
          rdfs:subClassOf :IgneousRock .


###  http://sweetontology.net/matrRockIgneous/Basalt
:Basalt rdf:type owl:Class ;
        rdfs:subClassOf :ExtrusiveRock ;
        rdfs:comment "Basalt is the most common extrusive volcanic rock. It is usually grey to black and fine-grained due to rapid cooling of lava at the surface of a planet. It may be porphyritic containing larger crystals in a fine matrix, or vesicular, or frothy scoria. Unweathered basalt is black or grey. On Earth, most basalt magmas have formed by decompression melting of the mantle. [Wikipedia]"@en .


###  http://sweetontology.net/matrRockIgneous/CinderCone
:CinderCone rdf:type owl:Class ;
            rdfs:subClassOf :VolcanicCone ;
            rdfs:comment "A volcanic cone built entirely of loose fragmented material (pyroclastics.)"@en .


###  http://sweetontology.net/matrRockIgneous/CompositeCone
:CompositeCone rdf:type owl:Class ;
               rdfs:subClassOf :VolcanicCone ;
               rdfs:comment "A steep volcanic cone built by both lava flows and pyroclastic eruptions"@en .


###  http://sweetontology.net/matrRockIgneous/Dacite
:Dacite rdf:type owl:Class ;
        rdfs:subClassOf :VolcanicRock ;
        rdfs:comment "Volcanic rock (or lava) that characteristically is light in color and contains 62% to 69% silica and moderate a mounts of sodium and potassium."@en .


###  http://sweetontology.net/matrRockIgneous/ExtrusiveRock
:ExtrusiveRock rdf:type owl:Class ;
               rdfs:subClassOf :IgneousRock ;
               rdfs:comment "Magma that has erupted onto the surface of the earth and cooled suffciently to form solid rock.  [Wikipedia]"@en .


###  http://sweetontology.net/matrRockIgneous/Felsic
:Felsic rdf:type owl:Class ;
        rdfs:subClassOf :IgneousRock ;
        owl:disjointWith :Mafic ;
        rdfs:comment "Felsic refers to silicate minerals, magma, and rocks which are enriched in the lighter elements such as silicon, oxygen, aluminium, sodium, and potassium. The term combines the words \"feldspar\" and \"silica.\" Felsic minerals are usually light in color and have specific gravities less than 3. Common felsic minerals include quartz, muscovite, orthoclase, and the sodium-rich plagioclase feldspars. The most common felsic rock is granite. On the opposite side of the rock spectrum are the iron and magnesium-rich mafic and ultramafic minerals and rocks. [Wikipedia]"@en .


###  http://sweetontology.net/matrRockIgneous/Hypabyssal
:Hypabyssal rdf:type owl:Class ;
            rdfs:subClassOf :IgneousRock ;
            rdfs:comment "Hypabyssal are igneous rocks formed at a depth in between the plutonic and volcanic rocks. They are characterized by their porphyritic nature (porphyry). They consist of phenocrysts embedded in a fine-grained groundmass. [Wikipedia]"@en .


###  http://sweetontology.net/matrRockIgneous/IgneousRock
:IgneousRock rdf:type owl:Class ;
             rdfs:subClassOf <http://sweetontology.net/matrRock/Rock> ,
                             [ rdf:type owl:Restriction ;
                               owl:onProperty <http://sweetontology.net/relaProvenance/hasGenesis> ;
                               owl:allValuesFrom <http://sweetontology.net/phenGeol/Igneous>
                             ] ;
             rdfs:comment "By definition, all igneous rock is formed from magma [Wikipedia]"@en .


###  http://sweetontology.net/matrRockIgneous/IntrusiveRock
:IntrusiveRock rdf:type owl:Class ;
               rdfs:subClassOf :IgneousRock ;
               rdfs:comment "Beneath the surface magma tends to cool slowly which allows for the growth of large crystals within the rock. Rocks formed in this way are intrusive or plutonic rocks. [Wikipedia]"@en .


###  http://sweetontology.net/matrRockIgneous/Kimberlite
:Kimberlite rdf:type owl:Class ;
            rdfs:subClassOf :IgneousRock ;
            rdfs:comment "Kimberlite is a type of potassic volcanic rock best known for sometimes containing diamonds. The general consensus reached on kimberlites is that they are formed deep within the mantle, at between 150 and 450 kilometres depth, from anomalously enriched exotic mantle compositions, and are erupted rapidly and violently, often with considerable carbon dioxide and other volatile components.  [Wikipedia]"@en .


###  http://sweetontology.net/matrRockIgneous/Lava
:Lava rdf:type owl:Class ;
      rdfs:subClassOf :ExtrusiveRock ,
                      :VolcanicRock ;
      rdfs:comment "Magma that extrudes onto the surface of earth is called lava.  [Wikipedia]"@en .


###  http://sweetontology.net/matrRockIgneous/Mafic
:Mafic rdf:type owl:Class ;
       rdfs:subClassOf :IgneousRock ;
       rdfs:comment "Mafic is an adjective describing a silicate mineral or rock that is rich in magnesium and iron; the term was derived by contracting \"magnesium\" and \"ferric\". Most mafic minerals are dark in color and the specific gravity is greater than 3. Common rock-forming mafic minerals include olivine, pyroxene, amphibole, and biotite. Common mafic rocks include basalt and gabbro. In terms of chemistry, mafic rocks are on the other side of the rock spectrum from the felsic rocks. The term roughly corresponds to the older basic rock class.Mafic lava, before cooling, has a low viscosity, in comparison to felsic lava, due to the lower silica content in mafic magma. Water and other volatiles can more easily and gradually escape from mafic lava, so eruptions of volcanoes made of mafic lavas are less explosively violent than felsic lava eruptions. Most mafic lava volcanoes are oceanic volcanoes, like Hawaii. [Wikipedia]"@en .


###  http://sweetontology.net/matrRockIgneous/Magma
:Magma rdf:type owl:Class ;
       rdfs:subClassOf :VolcanicRock ;
       rdfs:comment "Magma is molten rock that is found beneath the surface of the Earth.Magma is a complex high-temperature fluid substance in 3 phases; a system of silicate liquid, solid minerals, and perhaps a vapor phase. [Wikipedia]"@en .


###  http://sweetontology.net/matrRockIgneous/Obsidian
:Obsidian rdf:type owl:Class ;
          rdfs:subClassOf :ExtrusiveRock ,
                          :Lava ;
          rdfs:comment "Obsidian, a type of quenched lava, is a silicic black volcanic glass [Wikipedia]"@en .


###  http://sweetontology.net/matrRockIgneous/Pahoehoe
:Pahoehoe rdf:type owl:Class ;
          rdfs:subClassOf :ExtrusiveRock ,
                          :Lava ;
          rdfs:comment "Pahoehoe is basaltic lava that has a smooth, billowy, undulating, or ropy surface. These surface features are due to the movement of very fluid lava under a congealing surface crust. [Wikipedia]"@en .


###  http://sweetontology.net/matrRockIgneous/Peridotite
:Peridotite rdf:type owl:Class ;
            rdfs:subClassOf :IgneousRock .


###  http://sweetontology.net/matrRockIgneous/PillowLava
:PillowLava rdf:type owl:Class ;
            rdfs:subClassOf :ExtrusiveRock ,
                            :Lava ;
            rdfs:comment "Pillow lava is the lava structure typically formed when lava emerges from an underwater volcanic vent or subglacial volcano or a lava flow enters the ocean. However, pillow lava can also form when lava is erupted beneath thick glacial ice. The viscous lava gains a solid crust on contact with the water, and this crust cracks and oozes additional large blobs or \"pillows\" as more lava emerges from the advancing flow. Since water covers the majority of Earth's surface and most volcanoes are situated near or under bodies of water, pillow lava is very common. [Wikipedia]"@en .


###  http://sweetontology.net/matrRockIgneous/Pluton
:Pluton rdf:type owl:Class ;
        owl:equivalentClass :PlutonicRock ;
        rdfs:subClassOf :IntrusiveRock ;
        rdfs:comment "A pluton is an intrusive igneous rock body that crystallized from a magma slowly cooling below the surface of the Earth. Plutons include batholiths, dikes, sills, laccoliths, lopoliths, and other igneous bodies. In practice, \"pluton\" usually refers to a distinctive mass of igneous rock, typically kilometers in dimension, without a tabular shape like those of dikes and sills. Batholiths commonly are aggregations of plutons. The most common rock types in plutons are granite, granodiorite, tonalite, and quartz diorite. [Wikipedia]"@en .


###  http://sweetontology.net/matrRockIgneous/PlutonicRock
:PlutonicRock rdf:type owl:Class .


###  http://sweetontology.net/matrRockIgneous/Pumice
:Pumice rdf:type owl:Class ;
        rdfs:subClassOf :VolcanicRock ;
        rdfs:comment "Light-colored, frothy volcanic rock, usually of dacite or rhyolite composition, formed by the expansion of gas in erupting lava. Commonly seen as lumps or fragments of pea-size and larger, but can also occur abundantly as ash-sized particles."@en .


###  http://sweetontology.net/matrRockIgneous/Pyroclastic
:Pyroclastic rdf:type owl:Class ;
             rdfs:subClassOf :ExtrusiveRock ,
                             :VolcanicRock ;
             rdfs:comment "A descriptive term, usually for rock, which results from explosive magma ejection [Wikipedia]"@en .


###  http://sweetontology.net/matrRockIgneous/Rhyolite
:Rhyolite rdf:type owl:Class ;
          rdfs:subClassOf :VolcanicRock ;
          rdfs:comment "Volcanic rock (or lava) that characteristically is light in color, contains 69% silica or more, and is rich in potassium and sodium."@en .


###  http://sweetontology.net/matrRockIgneous/SpatterCone
:SpatterCone rdf:type owl:Class ;
             rdfs:subClassOf :VolcanicRock ;
             rdfs:comment "A low, steep-sided cone of spatter built up on a fissure or vent. It is usually of basaltic material."@en .


###  http://sweetontology.net/matrRockIgneous/Tephra
:Tephra rdf:type owl:Class ;
        rdfs:subClassOf :ExtrusiveRock ,
                        :VolcanicRock ;
        rdfs:comment "Tephra is a collective term (generally plural) used for all material -- regardless of size-- ejected during an explosive volcanic eruption."@en .


###  http://sweetontology.net/matrRockIgneous/Trachyandesite
:Trachyandesite rdf:type owl:Class ;
                rdfs:subClassOf :VolcanicRock ;
                rdfs:comment "An extrusive rock intermediate in composition between trachyte and andesite."@en .


###  http://sweetontology.net/matrRockIgneous/Trachybasalt
:Trachybasalt rdf:type owl:Class ;
              rdfs:subClassOf :VolcanicRock ;
              rdfs:comment "An extrusive rock intermediate in composition between trachyte and basalt."@en .


###  http://sweetontology.net/matrRockIgneous/Trachyte
:Trachyte rdf:type owl:Class ;
          rdfs:subClassOf :VolcanicRock ;
          rdfs:comment "A group of fine-grained, generally porphyritic, extrusive igneous rocks having alkali feldspar and minor mafic minerals as the main components, and possibly a small amount of sodic plagioclase."@en .


###  http://sweetontology.net/matrRockIgneous/Tuff
:Tuff rdf:type owl:Class ;
      rdfs:subClassOf :Pyroclastic ;
      rdfs:comment "Rock formed of pyroclastic material."@en .


###  http://sweetontology.net/matrRockIgneous/TuffCone
:TuffCone rdf:type owl:Class ;
          rdfs:subClassOf :VolcanicCone ;
          rdfs:comment "A type of volcanic cone formed by the interaction of basaltic magma and water. Smaller and steeper than a tuff ring."@en .


###  http://sweetontology.net/matrRockIgneous/TuffRing
:TuffRing rdf:type owl:Class ;
          rdfs:subClassOf :VolcanicRock ;
          rdfs:comment "A wide, low-rimmed, well-bedded accumulation of hyalo-clastic debris built around a volcanic vent located in a lake, coastal zone, marsh, or area of abundant ground water."@en .


###  http://sweetontology.net/matrRockIgneous/Ultramaphic
:Ultramaphic rdf:type owl:Class ;
             rdfs:subClassOf :ExtrusiveRock ,
                             :VolcanicRock ;
             rdfs:comment "The mantle is composed mostly of Ultramafic rocks (or see Igneous Primer) such as peridotite and dunite and their metamorphic equivalents (e.g. ecologite). [Wikipedia]"@en .


###  http://sweetontology.net/matrRockIgneous/VolcanicCone
:VolcanicCone rdf:type owl:Class ;
              rdfs:subClassOf :VolcanicRock ;
              rdfs:comment "A mound of loose material that was ejected ballistically."@en .


###  http://sweetontology.net/matrRockIgneous/VolcanicNeck
:VolcanicNeck rdf:type owl:Class ;
              rdfs:subClassOf :VolcanicRock ;
              rdfs:comment "A massive pillar of rock more resistant to erosion than the lavas and pyroclastic rocks of a volcanic cone."@en .


###  http://sweetontology.net/matrRockIgneous/VolcanicRock
:VolcanicRock rdf:type owl:Class ;
              rdfs:subClassOf :ExtrusiveRock ;
              rdfs:comment "Volcanic rock is an igneous rock produced by extrusion from a volcano. It has various subtypes based on chemical composition and whether the extrusion was violent (pyroclastic) or slow (laval). [Wikipedia]"@en .


###  http://sweetontology.net/matrRockIgneous/Xenocryst
:Xenocryst rdf:type owl:Class ;
           rdfs:subClassOf <http://sweetontology.net/matr/Mixture> ,
                           [ rdf:type owl:Restriction ;
                             owl:onProperty <http://sweetontology.net/rela/hasState> ;
                             owl:hasValue <http://sweetontology.net/stateSolid/Crystal>
                           ] ;
           rdfs:comment "A xenocryst is an individual foreign crystal included within an igneous body. Examples of xenocrysts are quartz crystals in a silica-deficient lava and diamonds within kimberlite diatremes. [Wikipedia]"@en .


###  http://sweetontology.net/matrRockIgneous/Xenolith
:Xenolith rdf:type owl:Class ;
          rdfs:subClassOf <http://sweetontology.net/matrRock/Rock> ;
          rdfs:comment "A xenolith is a rock fragment which becomes enveloped in a larger rock during the latter's development and hardening. The term xenolith is almost exclusively used to describe inclusions in igneous rock during magma emplacement and eruption [Wikipedia]"@en .


###  http://sweetontology.net/phenGeol/Igneous
<http://sweetontology.net/phenGeol/Igneous> rdf:type owl:Class .


#################################################################
#    Individuals
#################################################################

###  http://sweetontology.net/stateSolid/Crystal
<http://sweetontology.net/stateSolid/Crystal> rdf:type owl:NamedIndividual .


###  Generated by the OWL API (version 5.1.2.2017-10-13T07:13:07Z) https://github.com/owlcs/owlapi/
