@base          <http://sweetontology.net/matrWater> .
@prefix mrela: <http://sweetontology.net/relaMath/> .
@prefix comp:  <http://sweetontology.net/matrCompound/> .
@prefix crela: <http://sweetontology.net/relaChemical/> .
@prefix chem:  <http://sweetontology.net/matr/> .
@prefix owl:   <http://www.w3.org/2002/07/owl#> .
@prefix pstate: <http://sweetontology.net/statePhysical/> .
@prefix xsd:   <http://www.w3.org/2001/XMLSchema#> .
@prefix rdfs:  <http://www.w3.org/2000/01/rdf-schema#> .
@prefix mrela2: <http://sweetontology.net/relaMath/> .
@prefix water: <http://sweetontology.net/matrWater/> .
@prefix prrela: <http://sweetontology.net/relaProvenance/> .
@prefix srela: <http://sweetontology.net/relaSpace/> .
@prefix cstate: <http://sweetontology.net/stateChemical/> .
@prefix prec:  <http://sweetontology.net/phenAtmoPrecipitation/> .
@prefix rdf:   <http://www.w3.org/1999/02/22-rdf-syntax-ns#> .
@prefix sstate: <http://sweetontology.net/stateSolid/> .
@prefix realm: <http://sweetontology.net/realm/> .
@prefix state: <http://sweetontology.net/state/> .
@prefix xten2: <http://sweetontology.net/propSpaceDistance/> .
@prefix xten:  <http://sweetontology.net/propSpaceDistance/> .
@prefix rela:  <http://sweetontology.net/rela/> .
@prefix human: <http://sweetontology.net/human/> .

water:SeaWater  a        owl:Class ;
        rdfs:subClassOf  water:SaltWater .

water:Snow  a            owl:Class ;
        rdfs:subClassOf  water:WaterSubstance ;
        rdfs:subClassOf  [ a               owl:Restriction ;
                           owl:hasValue    pstate:Solid ;
                           owl:onProperty  rela:hasState
                         ] .

water:Hydrate  a         owl:Class ;
        rdfs:subClassOf  water:WaterSubstance .

water:DepthHoar  a       owl:Class ;
        rdfs:comment     "Depth hoares are large crystals occurring at the base of a snowpack that form due to the fact that a snow crystal can grow over time as moisture freezes onto the crystal from vapor that is rising in the snowpack."@en ;
        rdfs:subClassOf  water:IceCrystal .

water:DrizzleDrop  a     owl:Class ;
        rdfs:subClassOf  water:Drop ;
        rdfs:subClassOf  [ a               owl:Restriction ;
                           owl:hasValue    [ a                     xten:SizeRange_micron ;
                                             mrela2:hasUpperBound  "200"^^xsd:double
                                           ] ;
                           owl:onProperty  srela:diameter
                         ] .

water:FreshWater  a      owl:Class ;
        rdfs:subClassOf  water:WaterSubstance .

water:IceParticle  a         owl:Class ;
        owl:equivalentClass  water:IceCrystal .

water:Frost  a           owl:Class ;
        rdfs:subClassOf  water:WaterSubstance ;
        rdfs:subClassOf  [ a               owl:Restriction ;
                           owl:hasValue    pstate:Frozen ;
                           owl:onProperty  rela:hasState
                         ] .

water:Brine  a            owl:Class ;
        rdfs:subClassOf   water:SaltWater ;
        owl:disjointWith  water:SalineWater .

water:HoarCrystal  a     owl:Class ;
        rdfs:subClassOf  water:IceCrystal .

water:WaterSubstance  a  owl:Class ;
        rdfs:subClassOf  chem:Substance ;
        rdfs:subClassOf  [ a               owl:Restriction ;
                           owl:hasValue    comp:Water ;
                           owl:onProperty  crela:hasChemical
                         ] .

water:Groundwater  a     owl:Class ;
        rdfs:subClassOf  water:LiquidWater ;
        rdfs:subClassOf  [ a                  owl:Restriction ;
                           owl:allValuesFrom  realm:PlanetarySurface ;
                           owl:onProperty     srela:below
                         ] .

water:WaterMixture  a    owl:Class ;
        rdfs:subClassOf  chem:Mixture ;
        rdfs:subClassOf  [ a               owl:Restriction ;
                           owl:hasValue    comp:H2O ;
                           owl:onProperty  crela:hasChemical_1
                         ] .

water:Rime  a            owl:Class ;
        rdfs:comment     "A white or milky and opaque granular deposit of ice formed by the rapid freezing of supercooled water drops as they impinge upon an exposed object."@en ;
        rdfs:subClassOf  water:Ice .

water:Wastewater  a      owl:Class ;
        rdfs:subClassOf  water:Effluent .

water:Ice  a             owl:Class ;
        rdfs:subClassOf  water:WaterSubstance ;
        rdfs:subClassOf  [ a               owl:Restriction ;
                           owl:hasValue    pstate:Solid ;
                           owl:onProperty  rela:hasState
                         ] .

<>      a                owl:Ontology ;
        rdfs:label       "SWEET Ontology" ;
        owl:imports      <relaChemical> , <relaProvenance> , <rela> , <propSpaceDistance> , <statePhysical> , <matrCompound> , <stateSolid> , <realm> , <relaSpace> , <human> , <relaMath> , <state> , <stateChemical> , <matr> , <phenAtmoPrecipitation> ;
        owl:versionInfo  "3.1.0" .

water:Drop  a            owl:Class ;
        rdfs:subClassOf  water:LiquidWater .

water:SnowFacies  a      owl:Class ;
        rdfs:subClassOf  water:IceCrystal .

water:GrayWater  a       owl:Class ;
        rdfs:subClassOf  water:WaterMixture .

water:Rainwater  a       owl:Class ;
        rdfs:subClassOf  water:LiquidWater ;
        rdfs:subClassOf  [ a                  owl:Restriction ;
                           owl:allValuesFrom  prec:Rainfall ;
                           owl:onProperty     prrela:hasSource
                         ] .

water:Dew  a             owl:Class ;
        rdfs:subClassOf  water:LiquidWater .

water:SaltWater  a        owl:Class ;
        rdfs:subClassOf   water:WaterSubstance ;
        rdfs:subClassOf   [ a               owl:Restriction ;
                            owl:hasValue    cstate:Saline ;
                            owl:onProperty  rela:hasState
                          ] ;
        owl:disjointWith  water:FreshWater .

water:Firn  a            owl:Class ;
        rdfs:comment     "Firn is partially-compacted névé, a type of snow that has been left over from past seasons and has been recrystallized into a substance denser than névé. It is ice that is at an intermediate stage between snow and glacial ice. Firn has the appearance of wet sugar, but has a hardness that makes it extremely resistant to shovelling. It generally has a density greater than 550 kg/m³ and is often found underneath the snow that accumulates at the head of a glacier."@en ;
        rdfs:subClassOf  water:IceCrystal .

water:BrackishWater  a   owl:Class ;
        rdfs:comment     "Brackish water is water that has more salinity than fresh water, but not as much as seawater. It may result from mixing of seawater with fresh water, as in estuaries, or it may occur in brackish fossil aquifers."@en ;
        rdfs:subClassOf  water:SaltWater ;
        rdfs:subClassOf  [ a               owl:Restriction ;
                           owl:hasValue    cstate:Brackish ;
                           owl:onProperty  rela:hasState
                         ] .

water:WaterVapor  a          owl:Class ;
        rdfs:subClassOf      water:WaterSubstance ;
        rdfs:subClassOf      [ a               owl:Restriction ;
                               owl:hasValue    pstate:Gas ;
                               owl:onProperty  rela:hasState
                             ] ;
        owl:equivalentClass  water:Steam .

water:Effluent  a        owl:Class ;
        rdfs:subClassOf  water:WaterMixture .

water:SalineWater  a     owl:Class ;
        rdfs:subClassOf  water:SaltWater .

water:Steam  a  owl:Class .

water:RainDrop  a        owl:Class ;
        rdfs:subClassOf  water:Drop ;
        rdfs:subClassOf  [ a               owl:Restriction ;
                           owl:hasValue    [ a                     xten:SizeRange_micron ;
                                             mrela2:hasLowerBound  "500"^^xsd:double
                                           ] ;
                           owl:onProperty  srela:diameter
                         ] .

water:BlackWater  a      owl:Class ;
        rdfs:subClassOf  water:WaterMixture .

water:Sewage  a          owl:Class ;
        rdfs:subClassOf  water:Effluent .

water:GranularIce  a     owl:Class ;
        rdfs:subClassOf  water:Ice .

water:DrinkingWater  a   owl:Class ;
        rdfs:subClassOf  human:HumanNeed , water:WaterMixture .

water:LiquidWater  a     owl:Class ;
        rdfs:subClassOf  water:WaterSubstance ;
        rdfs:subClassOf  [ a               owl:Restriction ;
                           owl:hasValue    pstate:Liquid ;
                           owl:onProperty  rela:hasState
                         ] .

water:CloudDrop  a       owl:Class ;
        rdfs:subClassOf  water:Drop ;
        rdfs:subClassOf  [ a               owl:Restriction ;
                           owl:hasValue    [ a                     xten:SizeRange_micron ;
                                             mrela2:hasLowerBound  "200"^^xsd:double ;
                                             mrela2:hasUpperBound  "500"^^xsd:double
                                           ] ;
                           owl:onProperty  srela:diameter
                         ] .

water:IceCrystal  a      owl:Class ;
        rdfs:subClassOf  water:Ice ;
        rdfs:subClassOf  [ a               owl:Restriction ;
                           owl:hasValue    sstate:Crystal ;
                           owl:onProperty  rela:hasState
                         ] .

water:SnowGrain  a       owl:Class ;
        rdfs:subClassOf  water:Snow .
