@base          <http://sweetontology.net/phenSolid> .
@prefix proc:  <http://sweetontology.net/procPhysical/> .
@prefix solid: <http://sweetontology.net/phenSolid/> .
@prefix phen:  <http://sweetontology.net/phen/> .
@prefix rdf:   <http://www.w3.org/1999/02/22-rdf-syntax-ns#> .
@prefix owl:   <http://www.w3.org/2002/07/owl#> .
@prefix pstate: <http://sweetontology.net/statePhysical/> .
@prefix xsd:   <http://www.w3.org/2001/XMLSchema#> .
@prefix rdfs:  <http://www.w3.org/2000/01/rdf-schema#> .
@prefix sgeo:  <http://sweetontology.net/stateRoleGeographic/> .
@prefix rela:  <http://sweetontology.net/rela/> .

solid:Cataclasis  a      owl:Class ;
        rdfs:subClassOf  solid:Fracture .

solid:Harden  a          owl:Class ;
        rdfs:subClassOf  solid:SolidPhenomena .

solid:Compaction  a      owl:Class ;
        rdfs:subClassOf  solid:SolidPhenomena .

solid:Distortion  a      owl:Class ;
        rdfs:subClassOf  solid:SolidPhenomena .

solid:Subsidence  a  owl:Class .

solid:Strain  a          owl:Class ;
        rdfs:subClassOf  solid:SolidPhenomena .

solid:Slip  a            owl:Class ;
        rdfs:subClassOf  solid:SolidPhenomena .

solid:Diagenesis  a      owl:Class ;
        rdfs:subClassOf  solid:Consolidation .

solid:Pore  a            owl:Class ;
        rdfs:subClassOf  sgeo:Separation .

solid:Buckle  a          owl:Class ;
        rdfs:subClassOf  solid:SolidPhenomena .

solid:Solidify  a        owl:Class ;
        rdfs:subClassOf  solid:SolidPhenomena .

solid:Cleavage  a        owl:Class ;
        rdfs:subClassOf  solid:Crack .

solid:Break  a           owl:Class ;
        rdfs:subClassOf  solid:SolidPhenomena .

solid:Thinning  a        owl:Class ;
        rdfs:subClassOf  solid:SolidPhenomena .

solid:Conchoidal  a      owl:Class ;
        rdfs:comment     "The most common fracture type is conchoidal. This is a smoothly curved fracture that is familiar to people who have examined broken glass."@en ;
        rdfs:subClassOf  solid:Fracture .

solid:Accretion  a           owl:Class ;
        rdfs:subClassOf      solid:SolidPhenomena ;
        owl:equivalentClass  solid:Coalescence .

solid:Elongate  a  owl:Class .

solid:Deformation  a         owl:Class ;
        rdfs:subClassOf      solid:SolidPhenomena ;
        owl:equivalentClass  solid:Deform .

solid:Crack  a           owl:Class ;
        rdfs:subClassOf  sgeo:Separation .

solid:Subconchoidal  a   owl:Class ;
        rdfs:comment     "Similar to conchoidal, just not as curved, but still smooth."@en ;
        rdfs:subClassOf  solid:Fracture .

solid:Clumping  a  owl:Class .

solid:Extension  a       owl:Class ;
        rdfs:subClassOf  solid:SolidPhenomena .

solid:Fracture  a        owl:Class ;
        rdfs:subClassOf  solid:Failure .

solid:Disintegration  a  owl:Class .

solid:Coalescence  a  owl:Class .

solid:SolidPhenomena  a  owl:Class ;
        rdfs:subClassOf  phen:Phenomena ;
        rdfs:subClassOf  [ a               owl:Restriction ;
                           owl:hasValue    pstate:Solid ;
                           owl:onProperty  rela:hasState
                         ] .

solid:Metamorphism  a    owl:Class ;
        rdfs:subClassOf  solid:Consolidation .

solid:Congelation  a     owl:Class ;
        rdfs:subClassOf  solid:SolidPhenomena .

solid:Fissure  a         owl:Class ;
        rdfs:subClassOf  solid:Crack .

solid:Ablation  a        owl:Class ;
        rdfs:comment     "all processes that remove material from an object, such as a glacier" ;
        rdfs:label       "Ablation" ;
        rdfs:subClassOf  solid:SolidPhenomena .

solid:Cementation  a     owl:Class ;
        rdfs:subClassOf  solid:Consolidation .

solid:Disintegrate  a        owl:Class ;
        rdfs:subClassOf      solid:Failure ;
        owl:equivalentClass  solid:Disintegration .

solid:Spintery  a        owl:Class ;
        rdfs:comment     "Splintery is a fracture type that occurs in fibrous or finely acicular minerals and in minerals that have a relatively stronger structure in one direction than the other two."@en ;
        rdfs:subClassOf  solid:Fracture .

solid:Erode  a               owl:Class ;
        rdfs:comment         "Erosion is displacement of solids (soil, mud, rock and other particles) usually by the agents of currents such as, wind, water, or ice by downward or down-slope movement in response to gravity or by living organisms (in the case of bioerosion)." ;
        rdfs:subClassOf      solid:SolidPhenomena ;
        owl:equivalentClass  solid:Erosion .

solid:Failure  a         owl:Class ;
        rdfs:subClassOf  solid:SolidPhenomena .

solid:Shatter  a         owl:Class ;
        rdfs:subClassOf  solid:Failure .

solid:Consolidation  a   owl:Class ;
        rdfs:subClassOf  solid:SolidPhenomena .

solid:BergeronFindeisenProcess
        a                owl:Class ;
        rdfs:comment     "A theoretical explanation of the process by which precipitation particles may form within a mixed cloud (composed of both ice crystals and liquid water drops)."@en ;
        rdfs:subClassOf  solid:Coalescence .

solid:Elongation  a  owl:Class .

solid:Rupture  a         owl:Class ;
        rdfs:subClassOf  solid:Fracture .

solid:Stretch  a             owl:Class ;
        rdfs:subClassOf      solid:SolidPhenomena ;
        owl:equivalentClass  solid:Elongate , solid:Elongation .

solid:Wasting  a         owl:Class ;
        rdfs:subClassOf  solid:SolidPhenomena .

solid:Deform  a  owl:Class .

solid:Dislocation  a     owl:Class ;
        rdfs:subClassOf  solid:SolidPhenomena .

solid:Fault  a               owl:Class ;
        rdfs:comment         "In geology, a fault or fault line is a planar rock fracture, which shows evidence of relative movement. Large faults within the Earth's crust are the result of shear motion and active fault zones are the causal locations of most earthquakes. Earthquakes are caused by energy release during rapid slippage along faults. The largest examples are at tectonic plate boundaries but many faults occur far from active plate boundaries. Since faults do not usually consist of a single, clean fracture, the term fault zone is used when referring to the zone of complex deformation that is associated with the fault plane."@en ;
        rdfs:subClassOf      solid:Fracture ;
        owl:equivalentClass  solid:FaultLine .

solid:Earthy  a          owl:Class ;
        rdfs:comment     "a fracture that produces a texture similar to broken children's clay. It is found in minerals that are generally massive and loosely consolidated."@en ;
        rdfs:subClassOf  solid:Fracture .

solid:Jagged  a          owl:Class ;
        rdfs:comment     "Jagged has sharp points or edges that catch on a finger that's rubbed across the surface."@en ;
        rdfs:subClassOf  solid:Fracture .

solid:Bend  a            owl:Class ;
        rdfs:subClassOf  solid:SolidPhenomena .

solid:Rip  a             owl:Class ;
        rdfs:subClassOf  solid:SolidPhenomena .

solid:Solidification  a  owl:Class ;
        rdfs:subClassOf  solid:SolidPhenomena .

solid:PoreSpace  a           owl:Class ;
        owl:equivalentClass  solid:Pore .

solid:Joint  a           owl:Class ;
        rdfs:subClassOf  solid:Crack .

solid:Clump  a               owl:Class ;
        rdfs:subClassOf      solid:Accretion ;
        owl:equivalentClass  solid:Clumping .

solid:Comminution  a     owl:Class ;
        rdfs:subClassOf  solid:SolidPhenomena .

solid:Subside  a             owl:Class ;
        rdfs:subClassOf      solid:SolidPhenomena ;
        owl:equivalentClass  solid:Subsidence .

solid:Erosion  a  owl:Class .

solid:FaultLine  a  owl:Class .

solid:Ridging  a         owl:Class ;
        rdfs:subClassOf  solid:SolidPhenomena .

solid:Fold  a            owl:Class ;
        rdfs:comment     "The term fold is used in geology when one or a stack of originally flat and planar surfaces, such as sedimentary strata, are bent or curved as a result of plastic (i.e. permanent) deformation."@en ;
        rdfs:subClassOf  solid:Deformation .

solid:Shear  a           owl:Class ;
        rdfs:subClassOf  solid:SolidPhenomena .

solid:Microfracture  a   owl:Class ;
        rdfs:subClassOf  solid:Fracture .

<>      a                owl:Ontology ;
        rdfs:label       "SWEET Ontology" ;
        owl:imports      <statePhysical> , <rela> , <procPhysical> , <phen> , <stateRoleGeographic> ;
        owl:versionInfo  "3.1.0" .

solid:GrainSizeSorting
        a                owl:Class ;
        rdfs:subClassOf  solid:SolidPhenomena .
