@prefix : <http://sweetontology.net/phenAtmoWindMesoscale/> .
@prefix owl: <http://www.w3.org/2002/07/owl#> .
@prefix rdf: <http://www.w3.org/1999/02/22-rdf-syntax-ns#> .
@prefix xml: <http://www.w3.org/XML/1998/namespace> .
@prefix xsd: <http://www.w3.org/2001/XMLSchema#> .
@prefix rdfs: <http://www.w3.org/2000/01/rdf-schema#> .
@base <http://sweetontology.net/phenAtmoWindMesoscale> .

<http://sweetontology.net/phenAtmoWindMesoscale> rdf:type owl:Ontology ;
                                                  owl:imports <http://sweetontology.net/phenAtmo> ,
                                                              <http://sweetontology.net/phenAtmoFog> ,
                                                              <http://sweetontology.net/phenAtmoPrecipitation> ,
                                                              <http://sweetontology.net/phenFluidDynamics> ,
                                                              <http://sweetontology.net/procPhysical> ,
                                                              <http://sweetontology.net/realm> ,
                                                              <http://sweetontology.net/realmCryo> ,
                                                              <http://sweetontology.net/realmHydroBody> ,
                                                              <http://sweetontology.net/realmLandAeolian> ,
                                                              <http://sweetontology.net/realmLandFluvial> ,
                                                              <http://sweetontology.net/realmLandOrographic> ,
                                                              <http://sweetontology.net/rela> ,
                                                              <http://sweetontology.net/relaSpace> ,
                                                              <http://sweetontology.net/reprSpaceDirection> ;
                                                  rdfs:label "SWEET Ontology" ;
                                                  owl:versionInfo "3.1.0" .

#################################################################
#    Object Properties
#################################################################

###  http://sweetontology.net/rela/hasPhenomena
<http://sweetontology.net/rela/hasPhenomena> rdf:type owl:ObjectProperty .


###  http://sweetontology.net/rela/hasProcess
<http://sweetontology.net/rela/hasProcess> rdf:type owl:ObjectProperty .


###  http://sweetontology.net/rela/hasRealm
<http://sweetontology.net/rela/hasRealm> rdf:type owl:ObjectProperty .


###  http://sweetontology.net/relaSpace/hasDirection
<http://sweetontology.net/relaSpace/hasDirection> rdf:type owl:ObjectProperty .


###  http://sweetontology.net/relaSpace/originatesFrom
<http://sweetontology.net/relaSpace/originatesFrom> rdf:type owl:ObjectProperty .


#################################################################
#    Classes
#################################################################

###  http://sweetontology.net/phenAtmoWindMesoscale/AnabaticWind
:AnabaticWind rdf:type owl:Class ;
              rdfs:subClassOf :MountainWind ,
                              [ rdf:type owl:Restriction ;
                                owl:onProperty <http://sweetontology.net/rela/hasProcess> ;
                                owl:allValuesFrom <http://sweetontology.net/procPhysical/Heating>
                              ] ;
              rdfs:comment "In mountain meteorology, an upslope wind driven by heating (usually daytime insolation) at the slope surface under fair-weather conditions."@en .


###  http://sweetontology.net/phenAtmoWindMesoscale/BarrierJet
:BarrierJet rdf:type owl:Class ;
            rdfs:subClassOf :MountainWind ;
            rdfs:comment "A jet on the windward side of a mountain barrier, blowing parallel to the barrier."@en .


###  http://sweetontology.net/phenAtmoWindMesoscale/BlackSquall
:BlackSquall rdf:type owl:Class ;
             rdfs:subClassOf :Squall ;
             rdfs:comment "A squall accompanied by dark clouds and generally by heavy rain."@en .


###  http://sweetontology.net/phenAtmoWindMesoscale/BookEndVorticities
:BookEndVorticities rdf:type owl:Class ;
                    rdfs:subClassOf <http://sweetontology.net/phenAtmo/AtmosphericPhenomena> ,
                                    <http://sweetontology.net/phenFluidDynamics/Vortex> ;
                    rdfs:comment "Mesoscale vortices observed at the ends of a line segment of convective cells, usually cyclonic on the northern end of the system and anticyclonic on the southern end, for an environment of westerly vertical wind shear"@en .


###  http://sweetontology.net/phenAtmoWindMesoscale/Bora
:Bora rdf:type owl:Class ;
      rdfs:subClassOf :FallWind ;
      rdfs:comment "A fall wind with a source so cold that, when the air reaches the lowlands or coast, the dynamic warming is insufficient to raise the air temperature to the normal level for the region; hence it appears as a cold wind"@en .


###  http://sweetontology.net/phenAtmoWindMesoscale/CanyonWind
:CanyonWind rdf:type owl:Class ;
            rdfs:subClassOf :MountainWind ,
                            [ rdf:type owl:Restriction ;
                              owl:onProperty <http://sweetontology.net/rela/hasProcess> ;
                              owl:allValuesFrom <http://sweetontology.net/procPhysical/Cooling>
                            ] ;
            rdfs:comment "The mountain wind of a canyon, that is, the nighttime down-canyon flow of air caused by cooling at the canyon walls."@en .


###  http://sweetontology.net/phenAtmoWindMesoscale/CherguiWind
:CherguiWind rdf:type owl:Class ;
             rdfs:subClassOf :DesertWind ;
             rdfs:comment "An east or southeast desert wind in Morocco (North Africa), especially in the north."@en .


###  http://sweetontology.net/phenAtmoWindMesoscale/ChinookWind
:ChinookWind rdf:type owl:Class ;
             owl:equivalentClass :Foehn ;
             rdfs:comment "The name given to the foehn in western North America, especially on the plains to the lee or eastern side of the Rocky Mountains in the US and Canada." .


###  http://sweetontology.net/phenAtmoWindMesoscale/DesertWind
:DesertWind rdf:type owl:Class ;
            rdfs:subClassOf :MesoscaleWind ,
                            [ rdf:type owl:Restriction ;
                              owl:onProperty <http://sweetontology.net/rela/hasRealm> ;
                              owl:allValuesFrom <http://sweetontology.net/realmLandAeolian/Desert>
                            ] ;
            rdfs:comment "A wind blowing from the desert."@en .


###  http://sweetontology.net/phenAtmoWindMesoscale/DownslopeWind
:DownslopeWind rdf:type owl:Class ;
               rdfs:subClassOf :MountainWind ;
               rdfs:comment "A wind directed down a slope, often used to describe winds produced by processes larger in scale than the slope."@en .


###  http://sweetontology.net/phenAtmoWindMesoscale/DownslopeWindStorm
:DownslopeWindStorm rdf:type owl:Class ;
                    rdfs:subClassOf :DownslopeWind ;
                    rdfs:comment "A very strong, usually gusty, and occasionally, violent wind that blows down the lee slope of a mountain range, often reaching its peak strength near the foot of the mountains and weakening rapidly father away from the mountains."@en .


###  http://sweetontology.net/phenAtmoWindMesoscale/FallWind
:FallWind rdf:type owl:Class ;
          rdfs:subClassOf :KatabaticWind ,
                          :MountainWind ;
          rdfs:comment "A wind that accelerates as it moves downslope because of its low temperature and greater density."@en .


###  http://sweetontology.net/phenAtmoWindMesoscale/Foehn
:Foehn rdf:type owl:Class ;
       rdfs:subClassOf :MountainWind ,
                       [ rdf:type owl:Restriction ;
                         owl:onProperty <http://sweetontology.net/rela/hasProcess> ;
                         owl:allValuesFrom <http://sweetontology.net/procPhysical/Heating>
                       ] ;
       rdfs:comment "A warm, dry, downslope wind descending the lee side of the Alps as a result of synoptic-scale, cross-barrier flow over the mountain range."@en .


###  http://sweetontology.net/phenAtmoWindMesoscale/FogWind
:FogWind rdf:type owl:Class ;
         rdfs:subClassOf :Squall ,
                         [ rdf:type owl:Restriction ;
                           owl:onProperty <http://sweetontology.net/rela/hasPhenomena> ;
                           owl:allValuesFrom <http://sweetontology.net/phenAtmoFog/Fog>
                         ] ;
         rdfs:comment "The humid east wind that crosses the divide of the Andes east of Lake Titicaca and descends on the west in violent squalls; probably the same as puelche."@en .


###  http://sweetontology.net/phenAtmoWindMesoscale/Forano
:Forano rdf:type owl:Class ;
        rdfs:subClassOf :SeaBreeze ;
        rdfs:comment "A sea breeze of Naples in Italy."@en .


###  http://sweetontology.net/phenAtmoWindMesoscale/Galerne
:Galerne rdf:type owl:Class ;
         rdfs:subClassOf :Squall ;
         rdfs:comment "A squally northwesterly wind, cold, humid, and showery, that occurs in the rear of a low pressure area over the English Channel and off the Atlantic coast of France and northern Spain."@en .


###  http://sweetontology.net/phenAtmoWindMesoscale/Gallego
:Gallego rdf:type owl:Class ;
         rdfs:subClassOf :MountainWind ;
         rdfs:comment "A strong, low-level wind through either a relatively level channel between two mountain ranges or a gap in a mountain barrier; originally applied to strong (10?20 m s-1) easterly winds through the Strait of Juan de Fuca between the Olympic Mountains of western Washington State and the mountains of Vancouver Island, British Columbia, Canada. There they have been defined as ?a flow of air in a sea level channel that accelerates under the influence of a pressure gradient parallel to the axis of the channel.? As in the case of mountain- gap winds, this term has also been applied to pressure-gradient winds accelerating through a gap in a mountain barrier. The pressure gradient often results from a stable, post-cold-frontal anticyclone approaching the barrier and being partially blocked (see blocking) as it ascends the barrier, except for the flow through the gap or channel. The tehuantepecer of Central America is a well- known gap wind by this definition. These flows have sometimes been referred to as jet-effect wind and canyon wind."@en .


###  http://sweetontology.net/phenAtmoWindMesoscale/Garbin
:Garbin rdf:type owl:Class ;
        rdfs:subClassOf :SeaBreeze ;
        rdfs:comment "A sea breeze.  In southwest France it refers to a southwesterly sea breeze that sets in about 9 A.M., reaches it maximum towards 2 P.M. and ceases about 5 P.M."@en .


###  http://sweetontology.net/phenAtmoWindMesoscale/Gending
:Gending rdf:type owl:Class ;
         rdfs:subClassOf :MountainWind ;
         rdfs:comment "A local dry wind in the northern plains of Java, resembling the foehn. It is caused by a wind crossing the mountains near the south coast and pushing between the volcanoes."@en .


###  http://sweetontology.net/phenAtmoWindMesoscale/Gharbi
:Gharbi rdf:type owl:Class ;
        rdfs:subClassOf :OceanWind ;
        rdfs:comment "A fresh westerly wind of oceanic origin in Morocco."@en .


###  http://sweetontology.net/phenAtmoWindMesoscale/Gharra
:Gharra rdf:type owl:Class ;
        rdfs:subClassOf :Squall ;
        rdfs:comment "Hard squalls from the northeast in Libya and Africa. They are sudden and frequent and are accompanied by heavy rain and thunder."@en .


###  http://sweetontology.net/phenAtmoWindMesoscale/Ghibli
:Ghibli rdf:type owl:Class ;
        rdfs:subClassOf :DesertWind ;
        rdfs:comment "A hot dust-bearing desert wind in Tripolitania (northwestern Libya), similar to the foehn."@en .


###  http://sweetontology.net/phenAtmoWindMesoscale/GlacierWind
:GlacierWind rdf:type owl:Class ;
             rdfs:subClassOf :GravityWind ,
                             [ rdf:type owl:Restriction ;
                               owl:onProperty <http://sweetontology.net/rela/hasRealm> ;
                               owl:allValuesFrom <http://sweetontology.net/realmCryo/Glacier>
                             ] ;
             rdfs:comment "A shallow gravity wind, along the icy surface of a glacier, caused by the temperature difference between the air in contact with the glacier and free air at the same altitude. The glacier wind does not reverse itself diurnally as do mountain and valley winds, but it reaches its maximum intensity in the early afternoon. The glacier wind is characterized by strongly turbulent flow. See katabatic wind."@en .


###  http://sweetontology.net/phenAtmoWindMesoscale/GorgeWind
:GorgeWind rdf:type owl:Class ;
           rdfs:subClassOf :MesoscaleWind ,
                           [ rdf:type owl:Restriction ;
                             owl:onProperty <http://sweetontology.net/rela/hasRealm> ;
                             owl:allValuesFrom <http://sweetontology.net/realmLandFluvial/Gorge>
                           ] ;
           rdfs:comment "A gap wind or canyon wind through a gorge."@en .


###  http://sweetontology.net/phenAtmoWindMesoscale/GravityWind
:GravityWind rdf:type owl:Class ;
             rdfs:subClassOf :MountainWind ,
                             [ rdf:type owl:Restriction ;
                               owl:onProperty <http://sweetontology.net/rela/hasProcess> ;
                               owl:allValuesFrom <http://sweetontology.net/procPhysical/Gravity>
                             ] ;
             rdfs:comment "A wind resulting from cold air running or flowing down a slope, caused by greater air density near the slope than at the same altitude some distance horizontally from the slope."@en .


###  http://sweetontology.net/phenAtmoWindMesoscale/Greco
:Greco rdf:type owl:Class ;
       rdfs:subClassOf :OceanWind ;
       rdfs:comment "An Italian name for the northeast wind. It was given by Roman sailors to the northeast wind in the Gulf of Lions because it came from the direction of the Greek colony of Marsala (Marseilles). Wind names of similar origin are common in the western Mediterranean, for example, gregale."@en .


###  http://sweetontology.net/phenAtmoWindMesoscale/Gregale
:Gregale rdf:type owl:Class ;
         rdfs:subClassOf :MesoscaleWind ;
         rdfs:comment "The Maltese and best-known variant of a term for a strong northeast wind in the central and western Mediterranean and adjacent European land areas (stronger than the levante)."@en .


###  http://sweetontology.net/phenAtmoWindMesoscale/GregauWind
:GregauWind rdf:type owl:Class ;
            rdfs:subClassOf :MesoscaleWind ;
            rdfs:comment "In the Tirol, an east wind during March and April."@en .


###  http://sweetontology.net/phenAtmoWindMesoscale/GullySquall
:GullySquall rdf:type owl:Class ;
             rdfs:subClassOf :MountainWind ,
                             :Squall ;
             rdfs:comment "A nautical term for a violent squall of wind from mountain ravines on the Pacific side of Central America."@en .


###  http://sweetontology.net/phenAtmoWindMesoscale/Haboob
:Haboob rdf:type owl:Class ;
        rdfs:subClassOf :MesoscaleWind ;
        rdfs:comment "A strong wind and sandstorm or duststorm in northern and central Sudan, especially around Khartoum, where the average number is about 24 a year. The name comes from the Arabic word habb, meaning ?wind.? Haboobs are most frequent from May through September, especially in June, but they have occurred in every month except November. Their average duration is three hours; they are most severe in April and May when the soil is driest. They may approach from any direction, but most commonly from the north in winter and from the south, southeast, or east in summer. The average maximum wind velocity is over 13 m s-1 (30 mph) and a speed of 28 m s-1 (62 mph) has been recorded. The sand and dust form a dense whirling wall that may be 1000 m (3000 ft) high; it is often preceded by isolated dust whirls. During these storms, enormous quantities of sand are deposited. Haboobs usually occur after a few days of rising temperature and falling pressure."@en .


###  http://sweetontology.net/phenAtmoWindMesoscale/IbeWind
:IbeWind rdf:type owl:Class ;
         rdfs:subClassOf :Foehn ;
         rdfs:comment "A local strong wind that blows through the Dzungarian Gate (in western China), a gap in the mountain ridge separating the depression of Lakes Balkash and Ala Kul from that of Lake Ebi Nor. The wind resembles the foehn and brings a sudden rise of temperature, in winter from about -26? to about -1?C."@en .


###  http://sweetontology.net/phenAtmoWindMesoscale/InlandSeaBreeze
:InlandSeaBreeze rdf:type owl:Class ;
                 rdfs:subClassOf :SeaBreeze ;
                 rdfs:comment "A circulation similar to a sea breeze, except not at a shore. The inland sea breeze is a very weak thermal circulation caused by temperature contrast between different land surfaces and is sometimes observed between cool irrigated farm land and neighboring dry desert land. This phenomenon is observed only when the synoptic-scale winds are very light."@en .


###  http://sweetontology.net/phenAtmoWindMesoscale/Kachchan
:Kachchan rdf:type owl:Class ;
          rdfs:subClassOf :Foehn ;
          rdfs:comment "A hot, dry, west or southwest wind of foehn type in the lee of the Sri Lanka hills during the southwest monsoon in June and July."@en .


###  http://sweetontology.net/phenAtmoWindMesoscale/KalBaisakhi
:KalBaisakhi rdf:type owl:Class ;
             rdfs:subClassOf :Squall ,
                             [ rdf:type owl:Restriction ;
                               owl:onProperty <http://sweetontology.net/rela/hasPhenomena> ;
                               owl:allValuesFrom <http://sweetontology.net/phenAtmoPrecipitation/Monsoon>
                             ] ;
             rdfs:comment "In India, a short-lived dusty squall at the onset of the southwest monsoon (April? June) in Bengal."@en .


###  http://sweetontology.net/phenAtmoWindMesoscale/Karaburan
:Karaburan rdf:type owl:Class ;
           rdfs:subClassOf :MesoscaleWind ;
           rdfs:comment "A violent northeast wind of Central Asia occurring during spring and summer."@en .


###  http://sweetontology.net/phenAtmoWindMesoscale/Karajol
:Karajol rdf:type owl:Class ;
         rdfs:subClassOf :MesoscaleWind ;
         rdfs:comment "On the Bulgarian coast, a west wind that usually follows rain and persists for one to three days."@en .


###  http://sweetontology.net/phenAtmoWindMesoscale/Karema
:Karema rdf:type owl:Class ;
        rdfs:subClassOf :MesoscaleWind ;
        rdfs:comment "A violent east wind on Lake Tanganyika in Africa."@en .


###  http://sweetontology.net/phenAtmoWindMesoscale/Karif
:Karif rdf:type owl:Class ;
       rdfs:subClassOf :MesoscaleWind ;
       rdfs:comment "A strong southwest wind on the southern shore of the Gulf of Aden, especially at Berbera, Somaliland, during the southwest monsoon."@en .


###  http://sweetontology.net/phenAtmoWindMesoscale/KatabaticWind
:KatabaticWind rdf:type owl:Class ;
               rdfs:subClassOf :MountainWind ;
               rdfs:comment "Most widely used in mountain meteorology to denote a downslope flow driven by cooling at the slope surface during periods of light larger-scale winds; the nocturnal component of the along-slope wind systems."@en .


###  http://sweetontology.net/phenAtmoWindMesoscale/Kaus
:Kaus rdf:type owl:Class ;
      rdfs:subClassOf :MesoscaleWind ;
      rdfs:comment "A moderate to gale-force southeasterly wind in the Persian Gulf; it is accompanied by gloomy weather, rain, and squalls."@en .


###  http://sweetontology.net/phenAtmoWindMesoscale/Khamsin
:Khamsin rdf:type owl:Class ;
         rdfs:subClassOf :DesertWind ;
         rdfs:comment "(Also spelled camsin, chamsin, kamsin, khamasseen, khemsin.) A dry, dusty, and generally hot desert wind in Egypt and over the Red Sea. It is generally southerly or southeasterly, occurring in front of depressions moving eastward across North Africa or the southeastern Mediterranean. The deep khamsins occur in spring with depressions traveling east-northeast across the northern Sahara. They are preceded by a heat wave lasting about three days and are followed by a duststorm. The passage of the depression is marked by a cold front bringing Mediterranean air and a sudden drop in temperature. See ghibli, chili, sirocco."@en .


###  http://sweetontology.net/phenAtmoWindMesoscale/KloofWind
:KloofWind rdf:type owl:Class ;
           rdfs:subClassOf :MesoscaleWind ;
           rdfs:comment "A cold southwest wind of Simons Bay, South Africa."@en .


###  http://sweetontology.net/phenAtmoWindMesoscale/KnikWind
:KnikWind rdf:type owl:Class ;
          rdfs:subClassOf :MesoscaleWind ;
          rdfs:comment "Local name for a strong southeast wind in the vicinity of Palmer in the Matanuska Valley of Alaska. The knik wind blows most frequently in the winter, although it may occur at any time of year. In winter the knik winds are accompanied by very pronounced temperature rises; cases of more than 10?C in 24 hours have been observed. These winds may last from one to ten days. They result from a pressure gradient normal to the Chugach Mountains, causing a pronounced foehn effect in the Matanuska Valley."@en .


###  http://sweetontology.net/phenAtmoWindMesoscale/Koembang
:Koembang rdf:type owl:Class ;
          rdfs:subClassOf :MesoscaleWind ;
          rdfs:comment "A dry foehnlike wind from southeast or south in Cheribon and Tegal in Indonesia. It is caused by the east monsoon that develops a jet effect in passing through the gaps in the mountain ranges and descends on the leeward side."@en .


###  http://sweetontology.net/phenAtmoWindMesoscale/Kona
:Kona rdf:type owl:Class ;
      rdfs:subClassOf :MesoscaleWind ;
      rdfs:comment "A stormy, rain-bringing wind from the southwest or south-southwest in Hawaii. It blows about five times a year on the southwest slopes that are in the lee of the prevailing northeast trade winds. Kona is the Polynesian word for ?leeward.? It is associated with a southward or a southeastward swing of the Aleutian low and the passage of a secondary depression (kona cyclone) from northwest to southeast, north of the islands."@en .


###  http://sweetontology.net/phenAtmoWindMesoscale/Kossava
:Kossava rdf:type owl:Class ;
         rdfs:subClassOf :Squall ;
         rdfs:comment "(Also spelled kosava, koschawa.) A cold, very squally wind, descending from the east or southeast in the region of the Danube ?Iron Gate? through the Carpathians, continuing westward over Belgrade, thence spreading northward to the Rumanian and Hungarian borderlands and southward as far as Nish. In winter it brings temperatures down to below -29C and it is cool even in summer, when it is also dusty. It usually occurs with a depression over the Adriatic and high pressure over southern Russia, a frequent situation in winter. It is usually explained as a jet-effect wind through the Iron Gate, giving speeds well above the gradient wind, but it can be regarded as a katabatic wind intermediate between foehn and bora. The kossava has a marked diurnal variation, with its maximum occurring between 5 AM and 10 AM."@en .


###  http://sweetontology.net/phenAtmoWindMesoscale/KrakatoaWind
:KrakatoaWind rdf:type owl:Class ;
              rdfs:subClassOf :MesoscaleWind ;
              rdfs:comment "(Also spelled Krakatau; formerly called overtrades.) A layer of easterly winds over the Tropics at an altitude of about 18-24 km. This layer tops the midtropospheric westerlies (the antitrades), is at least 6 km deep, and is based at about 2 km above the tropopause. This easterly current is more prominent and better defined in the summer hemisphere. It derives its name from the observed behavior of the volcanic dust carried around the world after the great eruption of Krakatoa (6?S, 105?E) in 1883."@en .


###  http://sweetontology.net/phenAtmoWindMesoscale/Labbe
:Labbe rdf:type owl:Class ;
       rdfs:subClassOf :MesoscaleWind ;
       rdfs:comment "A moderate to strong southwest wind in Provence (southeastern France), mild, humid, and very cloudy or rainy. On the coast it raises a rough sea. It is not frequent, occurring only in March. In the Swiss? French Alps it is locally termed labech, and is squally with thunder, hail, and brief torrential downpours; it comes mainly in autumn and winter."@en .


###  http://sweetontology.net/phenAtmoWindMesoscale/Laheimar
:Laheimar rdf:type owl:Class ;
          rdfs:subClassOf :Squall ;
          rdfs:comment "Severe squalls during the change of seasons in October and November in Arabia."@en .


###  http://sweetontology.net/phenAtmoWindMesoscale/LakeBreeze
:LakeBreeze rdf:type owl:Class ;
            rdfs:subClassOf :MesoscaleWind ,
                            [ rdf:type owl:Restriction ;
                              owl:onProperty <http://sweetontology.net/relaSpace/originatesFrom> ;
                              owl:allValuesFrom <http://sweetontology.net/realmHydroBody/Lake>
                            ] ;
            rdfs:comment "A wind, similar in origin to the sea breeze but generally weaker, blowing from the surface of a large lake onto the shores during the afternoon; it is caused by the difference in surface temperature of land and water as in the land and sea breeze system. In addition to area, the depth of the lake is an important factor; a shallow lake warms up rapidly and is less effective as the source of a lake breeze in summer than is a deep lake. Lake breezes are well developed around the Great Lakes of North America, where they temper the summer heat."@en .


###  http://sweetontology.net/phenAtmoWindMesoscale/LandBreeze
:LandBreeze rdf:type owl:Class ;
            rdfs:subClassOf :OffshoreWind ;
            rdfs:comment "A coastal breeze blowing from land to sea, caused by the temperature difference when the sea surface is warmer than the adjacent land. Therefore, it usually blows by night and alternates with sea breeze, which blows in the opposite direction by day. See puelche, karif."@en .


###  http://sweetontology.net/phenAtmoWindMesoscale/Leste
:Leste rdf:type owl:Class ;
       rdfs:subClassOf :MesoscaleWind ;
       rdfs:comment "Spanish nautical term for east wind. The name is given to a hot, dry, dusty easterly, or southeasterly wind that blows from the Atlantic coast of Morocco out to Madeira and the Canary Islands. It is a form of sirocco and occurs in front of depressions advancing eastward. Compare levanto."@en .


###  http://sweetontology.net/phenAtmoWindMesoscale/Levante
:Levante rdf:type owl:Class ;
         rdfs:subClassOf :MesoscaleWind ;
         rdfs:comment "The Spanish and most widely used term for an east or northeast wind occurring along the coast and inland from southern France to the Straits of Gibraltar. It is moderate or fresh (not as strong as the gregale), mild, very humid, overcast, and rainy; it occurs with a depression over the western Mediterranean Sea. In summer it is rare and weak; in January it is inhibited by the Iberian anticyclone. It is most frequent from February to May and October to December. A levant (French spelling) with fine weather is a levant blanc; in the Roussillon region of southern France (where, as along the Catalonian coast of Spain, it is called llevant) it often brings floods in the mountain streams. The levanter of the Gibraltar Straits is a related phenomenon. Compare leste, lombarde, levantera."@en .


###  http://sweetontology.net/phenAtmoWindMesoscale/Levantera
:Levantera rdf:type owl:Class ;
           rdfs:subClassOf :MesoscaleWind ;
           rdfs:comment "A persistent east wind in the Adriatic, usually bringing cloudy weather."@en .


###  http://sweetontology.net/phenAtmoWindMesoscale/Leveche
:Leveche rdf:type owl:Class ;
         rdfs:subClassOf :MesoscaleWind ,
                         [ rdf:type owl:Restriction ;
                           owl:onProperty <http://sweetontology.net/rela/hasProcess> ;
                           owl:allValuesFrom <http://sweetontology.net/procPhysical/Heating>
                         ] ;
         rdfs:comment "A hot, sand- and dust-laden wind from between southeast and southwest that blows in front of a depression on the southeast coast of Spain but extends only a few miles inland."@en .


###  http://sweetontology.net/phenAtmoWindMesoscale/Libeccio
:Libeccio rdf:type owl:Class ;
          rdfs:subClassOf :MesoscaleWind ;
          rdfs:comment "Italian name for a southwest wind; used especially in northern Corsica for the west or southwest wind that blows throughout the year, and especially in winter when it is often stormy. On windward slopes it brings rain, with thunderstorms in summer and autumn. After crossing the mountains it is warm and dry, but may be very turbulent."@en .


###  http://sweetontology.net/phenAtmoWindMesoscale/Liberator
:Liberator rdf:type owl:Class ;
           rdfs:subClassOf :MesoscaleWind ;
           rdfs:comment "A name sometimes given the west wind through the Straits of Gibraltar."@en .


###  http://sweetontology.net/phenAtmoWindMesoscale/LineSquall
:LineSquall rdf:type owl:Class ;
            rdfs:subClassOf :Squall ;
            rdfs:comment "A squall that occurs along a squall line. This term is now confined mostly to nautical usage."@en .


###  http://sweetontology.net/phenAtmoWindMesoscale/Lombarde
:Lombarde rdf:type owl:Class ;
          rdfs:subClassOf :MountainWind ;
          rdfs:comment "An easterly wind (from Lombardy) that predominates along the French?Italian frontier. It comes from the High Alps. In winter it is violent and forms snowdrifts in the mountain valleys. In the plains it is gentle and very dry. It is associated with an anticyclone over France and central Europe, or with high pressure to the southeast of Europe and low pressure to the northwest along with falling pressure over western France."@en .


###  http://sweetontology.net/phenAtmoWindMesoscale/LongShoreWind
:LongShoreWind rdf:type owl:Class ;
               rdfs:subClassOf :MesoscaleWind ;
               rdfs:comment "1. A damp unpleasant wind that blows from the south in Madras (India). 2. A wind from the northeast at night in Sri Lanka."@en .


###  http://sweetontology.net/phenAtmoWindMesoscale/MackerelBreeze
:MackerelBreeze rdf:type owl:Class ;
                owl:equivalentClass :MackerelGale ;
                rdfs:subClassOf :OceanWind ;
                rdfs:comment "(Also called mackerel gale.) A wind that ruffles the water, favoring the catching of mackerel."@en .


###  http://sweetontology.net/phenAtmoWindMesoscale/MackerelGale
:MackerelGale rdf:type owl:Class ;
              rdfs:comment "Same as a mackerel breeze"@en .


###  http://sweetontology.net/phenAtmoWindMesoscale/Maestro
:Maestro rdf:type owl:Class ;
         rdfs:subClassOf :MesoscaleWind ;
         rdfs:comment "A northwesterly wind with fine weather that blows, especially in summer, in the Adriatic; it is most frequent on the western shore and is equivalent to the etesians of the eastern Mediterranean. It is also found on the coasts of Corsica and Sardinia. Compare mistral." ;
         rdfs:label "Maestro" .


###  http://sweetontology.net/phenAtmoWindMesoscale/MajolaWind
:MajolaWind rdf:type owl:Class ;
            rdfs:subClassOf :MountainWind ;
            rdfs:comment "A wind, named after the Maloja Pass between the Engadine and Bergall, Switzerland, that blows down the valley of the Upper Engadine by day and either up or down by night. This deviation from the usual nature of mountain and valley winds is attributed to the fact that the stronger daytime valley wind from the south overtops the ridge and continues down the Engadine."@en .


###  http://sweetontology.net/phenAtmoWindMesoscale/MalojaWind
:MalojaWind rdf:type owl:Class ;
            rdfs:subClassOf :MesoscaleWind ;
            rdfs:comment "A northwesterly wind with fine weather that blows, especially in summer, in the Adriatic; it is most frequent on the western shore and is equivalent to the etesians of the eastern Mediterranean. It is also found on the coasts of Corsica and Sardinia. Compare mistral."@en .


###  http://sweetontology.net/phenAtmoWindMesoscale/Mamatele
:Mamatele rdf:type owl:Class ;
          rdfs:subClassOf :MesoscaleWind ;
          rdfs:comment "(Also called mamaliti, mamatili.) A light northwest wind of Sicily; a form of mistral."@en .


###  http://sweetontology.net/phenAtmoWindMesoscale/Marin
:Marin rdf:type owl:Class ;
       rdfs:subClassOf :MesoscaleWind ;
       rdfs:comment "A warm moist southeast wind from the sea on the French Mediterranean coast and in the Maritime Alps, especially frequent in spring and autumn. In the Rh?ne delta it blows also from the south. The marin is associated with depressions that cross southern France or northern Spain and the Gulf of Lions. Generally, it is strong and regular, sometimes violent and turbulent in hilly country as the ayalas in the Massif Central; it is very humid, cloudy with hill fog, and often rainy (unless unaccompanied by fronts, when it is the marin blanc). The heavy rains, which may continue for one or two days on the mountain slopes, cause dangerous river floods. On the western slope of the C?vennes it becomes the autan. In the southern C?vennes the marin is called the aygalas. On the coast of Catalonia (northeast Spain) and Roussillon (southern France) it is the marinada and generally occurs with a depression centered over or south of the Gulf of Gascony. Compare sirocco."@en .


###  http://sweetontology.net/phenAtmoWindMesoscale/MatanuskaWind
:MatanuskaWind rdf:type owl:Class ;
               rdfs:subClassOf :MesoscaleWind ;
               rdfs:comment "The local name, taken from the Matanuska River, for a strong, gusty, northeast wind that occasionally occurs during the winter in the vicinity of Palmer, Alaska."@en .


###  http://sweetontology.net/phenAtmoWindMesoscale/Matinal
:Matinal rdf:type owl:Class ;
         rdfs:subClassOf :MesoscaleWind ;
         rdfs:comment "The morning wind, that is, an east wind. In the Morvan Mountains and the center of the Massif Central in France, the matinal often blows for several days, especially in summer, and brings fine weather. On winter mornings a northeast or east wind descends the western slopes of the Alps (where it is known as the matini?re) bringing cold and generally fine weather. Compare solaire."@en .


###  http://sweetontology.net/phenAtmoWindMesoscale/Meltem
:Meltem rdf:type owl:Class ;
        rdfs:subClassOf :MesoscaleWind ;
        rdfs:comment "1. (Also spelled melt?mi.) A strong wind from the northeast or east that often sets in suddenly and blows during the day in summer on the Bulgarian coast and in the Bosporus. 2. Same as monsoon."@en .


###  http://sweetontology.net/phenAtmoWindMesoscale/Mergozzo
:Mergozzo rdf:type owl:Class ;
          rdfs:subClassOf :MesoscaleWind ;
          rdfs:comment "Northwest wind on Lake Maggiore, Italy."@en .


###  http://sweetontology.net/phenAtmoWindMesoscale/Mesojet
:Mesojet rdf:type owl:Class ;
         rdfs:subClassOf :MesoscaleWind ;
         rdfs:comment "A mesoscale wind maximum. It typically may have an along-flow length scale of tens to hundreds of kilometers and a cross- flow length scale of 100 km. Mesojets differ from planetary-scale jets, which can have length scales of several thousand kilometers, and synoptic-scale jets, which may have length scales of 1000? 2000 km and are commonly found in association with progressive synoptic-scale troughs and ridges. Larger mesojets may also sometimes be known as jet streaks. Mesojets can form adjacent to prominent orographic features in association with terrain-channeled flow. Mesojets are also seen in association with organized mesocale convective systems as typified by the evaporatively driven rear-inflow jet commonly found behind active squall lines lines. Mesojets may also be found in conjunction with prominent lower-tropospheric stable layers where the airflow can become decoupled from the planetary boundary layer, especially at night. An exceptionally well organized lower-tropospheric mesojet extending over hundreds of kilometers might be known as a low-level jet."@en .


###  http://sweetontology.net/phenAtmoWindMesoscale/MesoscaleWind
:MesoscaleWind rdf:type owl:Class ;
               rdfs:subClassOf <http://sweetontology.net/phenAtmoWind/Wind> .


###  http://sweetontology.net/phenAtmoWindMesoscale/Miejour
:Miejour rdf:type owl:Class ;
         rdfs:subClassOf :SeaBreeze ;
         rdfs:comment "A warm, moist sea breeze from the south that sets in at midday in Provence, France, south of Mount Ventoux. In the Roussillon region the midday south wind (mitgjorn) is irregular and generally light, and is dry after crossing the Pyrenees."@en .


###  http://sweetontology.net/phenAtmoWindMesoscale/MoazagotlWind
:MoazagotlWind rdf:type owl:Class ;
               rdfs:subClassOf :MountainWind ;
               rdfs:comment "The strong wind blowing across a mountain crest, responsible for the formation of the Moazagotl cloud."@en .


###  http://sweetontology.net/phenAtmoWindMesoscale/Molan
:Molan rdf:type owl:Class ;
       rdfs:subClassOf :MesoscaleWind ;
       rdfs:comment "Breeze blowing from Arve toward Geneva in Switzerland."@en .


###  http://sweetontology.net/phenAtmoWindMesoscale/MonsoonSurge
:MonsoonSurge rdf:type owl:Class ;
              rdfs:subClassOf :MountainWind ;
              rdfs:comment "The temporary extension of deep monsoon flow into a region not normally dominated by persistent monsoon flow. This temporary extension or surge may last from a few days to three weeks. These surges most commonly occur eastward across the Philippine Sea into the western North Pacific and east of Australia into the western South Pacific. The establishment of a reverse-oriented monsoon trough is accompanied by an eastward surge in the monsoon flow. Monsoon surges are often precursors to the development of tropical cyclones."@en .


###  http://sweetontology.net/phenAtmoWindMesoscale/Morget
:Morget rdf:type owl:Class ;
        rdfs:subClassOf :LandBreeze ;
        rdfs:comment "The night land breeze on Lake Geneva, Switzerland.  It blows from the north from 5-7 P.M. until 7-9 A.M. as a poweful breeze.  In the late fall and winter it blows almost throughout the day."@en .


###  http://sweetontology.net/phenAtmoWindMesoscale/MountainBreeze
:MountainBreeze rdf:type owl:Class ;
                rdfs:subClassOf :MountainWind ;
                rdfs:comment "A nocturnal component of the mountain?plains or mountain?valley wind systems encountered during periods of light synoptic flow."@en .


###  http://sweetontology.net/phenAtmoWindMesoscale/MountainGapWind
:MountainGapWind rdf:type owl:Class ;
                 rdfs:subClassOf :MountainWind ;
                 rdfs:comment "A local wind blowing through a gap between mountains, a gap wind. This term was introduced by R. S. Scorer (1952) for the surface winds blowing through the Strait of Gibraltar. When air stratification is stable, as it usually is in summer, the air tends to flow through the gap from high to low pressure, emerging as a ?jet? with large standing eddies in the lee of the gap. The excess of pressure on the upwind side is attributed to a pool of cold air held up by the mountains. Similar winds occur at other gaps in mountain ranges, such as the tehuantepecer and the jochwinde, and in long channels, such as the Strait of Juan de Fuca between the Olympic Mountains of Washington and Vancouver Island, British Columbia. Compare jet-effect wind, canyon wind, mountain wind."@en .


###  http://sweetontology.net/phenAtmoWindMesoscale/MountainPlainWind
:MountainPlainWind rdf:type owl:Class ;
                   rdfs:subClassOf :MountainWind ;
                   rdfs:comment "The diurnal cycle of local winds between a mountain or a mountain range and the adjacent or surrounding plains during periods of weak synoptic flow."@en .


###  http://sweetontology.net/phenAtmoWindMesoscale/MountainValleyWind
:MountainValleyWind rdf:type owl:Class ;
                    rdfs:subClassOf :MountainWind ;
                    rdfs:comment "The diurnal cycle of local winds in a mountain valley during clear or mostly clear periods of weak synoptic flow."@en .


###  http://sweetontology.net/phenAtmoWindMesoscale/MountainWind
:MountainWind rdf:type owl:Class ;
              rdfs:subClassOf :MesoscaleWind ,
                              [ rdf:type owl:Restriction ;
                                owl:onProperty <http://sweetontology.net/rela/hasRealm> ;
                                owl:allValuesFrom <http://sweetontology.net/realmLandOrographic/Mountain>
                              ] ;
              rdfs:comment "A nocturnal, thermally forced wind from the direction of the mountains, generated by cooling along the mountain slopes; a downvalley wind, or the nighttime downslope (katabatic) component of a mountain?plains wind system."@en .


###  http://sweetontology.net/phenAtmoWindMesoscale/N_aschi
:N_aschi rdf:type owl:Class ;
         rdfs:subClassOf :MesoscaleWind ;
         rdfs:comment "The Arabic name for a northeasterly wind that ocurrs in winter on the Iranian coast of the Persian Gulf, especially near the entrance to the gulf and also on the Makran coast."@en .


###  http://sweetontology.net/phenAtmoWindMesoscale/Narbonnais
:Narbonnais rdf:type owl:Class ;
            rdfs:subClassOf :MesoscaleWind ;
            rdfs:comment "(Also spelled narbon?.) In France, a wind coming from Narbonne; a north wind in the Roussillon region of southern France resembling the tramontana. If associated with an influx of arctic air, it may be very stormy with heavy falls of rain or snow. It is especially violent in the region of Perpignan where it blows in a succession of squalls for several days. In Provence it is rarer and blows from the west. In lower Languedoc and the southern C?vennes, the narbonnais is an infrequent, mild, moist, moderate southwest wind in winter and early spring, sometimes bringing thunderstorms."@en .


###  http://sweetontology.net/phenAtmoWindMesoscale/NightWind
:NightWind rdf:type owl:Class ;
           rdfs:subClassOf :MesoscaleWind ;
           rdfs:comment "Dry squalls that occur at night in southwest Africa and the Congo. It is likely that this term is loosely applied to other diurnal local winds such as mountain wind, land breeze, midnight wind, etc."@en .


###  http://sweetontology.net/phenAtmoWindMesoscale/Nortada
:Nortada rdf:type owl:Class ;
         rdfs:subClassOf :MesoscaleWind ;
         rdfs:comment "A strong, persistent northerly wind in the Philippines."@en .


###  http://sweetontology.net/phenAtmoWindMesoscale/Norte
:Norte rdf:type owl:Class ;
       rdfs:subClassOf :MesoscaleWind .


###  http://sweetontology.net/phenAtmoWindMesoscale/NorthFoehn
:NorthFoehn rdf:type owl:Class ;
            rdfs:subClassOf :Foehn ;
            rdfs:comment "A northerly foehn wind blowing down the Italian side of the Alps. The northern slopes are normally cooler than the southern slopes, and the dynamic warming is often insufficient to overcome the difference of temperature. Hence a warm dry northerly wind of foehnlike character occurs less frequently than the south foehn."@en .


###  http://sweetontology.net/phenAtmoWindMesoscale/Northeaster
:Northeaster rdf:type owl:Class ;
             rdfs:subClassOf :MesoscaleWind ;
             rdfs:comment "A northeast wind, particularly a strong wind or gale."@en .


###  http://sweetontology.net/phenAtmoWindMesoscale/Norther
:Norther rdf:type owl:Class ;
         rdfs:subClassOf :MesoscaleWind ;
         rdfs:comment "A northerly wind; in general, a cold windstorm from the north."@en .


###  http://sweetontology.net/phenAtmoWindMesoscale/Northwester
:Northwester rdf:type owl:Class ;
             rdfs:subClassOf :MesoscaleWind ;
             rdfs:comment "(Often contracted nor'wester.) A northwesterly wind (as Canterbury northwester)."@en .


###  http://sweetontology.net/phenAtmoWindMesoscale/OceanWind
:OceanWind rdf:type owl:Class ;
           rdfs:subClassOf :MesoscaleWind ,
                           [ rdf:type owl:Restriction ;
                             owl:onProperty <http://sweetontology.net/rela/hasRealm> ;
                             owl:allValuesFrom <http://sweetontology.net/realm/Ocean>
                           ] .


###  http://sweetontology.net/phenAtmoWindMesoscale/OffshoreWind
:OffshoreWind rdf:type owl:Class ;
              rdfs:subClassOf :MesoscaleWind ,
                              [ rdf:type owl:Restriction ;
                                owl:onProperty <http://sweetontology.net/relaSpace/originatesFrom> ;
                                owl:allValuesFrom <http://sweetontology.net/realm/Land>
                              ] ;
              rdfs:comment "Wind blowing from land to sea.  During synoptic conditions of light winds, offshore winds near the surface often occur at night as a component of the land breeze."@en .


###  http://sweetontology.net/phenAtmoWindMesoscale/OnshoreWind
:OnshoreWind rdf:type owl:Class ;
             rdfs:subClassOf :MesoscaleWind ,
                             [ rdf:type owl:Restriction ;
                               owl:onProperty <http://sweetontology.net/relaSpace/originatesFrom> ;
                               owl:allValuesFrom <http://sweetontology.net/realm/Ocean>
                             ] ;
             rdfs:comment "A wind blowing from water onto land; the wind may be a result of heating differences between land and water or related to synoptic weather patterns."@en .


###  http://sweetontology.net/phenAtmoWindMesoscale/OutflowJet
:OutflowJet rdf:type owl:Class ;
            rdfs:subClassOf :MesoscaleWind ,
                            [ rdf:type owl:Restriction ;
                              owl:onProperty <http://sweetontology.net/rela/hasRealm> ;
                              owl:someValuesFrom <http://sweetontology.net/realmLandFluvial/Canyon>
                            ] ,
                            [ rdf:type owl:Restriction ;
                              owl:onProperty <http://sweetontology.net/rela/hasRealm> ;
                              owl:someValuesFrom <http://sweetontology.net/realmLandFluvial/Valley>
                            ] ;
            rdfs:comment "Nocturnal cold-air jet flowing out of the mouth of a valley or canyon as it opens onto a plain."@en .


###  http://sweetontology.net/phenAtmoWindMesoscale/PlowWind
:PlowWind rdf:type owl:Class ;
          rdfs:subClassOf :MesoscaleWind ,
                          [ rdf:type owl:Restriction ;
                            owl:onProperty <http://sweetontology.net/rela/hasPhenomena> ;
                            owl:allValuesFrom <http://sweetontology.net/phenAtmoPrecipitation/Thunderstorm>
                          ] ;
          rdfs:comment "Strong straight-line winds associated with nontornadic outflow from strong thunderstorms."@en .


###  http://sweetontology.net/phenAtmoWindMesoscale/SeaBreeze
:SeaBreeze rdf:type owl:Class ;
           rdfs:subClassOf :OnshoreWind ;
           rdfs:comment "A coastal local wind that blows from sea to land, caused by the temperature difference when the sea surface is colder than the adjacent land."@en .


###  http://sweetontology.net/phenAtmoWindMesoscale/Squall
:Squall rdf:type owl:Class ;
        rdfs:subClassOf :MountainWind ;
        rdfs:comment "A strong wind characterized by a sudden onset, a duration of the order of minutes, and then a rather sudden decrease in speed."@en .


###  http://sweetontology.net/phenAtmoWindMesoscale/ThunderstormOutflow
:ThunderstormOutflow rdf:type owl:Class ;
                     rdfs:subClassOf :MesoscaleWind ,
                                     [ rdf:type owl:Restriction ;
                                       owl:onProperty <http://sweetontology.net/rela/hasPhenomena> ;
                                       owl:allValuesFrom <http://sweetontology.net/phenAtmoPrecipitation/Thunderstorm>
                                     ] ;
                     rdfs:comment "The relatively cool pool of air that results when a thunderstorm downdraft reaches the earth's surface and spreads horizontally as a density current."@en .


###  http://sweetontology.net/phenAtmoWindMesoscale/UpslopeWind
:UpslopeWind rdf:type owl:Class ;
             rdfs:subClassOf :MountainWind ,
                             [ rdf:type owl:Restriction ;
                               owl:onProperty <http://sweetontology.net/relaSpace/hasDirection> ;
                               owl:hasValue <http://sweetontology.net/reprSpaceDirection/Upslope>
                             ] ;
             rdfs:comment "A wind directed up a slope, often used to describe winds produced by processes larger in scale than the slope."@en .


###  http://sweetontology.net/phenAtmoWindMesoscale/ValleyWind
:ValleyWind rdf:type owl:Class ;
            rdfs:subClassOf :MesoscaleWind ,
                            [ rdf:type owl:Restriction ;
                              owl:onProperty <http://sweetontology.net/rela/hasRealm> ;
                              owl:allValuesFrom <http://sweetontology.net/realmLandFluvial/Valley>
                            ] ;
            rdfs:comment "A wind that ascends a mountain valley (upvalley wind) during the day; the daytime component of a mountain?valley wind system."@en .


###  http://sweetontology.net/phenAtmoWindMesoscale/YellowWind
:YellowWind rdf:type owl:Class ;
            rdfs:subClassOf :DesertWind ;
            rdfs:comment "A strong, cold, dry, west wind of eastern Asia, especially northern China, that sweeps across the plains in winter carrying a fine yellow dust from the deserts."@en .


###  http://sweetontology.net/phenAtmoWindMesoscale/Zephyr
:Zephyr rdf:type owl:Class ;
        rdfs:subClassOf :MesoscaleWind ;
        rdfs:comment "Any soft, gentle breeze."@en .


###  http://sweetontology.net/phenFluidDynamics/Vortex
<http://sweetontology.net/phenFluidDynamics/Vortex> rdf:type owl:Class .


###  http://sweetontology.net/procPhysical/Cooling
<http://sweetontology.net/procPhysical/Cooling> rdf:type owl:Class .


###  http://sweetontology.net/procPhysical/Gravity
<http://sweetontology.net/procPhysical/Gravity> rdf:type owl:Class .


###  http://sweetontology.net/procPhysical/Heating
<http://sweetontology.net/procPhysical/Heating> rdf:type owl:Class .


###  http://sweetontology.net/realm/Land
<http://sweetontology.net/realm/Land> rdf:type owl:Class .


###  http://sweetontology.net/realm/Ocean
<http://sweetontology.net/realm/Ocean> rdf:type owl:Class .


###  http://sweetontology.net/realmCryo/Glacier
<http://sweetontology.net/realmCryo/Glacier> rdf:type owl:Class .


###  http://sweetontology.net/realmHydroBody/Lake
<http://sweetontology.net/realmHydroBody/Lake> rdf:type owl:Class .


###  http://sweetontology.net/realmLandAeolian/Desert
<http://sweetontology.net/realmLandAeolian/Desert> rdf:type owl:Class .


###  http://sweetontology.net/realmLandFluvial/Canyon
<http://sweetontology.net/realmLandFluvial/Canyon> rdf:type owl:Class .


###  http://sweetontology.net/realmLandFluvial/Gorge
<http://sweetontology.net/realmLandFluvial/Gorge> rdf:type owl:Class .


###  http://sweetontology.net/realmLandFluvial/Valley
<http://sweetontology.net/realmLandFluvial/Valley> rdf:type owl:Class .


###  http://sweetontology.net/realmLandOrographic/Mountain
<http://sweetontology.net/realmLandOrographic/Mountain> rdf:type owl:Class .


#################################################################
#    Individuals
#################################################################

###  http://sweetontology.net/reprSpaceDirection/Upslope
<http://sweetontology.net/reprSpaceDirection/Upslope> rdf:type owl:NamedIndividual .


###  Generated by the OWL API (version 5.1.2.2017-10-13T07:13:07Z) https://github.com/owlcs/owlapi/
