@base          <http://sweetontology.net/phenAtmoWind> .
@prefix crela: <http://sweetontology.net/relaChemical/> .
@prefix pres:  <http://sweetontology.net/propPressure/> .
@prefix owl:   <http://www.w3.org/2002/07/owl#> .
@prefix xsd:   <http://www.w3.org/2001/XMLSchema#> .
@prefix aphen: <http://sweetontology.net/phenAtmo/> .
@prefix rdfs:  <http://www.w3.org/2000/01/rdf-schema#> .
@prefix pol:   <http://sweetontology.net/matrAerosol/> .
@prefix dir:   <http://sweetontology.net/propSpaceDirection/> .
@prefix sed:   <http://sweetontology.net/matrSediment/> .
@prefix rdf:   <http://www.w3.org/1999/02/22-rdf-syntax-ns#> .
@prefix pproc: <http://sweetontology.net/procPhysical/> .
@prefix fluid: <http://sweetontology.net/phenFluidDynamics/> .
@prefix rela:  <http://sweetontology.net/rela/> .
@prefix screla: <http://sweetontology.net/relaSci/> .
@prefix wind:  <http://sweetontology.net/phenAtmoWind/> .

wind:SandStorm  a        owl:Class ;
        rdfs:subClassOf  wind:Wind ;
        rdfs:subClassOf  [ a                  owl:Restriction ;
                           owl:allValuesFrom  sed:Sand ;
                           owl:onProperty     crela:hasSubstance
                         ] .

wind:Windborne  a        owl:Class ;
        rdfs:subClassOf  aphen:MeteorologicalPhenomena .

wind:HotWind  a          owl:Class ;
        rdfs:comment     "General term for winds characterized by intense heat and low relative humidity, such as summertime desert winds or an extreme foehn."@en ;
        rdfs:subClassOf  wind:Wind ;
        rdfs:subClassOf  [ a                  owl:Restriction ;
                           owl:allValuesFrom  pproc:Heating ;
                           owl:onProperty     rela:hasPhenomena
                         ] .

wind:WarmConveyorBelt
        a                owl:Class ;
        rdfs:subClassOf  wind:GlobalWindCirculation .

wind:ZonalWind  a        owl:Class ;
        rdfs:subClassOf  wind:GlobalWindCirculation ;
        rdfs:subClassOf  [ a                  owl:Restriction ;
                           owl:allValuesFrom  wind:ZonalFlow ;
                           owl:onProperty     rela:hasPhenomena
                         ] .

wind:WindGust  a         owl:Class ;
        rdfs:subClassOf  wind:Wind .

wind:JetEffectWind  a    owl:Class ;
        rdfs:comment     "A local wind created by acceleration of the airflow through a gap, constriction, or channel in a mountain range or between ranges."@en ;
        rdfs:subClassOf  wind:Wind .

wind:Wind  a             owl:Class ;
        rdfs:subClassOf  aphen:MeteorologicalPhenomena ;
        rdfs:subClassOf  [ a                  owl:Restriction ;
                           owl:allValuesFrom  pres:PressureGradient ;
                           owl:onProperty     screla:hasCause
                         ] .

wind:ThermalWind  a      owl:Class ;
        rdfs:comment     "The mean wind-shear vector in geostrophic balance with the gradient of mean temperature of a layer bounded by two isobaric surfaces."@en ;
        rdfs:subClassOf  wind:Wind .

wind:GlobalWindCirculation
        a                owl:Class ;
        rdfs:subClassOf  wind:AtmosphericCirculation .

wind:LocalWind  a        owl:Class ;
        rdfs:comment     "1. Winds that, over a small area, differ from those that would be appropriate to the general large-scale pressure distribution, or that possess some other peculiarity. Often these winds have names unique to the area where they occur. Local winds may be classified into three main groups. The first includes diurnally varying airflows that are driven by local gradients of surface heat flux (e.g., near the shore of a sea or lake) or by diurnal heating or cooling of the ground surface in areas of sloping or mountainous terrain. These include land and sea breezes, mountain?valley circulations, and drainage and slope winds. The second group consists of winds produced by the interaction of a synoptic-scale flow with orography. These may be further subdivided into barrier jets, gap winds, downslope windstorms, and include such local phenomena as the tehuantepecer, Santa Ana, foehn, mistral, and bora. The third group includes those winds accompanying convective activity, more specifically individual thunderstorms or mesoscale convective systems. These are generally the surface manifestations of precipitation- cooled diverging outflow and in some locations are given special names due to the distinctive character of the weather associated with them (e.g., the haboob). 2. Local or colloquial names given to frequently occurring or particularly noteworthy winds (sometimes because of the bad weather associated with them), usually from a certain direction. Often these names reflect the direction from which the wind comes (e.g., sou'wester, nor'easter)."@en ;
        rdfs:subClassOf  wind:Wind .

wind:TertiaryCirculation
        a                owl:Class ;
        rdfs:comment     "The generally small, localized atmospheric circulations."@en ;
        rdfs:subClassOf  wind:AtmosphericCirculation .

wind:JetStreamWind  a  owl:Class .

wind:DustStorm  a        owl:Class ;
        rdfs:subClassOf  wind:LocalWind ;
        rdfs:subClassOf  [ a                  owl:Restriction ;
                           owl:allValuesFrom  pol:Dust ;
                           owl:onProperty     crela:hasSubstance
                         ] .

wind:WalkerCell  a  owl:Class .

wind:Gust  a                 owl:Class ;
        rdfs:comment         "1. A sudden, brief increase in the speed of the wind. It is of a more transient character than a squall and is followed by a lull or slackening in the wind speed. Generally, winds are least gusty over large water surfaces and most gusty over rough land and near high buildings. According to U.S. weather observing practice, gusts are reported when the peak wind speed reaches at least 16 knots and the variation in wind speed between the peaks and lulls is at least 9 knots. The duration of a gust is usually less than 20 s. 2. With respect to aircraft turbulence, a sharp change in wind speed relative to the aircraft; a sudden increase in airspeed due to fluctuations in the airflow, resulting in increased structural stresses upon the aircraft. 3. (Rare.) Same as cloudburst."@en ;
        rdfs:subClassOf      wind:Wind ;
        owl:equivalentClass  wind:WindGust .

wind:MeridionalWind  a   owl:Class ;
        rdfs:comment     "The wind or wind component along the local meridian, as distinguished from the zonal wind. In a horizontal coordinate system fixed locally with the x axis directed eastward and the y axis northward, the meridional wind is positive if from the south, and negative if from the north."@en ;
        rdfs:subClassOf  wind:Wind .

wind:Derecho  a          owl:Class ;
        rdfs:comment     "A widespread convectively induced straight-line windstorm."@en ;
        rdfs:subClassOf  wind:WindStorm .

wind:EasterlyWind  a     owl:Class ;
        rdfs:subClassOf  wind:GlobalWindCirculation .

wind:WindStorm  a        owl:Class ;
        rdfs:subClassOf  wind:Wind .

wind:EulerianWind  a     owl:Class ;
        rdfs:comment     "In the classification of Jeffreys, a wind motion only in response to the pressure force."@en ;
        rdfs:subClassOf  wind:Wind .

wind:JetStream  a            owl:Class ;
        rdfs:comment         "Relatively strong winds concentrated within a narrow stream in the atmosphere."@en ;
        rdfs:subClassOf      aphen:AtmosphericWave , wind:GlobalWindCirculation ;
        owl:equivalentClass  wind:JetStreamWind .

wind:TradeWind  a        owl:Class ;
        rdfs:comment     "The wind system, occupying most of the Tropics, that blows from the subtropical highs toward the equatorial trough; a major component of the general circulation of the atmosphere."@en ;
        rdfs:subClassOf  wind:GlobalWindCirculation ;
        rdfs:subClassOf  [ a                  owl:Restriction ;
                           owl:allValuesFrom  wind:AtmosphericCirculation ;
                           owl:onProperty     rela:hasPhenomena
                         ] .

wind:JetStreamAxis  a    owl:Class ;
        rdfs:comment     "The axis of maximum wind speed in a jet stream."@en ;
        rdfs:subClassOf  dir:Axis ;
        rdfs:subClassOf  [ a                  owl:Restriction ;
                           owl:allValuesFrom  wind:JetStream ;
                           owl:onProperty     rela:hasPhenomena
                         ] .

wind:VeeringWind  a      owl:Class ;
        rdfs:comment     "In the Northern Hemisphere, a wind that rotates in a clockwise direction with increasing height; the opposite of backing wind."@en ;
        rdfs:subClassOf  wind:Wind ;
        rdfs:subClassOf  [ a                  owl:Restriction ;
                           owl:allValuesFrom  pproc:Rotation ;
                           owl:onProperty     rela:hasPhenomena
                         ] .

wind:AtmosphericPumping
        a                owl:Class ;
        rdfs:subClassOf  wind:GlobalWindCirculation .

wind:HadleyCirculation
        a                owl:Class ;
        rdfs:subClassOf  wind:GlobalWindCirculation .

wind:DrainageWind  a     owl:Class ;
        rdfs:subClassOf  wind:Wind .

wind:ZonalFlow  a        owl:Class ;
        rdfs:comment     "In meteorology, the flow of air along a latitude circle; more specifically, the latitudinal (east or west) component of existing flow."@en ;
        rdfs:subClassOf  wind:GlobalWindCirculation .

wind:DustDevil  a        owl:Class ;
        rdfs:subClassOf  wind:DustStorm .

wind:AtmosphericCirculation
        a                owl:Class ;
        rdfs:subClassOf  fluid:Circulation , aphen:MeteorologicalPhenomena .

wind:CrossWind  a        owl:Class ;
        rdfs:subClassOf  wind:Wind .

wind:JetStreak  a        owl:Class ;
        rdfs:comment     "The region of a jet stream axis with the greatest winds."@en ;
        rdfs:subClassOf  wind:JetStream .

wind:WalkerCirculation
        a                    owl:Class ;
        rdfs:comment         "A zonal circulation of the atmosphere confined to equatorial regions and driven principally by the oceanic temperature gradient. In the Pacific, air flows westward from the colder, eastern area to the warm, western ocean, where it acquires warmth and moisture and subsequently rises. A return flow aloft and subsidence over the eastern ocean complete the cell"@en ;
        rdfs:subClassOf      wind:GlobalWindCirculation ;
        owl:equivalentClass  wind:WalkerCell .

wind:Microburst  a       owl:Class ;
        rdfs:subClassOf  wind:Wind .

wind:Blowing  a          owl:Class ;
        rdfs:comment     "When dust, sand, snow, and/or spray is raised by the wind to a height of 6 feet or more" ;
        rdfs:subClassOf  wind:Wind .

<>      a                owl:Ontology ;
        rdfs:label       "SWEET Ontology" ;
        owl:imports      <relaChemical> , <matrSediment> , <propSpaceDirection> , <phenAtmo> , <procPhysical> , <propPressure> , <rela> , <phenFluidDynamics> , <matrAerosol> , <relaSci> ;
        owl:versionInfo  "3.1.0" .

wind:Downdraft  a        owl:Class ;
        rdfs:comment     "Small-scale downward moving air current in a cumulonimbus cloud."@en ;
        rdfs:subClassOf  wind:Wind .

wind:GeostrophicWind  a  owl:Class ;
        rdfs:subClassOf  wind:GlobalWindCirculation .

wind:Tailwind  a         owl:Class ;
        rdfs:comment     "A wind that assists the intended progress of an exposed, moving object, for example, rendering an airborne object's groundspeed greater than its airspeed; the opposite of a headwind."@en ;
        rdfs:subClassOf  wind:Wind .

wind:HeadWind  a         owl:Class ;
        rdfs:comment     "A wind that opposes the intended progress of an exposed, moving object, for example, rendering an airborne object's airspeed greater than its groundspeed; the opposite of a tailwind."@en ;
        rdfs:subClassOf  wind:Wind .

wind:AgeostrophicWind
        a                owl:Class ;
        rdfs:comment     "The vector difference between the real (or observed) wind and the geostrophic wind" ;
        rdfs:label       "Ageostrophic Wind" ;
        rdfs:subClassOf  wind:Wind .
