@base          <http://sweetontology.net/phenWave> .
@prefix sysc:  <http://sweetontology.net/phenSystemComplexity/> .
@prefix proc:  <http://sweetontology.net/procPhysical/> .
@prefix owl:   <http://www.w3.org/2002/07/owl#> .
@prefix prela: <http://sweetontology.net/relaPhysical/> .
@prefix pstate: <http://sweetontology.net/statePhysical/> .
@prefix xsd:   <http://www.w3.org/2001/XMLSchema#> .
@prefix rdfs:  <http://www.w3.org/2000/01/rdf-schema#> .
@prefix sys:   <http://sweetontology.net/phenSystem/> .
@prefix wave:  <http://sweetontology.net/phenWave/> .
@prefix sdir:  <http://sweetontology.net/reprSpaceDirection/> .
@prefix sol:   <http://sweetontology.net/phenSolid/> .
@prefix phen:  <http://sweetontology.net/phen/> .
@prefix rdf:   <http://www.w3.org/1999/02/22-rdf-syntax-ns#> .
@prefix inst:  <http://sweetontology.net/phenFluidInstability/> .
@prefix tran:  <http://sweetontology.net/phenFluidTransport/> .
@prefix rela:  <http://sweetontology.net/rela/> .

wave:SurfaceWave  a       owl:Class ;
        rdfs:subClassOf   wave:Wave ;
        owl:disjointWith  wave:InternalWave , wave:BodyWave .

wave:InternalGravityWave
        a                    owl:Class ;
        rdfs:comment         "A wave that propagates in density-stratified fluid under the influence of buoyancy forces."@en ;
        rdfs:subClassOf      wave:InternalWave , wave:GravityWave ;
        rdfs:subClassOf      [ a                   owl:Restriction ;
                               owl:onProperty      rela:hasState ;
                               owl:someValuesFrom  inst:StaticStability
                             ] ;
        owl:equivalentClass  wave:InternalWave .

wave:SoundWave  a  owl:Class .

<>      a                owl:Ontology ;
        rdfs:label       "SWEET Ontology" ;
        owl:imports      <phen> , <phenSolid> , <phenSystem> , <phenFluidInstability> , <phenFluidTransport> , <statePhysical> , <phenSystemComplexity> , <rela> , <reprSpaceDirection> , <procPhysical> , <relaPhysical> ;
        owl:versionInfo  "3.1.0" .

wave:LongitudinalWave
        a                owl:Class ;
        rdfs:comment     "Longitudinal waves are waves that have vibrations along or parallel to their direction of travel. They include waves in which the motion of the medium is in the same direction as the motion of the wave. Mechanical longitudinal waves have been also referred to as compressional waves or pressure waves"@en ;
        rdfs:subClassOf  wave:Wave ;
        rdfs:subClassOf  [ a               owl:Restriction ;
                           owl:hasValue    sdir:Parallel ;
                           owl:onProperty  prela:hasOscillationDirection
                         ] .

wave:CapillaryWave  a    owl:Class ;
        rdfs:subClassOf  wave:Wave .

wave:Acoustics  a  owl:Class .

wave:RayleighWave  a     owl:Class ;
        rdfs:comment     "Rayleigh waves, also called ground roll, are surface waves that travel as ripples similar to those on the surface of water. The existence of these waves was predicted by John William Strutt, Lord Rayleigh, in 1885. They are slower than body waves, roughly 70% of the velocity of S waves, and have been asserted to be visible during an earthquake in an open space like a parking lot where the cars move up and down with the waves. Reports among seismologists suggest that the apparent motion may be due to distortion of the human eye during shaking. Anecdotally, placing people on shake tables causes the room to appear to ripple. In any case, waves of the reported amplitude, wavelength, and velocity of the visible waves have never been recorded instrumentally."@en ;
        rdfs:subClassOf  wave:SolidWave , wave:AcousticWave , wave:SurfaceWave .

wave:WavePhenomena  a    owl:Class ;
        rdfs:subClassOf  phen:Phenomena ;
        rdfs:subClassOf  [ a                   owl:Restriction ;
                           owl:onProperty      rela:hasPhenomena ;
                           owl:someValuesFrom  wave:Wave
                         ] .

wave:TopographicWave  a  owl:Class ;
        rdfs:comment     "Waves with a restoring force arising from variations in depth. The stretching or compression of displaced columns of water generates anomalous vorticity tending to drive them back to their original position." ;
        rdfs:subClassOf  wave:GravityWave .

wave:ShallowWaterWave
        a                owl:Class ;
        rdfs:comment     "An ocean wave with its length sufficiently large compared to the water depth (i.e., 25 or more times the depth)"@en ;
        rdfs:subClassOf  wave:GravityWave .

wave:InertialWave  a  owl:Class .

wave:HelmholtzWave  a    owl:Class ;
        rdfs:comment     "An unstable wave in a system of two homogeneous fluids with a velocity discontinuity at the interface."@en ;
        rdfs:subClassOf  wave:GravityWave .

wave:TravelingWave  a     owl:Class ;
        rdfs:subClassOf   wave:Wave ;
        owl:disjointWith  wave:StandingWave .

wave:SolidWave  a        owl:Class ;
        rdfs:subClassOf  wave:Wave ;
        rdfs:subClassOf  [ a               owl:Restriction ;
                           owl:hasValue    pstate:Solid ;
                           owl:onProperty  rela:hasState
                         ] .

wave:TransverseWave  a   owl:Class ;
        rdfs:comment     "A transverse wave is a wave that causes vibration in the medium in a perpendicular direction to its own motion. For example: if a wave moves along the x-axis, its disturbances are in the yz-plane. In other words, it causes medium disturbances across the two-dimensional plane that it is travelling in. Contrary to popular belief, transversal waves do not necessarily move up and down."@en ;
        rdfs:subClassOf  wave:Wave ;
        rdfs:subClassOf  [ a               owl:Restriction ;
                           owl:hasValue    sdir:Perpendicular ;
                           owl:onProperty  prela:hasOscillationDirection
                         ] .

wave:AcousticGravityWave
        a                owl:Class ;
        rdfs:comment     "A wave disturbance with restoring forces that include buoyancy and the elastic compressibility of the fluid medium." ;
        rdfs:label       "Acoustic Gravity Wave" ;
        rdfs:subClassOf  wave:AcousticWave , wave:GravityWave .

wave:GravityWave  a          owl:Class ;
        rdfs:comment         "A wave disturbance in which buoyancy (or reduced gravity) acts as the restoring force on parcels displaced from hydrostatic equilibrium."@en ;
        rdfs:label           "Gravity Wave" ;
        rdfs:subClassOf      wave:FluidWave ;
        rdfs:subClassOf      [ a                   owl:Restriction ;
                               owl:onProperty      prela:hasRestoringForce ;
                               owl:someValuesFrom  tran:Buoyancy
                             ] ;
        owl:equivalentClass  wave:GravitationalWave .

wave:ShockWave  a        owl:Class ;
        rdfs:subClassOf  wave:Wave ;
        rdfs:subClassOf  [ a                  owl:Restriction ;
                           owl:allValuesFrom  sysc:Shock ;
                           owl:onProperty     rela:hasPhenomena
                         ] .

wave:ShortWave  a        owl:Class ;
        rdfs:comment     "With regard to atmospheric circulation, a progressive wave in the horizontal pattern of air motion with dimensions of cyclonic scale, as distinguished from a long wave."@en ;
        rdfs:subClassOf  wave:Wave .

wave:AlfvenWave  a       owl:Class ;
        rdfs:subClassOf  wave:PlasmaWave .

wave:LongCrestedWave  a  owl:Class ;
        rdfs:comment     "Ocean surface waves that are nearly two-dimensional, in that the crests appear very long in comparison with the wavelength, and the energy propagation is concentrated in a narrow band around the mean wave direction."@en ;
        rdfs:subClassOf  wave:SurfaceWave .

wave:KelvinWave  a       owl:Class ;
        rdfs:comment     "A type of low-frequency gravity wave trapped to a vertical boundary, or the equator, which propagates anticlockwise (in the Northerm Hemisphere) around a basin."@en ;
        rdfs:subClassOf  wave:GravityWave .

wave:MagnetohydrodynamicWave
        a                owl:Class ;
        rdfs:subClassOf  wave:PlasmaWave .

wave:ShearWave  a        owl:Class ;
        rdfs:subClassOf  wave:SolidWave , wave:TransverseWave ;
        rdfs:subClassOf  [ a                   owl:Restriction ;
                           owl:onProperty      prela:hasRestoringForce ;
                           owl:someValuesFrom  sol:Shear
                         ] .

wave:Wave  a             owl:Class ;
        rdfs:subClassOf  sys:Oscillation .

wave:Seiche  a           owl:Class ;
        rdfs:comment     "A seiche is a standing wave in an enclosed or partially enclosed body of water. Seiches and seiche-related phenomena have been observed on lakes, reservoirs, bays and seas. The key requirement for formation of a seiche is that the body of water be at least partially bounded, allowing natural phenomena to form a standing wave."@en ;
        rdfs:subClassOf  wave:StandingWave .

wave:PlanetaryWave  a  owl:Class .

wave:KelvinHelmholtzWave
        a                owl:Class ;
        rdfs:comment     "A waveform disturbance that arises from Kelvin?Helmholtz instability."@en ;
        rdfs:subClassOf  wave:GravityWave ;
        rdfs:subClassOf  [ a                  owl:Restriction ;
                           owl:allValuesFrom  inst:KelvinHelmholtzInstability ;
                           owl:onProperty     rela:hasState
                         ] .

wave:InertiaWave  a          owl:Class ;
        rdfs:comment         "1. Any wave motion in which no form of energy other than kinetic energy is present. In this general sense, Helmholtz waves, barotropic disturbances, Rossby waves, etc., are inertia waves. 2. More restrictedly, a wave motion in which the source of kinetic energy of the disturbance is the rotation of the fluid about some given axis. In the atmosphere a westerly wind system is such a source, the inertia waves here being, in general, stable. A similar analysis has been applied to smaller vortices, such as the hurricane. See inertial instability"@en ;
        rdfs:subClassOf      wave:InternalWave ;
        rdfs:subClassOf      [ a                   owl:Restriction ;
                               owl:onProperty      prela:hasRestoringForce ;
                               owl:someValuesFrom  proc:CoriolisForce
                             ] ;
        owl:equivalentClass  wave:InertialWave .

wave:Sound  a   owl:Class .

wave:GravitationalWave
        a       owl:Class .

wave:InternalWave  a  owl:Class .

wave:FluidWave  a        owl:Class ;
        rdfs:subClassOf  wave:Wave ;
        rdfs:subClassOf  [ a               owl:Restriction ;
                           owl:hasValue    pstate:Fluid ;
                           owl:onProperty  rela:hasState
                         ] .

wave:StandingWave  a     owl:Class ;
        rdfs:comment     "A wave that is stationary with respect to the medium in which it is embedded, for example, two equal gravity waves moving in opposite directions."@en ;
        rdfs:subClassOf  wave:Wave .

wave:BodyWave  a         owl:Class ;
        rdfs:subClassOf  wave:SolidWave .

wave:AcousticWave  a         owl:Class ;
        rdfs:subClassOf      wave:Wave ;
        rdfs:subClassOf      [ a                   owl:Restriction ;
                               owl:onProperty      prela:hasRestoringForce ;
                               owl:someValuesFrom  proc:Pressure
                             ] ;
        owl:equivalentClass  wave:Acoustics , wave:Acoustic , wave:Sound , wave:SoundWave .

wave:Acoustic  a  owl:Class .

wave:Whistler  a         owl:Class ;
        rdfs:subClassOf  wave:SoundWave , wave:PlasmaWave .

wave:RossbyWave  a           owl:Class ;
        rdfs:comment         "Rossby (or planetary) waves are large-scale motions in the ocean or atmosphere whose restoring force is the variation in Coriolis effect with latitude. The waves were first identified in the atmosphere in 1939 by Carl-Gustaf Arvid Rossby who went on to explain their motion. Rossby waves are a subset of inertial waves"@en ;
        rdfs:subClassOf      wave:InertialWave ;
        owl:equivalentClass  wave:PlanetaryWave .

wave:PlasmaWave  a       owl:Class ;
        rdfs:subClassOf  wave:Wave ;
        rdfs:subClassOf  [ a               owl:Restriction ;
                           owl:hasValue    pstate:Plasma ;
                           owl:onProperty  rela:hasState
                         ] .

wave:CompressionWave  a  owl:Class ;
        rdfs:subClassOf  wave:LongitudinalWave .
