@base          <http://sweetontology.net/phenHelio> .
@prefix waves: <http://sweetontology.net/procWave/> .
@prefix star:  <http://sweetontology.net/phenStar/> .
@prefix owl:   <http://www.w3.org/2002/07/owl#> .
@prefix planet: <http://sweetontology.net/realm/> .
@prefix prela: <http://sweetontology.net/relaPhysical/> .
@prefix part:  <http://sweetontology.net/matrParticle/> .
@prefix xsd:   <http://www.w3.org/2001/XMLSchema#> .
@prefix rdfs:  <http://www.w3.org/2000/01/rdf-schema#> .
@prefix sys:   <http://sweetontology.net/phenSystem/> .
@prefix phen:  <http://sweetontology.net/phen/> .
@prefix rdf:   <http://www.w3.org/1999/02/22-rdf-syntax-ns#> .
@prefix pproc: <http://sweetontology.net/procPhysical/> .
@prefix helio: <http://sweetontology.net/phenHelio/> .
@prefix rela:  <http://sweetontology.net/rela/> .
@prefix screla: <http://sweetontology.net/relaSci/> .

<>      a                owl:Ontology ;
        rdfs:label       "SWEET Ontology" ;
        owl:imports      <procWave> , <rela> , <phenSystem> , <phenStar> , <realm> , <relaSci> , <matrParticle> , <relaPhysical> , <phen> , <procPhysical> ;
        owl:versionInfo  "3.1.0" .

helio:Substorm  a        owl:Class ;
        rdfs:subClassOf  helio:InterplanetaryPhenomena .

helio:ProtonPrecipitation
        a                owl:Class ;
        rdfs:subClassOf  phen:Precipitation , helio:GeomagneticStorm .

helio:BowShock  a        owl:Class ;
        rdfs:comment     "The bow shock is a discontinuity that forms in the solar wind when the supersonic solar wind encounters the magnetic field of a planet, very similar to the shock wave that forms upstream of an aircraft moving at a supersonic speed."@en ;
        rdfs:subClassOf  helio:BowShockCrossing .

helio:Geomagnetism  a    owl:Class ;
        rdfs:subClassOf  pproc:Magnetism .

helio:AtmosphericLightEmission
        a                owl:Class ;
        rdfs:subClassOf  helio:HeliosphericPhenomena ;
        rdfs:subClassOf  [ a                  owl:Restriction ;
                           owl:allValuesFrom  waves:Emission ;
                           owl:onProperty     rela:hasPhenomena
                         ] .

helio:MagnetopauseCrossing
        a                owl:Class ;
        rdfs:subClassOf  helio:HeliosphericPhenomena .

helio:BowShockCrossing
        a                owl:Class ;
        rdfs:subClassOf  helio:HeliosphericPhenomena .

helio:SolarParticleEvent
        a                owl:Class ;
        rdfs:subClassOf  helio:GeomagneticStorm .

helio:InterplanetaryPhenomena
        a                owl:Class ;
        rdfs:subClassOf  phen:Phenomena .

helio:SolarWindExtreme
        a                owl:Class ;
        rdfs:subClassOf  helio:InterplanetaryPhenomena .

helio:Aurora  a          owl:Class ;
        rdfs:comment     "The sporadic radiant emission from the upper atmosphere over the middle and high latitudes"@en ;
        rdfs:subClassOf  helio:AtmosphericLightEmission .

helio:SolarWind  a       owl:Class ;
        rdfs:comment     "The solar wind is a stream of charged particles (i.e., a plasma) which are ejected from the upper atmosphere of the sun. It consists mostly of high-energy electrons and protons (about 1 keV) that are able to escape the sun's gravity in part because of the high temperature of the corona and the high kinetic energy particles gain through a process that is not well understood at this time." ;
        rdfs:subClassOf  star:StellarWind ;
        rdfs:subClassOf  [ a               owl:Restriction ;
                           owl:hasValue    star:Sun ;
                           owl:onProperty  prela:hasAstronomicalBody
                         ] .

helio:HeliosphericPhenomena
        a                owl:Class ;
        rdfs:subClassOf  phen:Phenomena .

helio:Airglow  a         owl:Class ;
        rdfs:subClassOf  helio:AtmosphericLightEmission .

helio:Heliosheath  a     owl:Class ;
        rdfs:subClassOf  helio:HeliosphericPhenomena .

helio:SchumannResonance
        a                owl:Class ;
        rdfs:subClassOf  helio:HeliosphericPhenomena .

helio:SunEarthInteraction
        a                owl:Class ;
        rdfs:subClassOf  sys:Interaction ;
        rdfs:subClassOf  [ a               owl:Restriction ;
                           owl:hasValue    star:Sun ;
                           owl:onProperty  screla:hasCause
                         ] ;
        rdfs:subClassOf  [ a               owl:Restriction ;
                           owl:hasValue    planet:Earth ;
                           owl:onProperty  screla:hasEffect
                         ] .

helio:GeomagneticStorm
        a                owl:Class ;
        rdfs:comment     "A geomagnetic storm is a temporary disturbance of the Earths magnetosphere caused by a disturbance in space weather. Associated with solar coronal mass ejections (CME), coronal holes, or solar flares, a geomagnetic storm is caused by a solar wind shock wave which typically strikes the Earths magnetic field 24 to 36 hours after the event. This only happens if the shock wave travels in a direction toward Earth. The solar wind pressure on the magnetosphere will increase or decrease depending on the Sun's activity. These solar wind pressure changes modify the electric currents in the ionosphere." ;
        rdfs:subClassOf  phen:Event , helio:InterplanetaryPhenomena , sys:Disturbance ;
        rdfs:subClassOf  [ a                  owl:Restriction ;
                           owl:allValuesFrom  helio:SpaceWeather ;
                           owl:onProperty     rela:hasPhenomena
                         ] .

owl:versionInfo  a  owl:AnnotationProperty .

helio:AuroralSubstorm
        a                    owl:Class ;
        rdfs:subClassOf      helio:AtmosphericLightEmission ;
        owl:equivalentClass  helio:MagneticSubstorm .

helio:Magnetotail  a     owl:Class ;
        rdfs:subClassOf  helio:HeliosphericPhenomena .

helio:InterplanetaryShock
        a                owl:Class ;
        rdfs:subClassOf  helio:InterplanetaryPhenomena .

helio:MagneticStorm  a       owl:Class ;
        owl:equivalentClass  helio:GeomagneticStorm .

helio:TelluricCurrent
        a                owl:Class ;
        rdfs:subClassOf  pproc:ElectricCurrent .

helio:SpaceWeather  a    owl:Class ;
        rdfs:comment     "Space weather is the concept of changing environmental conditions in outer space. It is distinct from the concept of weather within a planetary atmosphere, and generally deals with the interactions of ambient radiation and matter within interplanetary, and occasionally interstellar space. Space weather describes the conditions in space that affect Earth and its technological systems. Our space weather is a consequence of the behavior of the sun, the nature of Earth's magnetic field, and our location in the solar system." ;
        rdfs:subClassOf  helio:HeliosphericPhenomena .

helio:MagneticSubstorm
        a       owl:Class .

helio:Magnetosheath  a   owl:Class ;
        rdfs:subClassOf  helio:HeliosphericPhenomena .
