@base          <http://sweetontology.net/phen> .
@prefix tstate: <http://sweetontology.net/stateTimeFrequency/> .
@prefix proc:  <http://sweetontology.net/procPhysical/> .
@prefix trela: <http://sweetontology.net/relaTime/> .
@prefix owl:   <http://www.w3.org/2002/07/owl#> .
@prefix planet: <http://sweetontology.net/phen/> .
@prefix xsd:   <http://www.w3.org/2001/XMLSchema#> .
@prefix rdfs:  <http://www.w3.org/2000/01/rdf-schema#> .
@prefix sys:   <http://sweetontology.net/phenSystem/> .
@prefix srela: <http://sweetontology.net/relaSpace/> .
@prefix rad:   <http://sweetontology.net/propEnergyFlux/> .
@prefix rdf:   <http://www.w3.org/1999/02/22-rdf-syntax-ns#> .
@prefix sstate: <http://sweetontology.net/stateSystem/> .
@prefix sscale: <http://sweetontology.net/stateSpaceScale/> .
@prefix realm: <http://sweetontology.net/realm/> .
@prefix state: <http://sweetontology.net/state/> .
@prefix rela:  <http://sweetontology.net/rela/> .
@prefix screla: <http://sweetontology.net/relaSci/> .

planet:Occurrence  a  owl:Class .

planet:StochasticProcess
        a                owl:Class ;
        rdfs:subClassOf  planet:DynamicalPhenomena ;
        rdfs:subClassOf  [ a               owl:Restriction ;
                           owl:hasValue    sstate:Stochastic ;
                           owl:onProperty  rela:hasState
                         ] .

planet:AtmosphereOceanExchange
        a       owl:Class .

planet:DynamicalPhenomena
        a                owl:Class ;
        rdfs:subClassOf  planet:Phenomena .

planet:AtmosphereLandExchange
        a                owl:Class ;
        rdfs:subClassOf  sys:Exchange , planet:Phenomena ;
        rdfs:subClassOf  [ a                   owl:Restriction ;
                           owl:onProperty      screla:hasSource ;
                           owl:someValuesFrom  realm:Land
                         ] ;
        rdfs:subClassOf  [ a                   owl:Restriction ;
                           owl:onProperty      screla:hasSource ;
                           owl:someValuesFrom  realm:Atmosphere
                         ] .

planet:RadiativeCooling
        a                    owl:Class ;
        rdfs:comment         "In meteorology, the result of radiative cooling of the earth's surface and adjacent air.  Radiational cooling occurs, as is typical on calm, clear nights"@en ;
        rdfs:subClassOf      rad:RadiativeForcing , proc:Cooling ;
        owl:disjointWith     planet:RadiativeHeating ;
        owl:equivalentClass  planet:RadiationalCooling .

<>      a                owl:Ontology ;
        rdfs:label       "SWEET Ontology" ;
        owl:imports      <stateTimeFrequency> , <state> , <rela> , <relaSpace> , <phenSystem> , <propEnergyFlux> , <relaSci> , <stateSystem> , <relaTime> , <procPhysical> , <stateSpaceScale> , <realm> ;
        owl:versionInfo  "3.1.0" .

planet:BrownianMotion
        a                owl:Class ;
        rdfs:comment     "A stochastic process that describes (among other things) the rapid and chaotic motion of particles suspended in a fluid at rest as a consequence of fluctuations in the rate at which fluid molecules collide with the particles."@en ;
        rdfs:subClassOf  planet:StochasticProcess .

planet:ExtremeEvent  a   owl:Class ;
        rdfs:subClassOf  planet:Event ;
        rdfs:subClassOf  [ a               owl:Restriction ;
                           owl:hasValue    tstate:Infrequent ;
                           owl:onProperty  trela:hasFrequency
                         ] .

planet:RadiativeHeating
        a                    owl:Class ;
        rdfs:subClassOf      rad:RadiativeForcing , proc:Heating ;
        owl:equivalentClass  planet:RadiationalHeating .

planet:PlanetaryPhenomena
        a                owl:Class ;
        rdfs:comment     "Planetary phenomena are the movements of planets and the sun, including  for example orbits, alignments, eclipses day and night cycles, and the change of seasons."@en ;
        rdfs:subClassOf  planet:Phenomena ;
        rdfs:subClassOf  [ a               owl:Restriction ;
                           owl:hasValue    sscale:PlanetaryScale ;
                           owl:onProperty  srela:hasSpatialScale
                         ] .

planet:Event  a              owl:Class ;
        rdfs:subClassOf      planet:Phenomena ;
        owl:equivalentClass  planet:Occurrence .

planet:Flash  a          owl:Class ;
        rdfs:subClassOf  planet:Phenomena .

planet:RadiationalCooling
        a       owl:Class .

planet:RadiationalHeating
        a       owl:Class .

planet:AirSeaExchange
        a                    owl:Class ;
        rdfs:subClassOf      sys:Exchange , planet:Phenomena ;
        rdfs:subClassOf      [ a                   owl:Restriction ;
                               owl:onProperty      screla:hasSource ;
                               owl:someValuesFrom  realm:Ocean
                             ] ;
        rdfs:subClassOf      [ a                   owl:Restriction ;
                               owl:onProperty      screla:hasSource ;
                               owl:someValuesFrom  realm:Atmosphere
                             ] ;
        owl:equivalentClass  planet:AtmosphereOceanExchange .

planet:Phenomena  a  owl:Class .

planet:Teleconnection
        a                owl:Class ;
        rdfs:subClassOf  planet:PlanetaryPhenomena .

planet:Precipitation  a  owl:Class ;
        rdfs:subClassOf  planet:Phenomena .
