@base          <http://sweetontology.net/phenGeolGeomorphology> .
@prefix comp:  <http://sweetontology.net/matrCompound/> .
@prefix solid: <http://sweetontology.net/phenSolid/> .
@prefix crela: <http://sweetontology.net/relaChemical/> .
@prefix impa:  <http://sweetontology.net/stateRoleImpact/> .
@prefix owl:   <http://www.w3.org/2002/07/owl#> .
@prefix planet: <http://sweetontology.net/realm/> .
@prefix petr:  <http://sweetontology.net/matrRock/> .
@prefix xsd:   <http://www.w3.org/2001/XMLSchema#> .
@prefix rdfs:  <http://www.w3.org/2000/01/rdf-schema#> .
@prefix geol:  <http://sweetontology.net/phenGeol/> .
@prefix sys:   <http://sweetontology.net/phenSystemComplexity/> .
@prefix sed:   <http://sweetontology.net/matrSediment/> .
@prefix phen:  <http://sweetontology.net/phen/> .
@prefix rdf:   <http://www.w3.org/1999/02/22-rdf-syntax-ns#> .
@prefix geomor: <http://sweetontology.net/phenGeolGeomorphology/> .
@prefix screla: <http://sweetontology.net/relaSci/> .
@prefix rela:  <http://sweetontology.net/rela/> .
@prefix trans: <http://sweetontology.net/phenFluidTransport/> .

geomor:Avalanche  a      owl:Class ;
        rdfs:comment     "A mass of snow, ice or rocks moving rapidly down a steep mountain slope. Avalanches may be characterized as loose and turbulent, or slab; either type may be dry or wet according to the nature of the snow forming it, although dry snow usually forms loose avalanches and wet snow forms slabs. A large avalanche sweeps a current of air along with and in front of it as an avalanche wind, which supplements its already tremendous destructive force." ;
        rdfs:subClassOf  sys:Collapse , geomor:Slide .

geomor:Denundation  a    owl:Class ;
        rdfs:subClassOf  geomor:MaterialDisplacement .

geomor:Slump  a          owl:Class ;
        rdfs:subClassOf  geomor:MaterialDisplacement .

geomor:Saltation  a      owl:Class ;
        rdfs:subClassOf  geomor:MaterialDisplacement .

geomor:Diagenesis  a     owl:Class ;
        rdfs:comment     "In geology and oceanography, diagenesis is any chemical, physical, or biological change undergone by a sediment after its initial deposition and during and after its lithification, exclusive of surface alteration (weathering) and metamorphism. These changes happen at relatively low temperatures and pressures and result in changes to the rock's original mineralogy and texture. The boundary between diagenesis and metamorphism, which occurs under conditions of higher temperature and pressure, is gradational. After deposition, sediments are compacted as they are buried beneath successive layers of sediment and cemented by minerals that precipitate from solution. Grains of sediment, rock fragments and fossils can be replaced by other minerals during diagenesis. Porosity usually decreases during diagenesis, except in rare cases such as dissolution of minerals and dolomitization."@en ;
        rdfs:subClassOf  geomor:SedimentFormation .

geomor:Solifluction  a   owl:Class ;
        rdfs:subClassOf  geomor:MaterialDisplacement .

geomor:Abrasion  a       owl:Class ;
        rdfs:subClassOf  geomor:MaterialDisplacement .

geomor:Mudslide  a       owl:Class ;
        rdfs:subClassOf  geomor:Slide .

geomor:Reptation  a  owl:Class .

geomor:Weathering  a      owl:Class ;
        rdfs:comment      "Weathering is the decomposition of rocks, soils and their minerals through direct contact with the Earth's atmosphere. Weathering occurs in situ, or with no movement, and thus should not to be confused with erosion, which involves the movement and disintegration of rocks and minerals by agents such as water, ice, wind and gravity."@en ;
        rdfs:subClassOf   geomor:MaterialDisplacement ;
        rdfs:subClassOf   [ a                  owl:Restriction ;
                            owl:allValuesFrom  petr:Rock ;
                            owl:onProperty     crela:hasSubstance
                          ] ;
        owl:disjointWith  solid:Erosion .

geomor:Slide  a          owl:Class ;
        rdfs:subClassOf  phen:Phenomena , geomor:MaterialDisplacement ;
        rdfs:subClassOf  [ a               owl:Restriction ;
                           owl:hasValue    impa:Hazard ;
                           owl:onProperty  screla:hasImpact
                         ] .

geomor:Landslide  a      owl:Class ;
        rdfs:comment     "A landslide (or landslip) is a geological phenomenon which includes a wide range of ground movement, such as rock falls, deep solidure of slopes and shallow debris flows, which can occur in offshore, coastal and onshore environments. [Wikpedia]"@en ;
        rdfs:subClassOf  geomor:Slide ;
        rdfs:subClassOf  [ a                  owl:Restriction ;
                           owl:allValuesFrom  planet:Land ;
                           owl:onProperty     rela:hasRealm
                         ] .

<>      a                owl:Ontology ;
        rdfs:label       "SWEET Ontology" ;
        owl:imports      <matrSediment> , <phenFluidTransport> , <phen> , <stateRoleImpact> , <matrCompound> , <rela> , <realm> , <relaChemical> , <phenGeol> , <matrRock> , <phenSystemComplexity> , <phenSolid> , <relaSci> ;
        owl:versionInfo  "3.1.0" .

geomor:Subsidence  a     owl:Class ;
        rdfs:comment     "Subsidence is the motion of a surface (usually, the Earth's surface) as it shifts downward relative to a datum such as sea-level. [Wikipedia]"@en ;
        rdfs:subClassOf  geomor:MaterialDisplacement .

geomor:RockSlopeFailure
        a                owl:Class ;
        rdfs:subClassOf  geomor:MaterialDisplacement .

geomor:Karst  a          owl:Class ;
        rdfs:comment     "Karst topography is a landscape shaped by the dissolution of a layer or layers of soluble bedrock, usually carbonate rock such as limestone or dolomite. [Wikipedia]"@en ;
        rdfs:subClassOf  geol:GeologicalPhenomena .

geomor:Creep  a              owl:Class ;
        rdfs:subClassOf      geomor:MaterialDisplacement ;
        owl:equivalentClass  geomor:Reptation .

geomor:Sedimentation  a  owl:Class ;
        rdfs:comment     "The process of depositing material by water, wind, or glaciers."@en ;
        rdfs:subClassOf  geol:GeologicalPhenomena ;
        rdfs:subClassOf  [ a                  owl:Restriction ;
                           owl:allValuesFrom  trans:Deposition ;
                           owl:onProperty     rela:hasPhenomena
                         ] .

geomor:MassWasting  a    owl:Class ;
        rdfs:subClassOf  geomor:MaterialDisplacement .

geomor:Exfoliation  a    owl:Class ;
        rdfs:subClassOf  geomor:Weathering .

geomor:Compaction  a     owl:Class ;
        rdfs:comment     "Compaction, part of the process of lithification involving mechanical dewatering of a sediment by progressive loading under several km of geomaterial [Wikipedia]"@en ;
        rdfs:subClassOf  geomor:SedimentFormation .

geomor:SedimentFormation
        a                owl:Class ;
        rdfs:subClassOf  geomor:MaterialDisplacement ;
        rdfs:subClassOf  [ a                  owl:Restriction ;
                           owl:allValuesFrom  sed:Sediment ;
                           owl:onProperty     crela:hasSubstance
                         ] .

geomor:Haloclasty  a     owl:Class ;
        rdfs:subClassOf  geomor:Weathering ;
        rdfs:subClassOf  [ a               owl:Restriction ;
                           owl:hasValue    comp:Salt ;
                           owl:onProperty  rela:hasPhenomena
                         ] .

geomor:MaterialDisplacement
        a                owl:Class ;
        rdfs:subClassOf  phen:PlanetaryPhenomena .
