@base          <http://sweetontology.net/phenSystem> .
@prefix mod:   <http://sweetontology.net/reprSciModel/> .
@prefix phen:  <http://sweetontology.net/phen/> .
@prefix rdf:   <http://www.w3.org/1999/02/22-rdf-syntax-ns#> .
@prefix owl:   <http://www.w3.org/2002/07/owl#> .
@prefix xsd:   <http://www.w3.org/2001/XMLSchema#> .
@prefix rdfs:  <http://www.w3.org/2000/01/rdf-schema#> .
@prefix sys:   <http://sweetontology.net/phenSystem/> .

sys:Collection  a        owl:Class ;
        rdfs:subClassOf  sys:SystemStateChange .

sys:Disturbance  a       owl:Class ;
        rdfs:subClassOf  sys:Variation .

sys:Interruption  a      owl:Class ;
        rdfs:subClassOf  sys:SystemStateChange .

sys:System  a            owl:Class ;
        rdfs:comment     "System is a set of interacting or interdependent entities, real or abstract, forming an integrated whole." ;
        rdfs:subClassOf  mod:Model .

sys:Conversion  a        owl:Class ;
        rdfs:subClassOf  sys:SystemStateChange .

sys:Change  a            owl:Class ;
        rdfs:subClassOf  sys:SystemPhenomena .

sys:Displacement  a      owl:Class ;
        rdfs:subClassOf  sys:SystemStateChange .

sys:Fall  a     owl:Class .

sys:Stress  a            owl:Class ;
        rdfs:subClassOf  sys:SystemPhenomena .

sys:Lag  a               owl:Class ;
        rdfs:subClassOf  sys:SystemPhenomena .

sys:Inundation  a        owl:Class ;
        rdfs:subClassOf  sys:SystemStateChange .

<>      a                owl:Ontology ;
        rdfs:label       "SWEET Ontology" ;
        owl:imports      <phen> , <reprSciModel> ;
        owl:versionInfo  "3.1.0" .

sys:Variation  a         owl:Class ;
        rdfs:subClassOf  sys:SystemStateChange .

sys:Exchange  a          owl:Class ;
        rdfs:subClassOf  sys:SystemStateChange .

sys:Drift  a             owl:Class ;
        rdfs:subClassOf  sys:Trend .

sys:Accumulation  a      owl:Class ;
        rdfs:subClassOf  sys:SystemPhenomena .

sys:Increase  a              owl:Class ;
        rdfs:subClassOf      sys:SystemStateChange ;
        owl:equivalentClass  sys:Rise .

sys:Oscillation  a       owl:Class ;
        rdfs:subClassOf  sys:SystemStateChange .

sys:Shift  a             owl:Class ;
        rdfs:subClassOf  sys:Trend .

sys:Comeback  a          owl:Class ;
        rdfs:subClassOf  sys:Return .

sys:SystemStateChange
        a                owl:Class ;
        rdfs:subClassOf  sys:Change .

sys:Perturbation  a      owl:Class ;
        rdfs:comment     "Any departure introduced into an assumed steady state of a system.   The magnitude is often assumed to be small so that product terms in the dependent variables may be neglected."@en ;
        rdfs:subClassOf  sys:Variation .

sys:Growth  a            owl:Class ;
        rdfs:subClassOf  sys:SystemStateChange .

sys:Flow  a              owl:Class ;
        rdfs:subClassOf  sys:SystemStateChange .

sys:Reduction  a  owl:Class .

sys:Demand  a            owl:Class ;
        rdfs:subClassOf  sys:SystemPhenomena .

sys:Vacillation  a       owl:Class ;
        rdfs:comment     "Oscillation, usually of a small amplitude, about a reference state."@en ;
        rdfs:subClassOf  sys:Oscillation .

sys:Retreat  a           owl:Class ;
        rdfs:subClassOf  sys:SystemStateChange .

sys:Deposit  a           owl:Class ;
        rdfs:subClassOf  sys:Accumulation .

sys:Extension  a         owl:Class ;
        rdfs:subClassOf  sys:SystemStateChange .

sys:Removal  a           owl:Class ;
        rdfs:subClassOf  sys:SystemStateChange .

sys:Decline  a  owl:Class .

sys:SystemPhenomena  a   owl:Class ;
        rdfs:subClassOf  phen:Phenomena .

sys:Trend  a             owl:Class ;
        rdfs:subClassOf  sys:SystemPhenomena .

sys:Interaction  a       owl:Class ;
        rdfs:comment     "process that multiple substances are in contact and have some consequence" ;
        rdfs:subClassOf  sys:SystemStateChange .

sys:Halting  a           owl:Class ;
        rdfs:subClassOf  sys:SystemStateChange .

sys:Destruction  a       owl:Class ;
        rdfs:subClassOf  sys:SystemStateChange .

sys:Drop  a     owl:Class .

sys:Recycling  a         owl:Class ;
        rdfs:subClassOf  sys:SystemPhenomena .

sys:Return  a            owl:Class ;
        rdfs:subClassOf  sys:SystemStateChange .

sys:Variability  a       owl:Class ;
        rdfs:subClassOf  sys:SystemStateChange .

sys:Loss  a              owl:Class ;
        rdfs:subClassOf  sys:SystemStateChange .

sys:Disruption  a        owl:Class ;
        rdfs:subClassOf  sys:SystemStateChange .

sys:Decrease  a              owl:Class ;
        rdfs:subClassOf      sys:SystemStateChange ;
        owl:equivalentClass  sys:Reduction , sys:Decline , sys:Fall , sys:Drop .

sys:Rise  a     owl:Class .

sys:Replenishment  a     owl:Class ;
        rdfs:subClassOf  sys:SystemStateChange .
