@base          <http://sweetontology.net/procChemical> .
@prefix proc:  <http://sweetontology.net/proc/> .
@prefix rdf:   <http://www.w3.org/1999/02/22-rdf-syntax-ns#> .
@prefix owl:   <http://www.w3.org/2002/07/owl#> .
@prefix part:  <http://sweetontology.net/matrParticle/> .
@prefix pproc: <http://sweetontology.net/procPhysical/> .
@prefix xsd:   <http://www.w3.org/2001/XMLSchema#> .
@prefix rdfs:  <http://www.w3.org/2000/01/rdf-schema#> .
@prefix state: <http://sweetontology.net/stateSystem/> .
@prefix rela:  <http://sweetontology.net/rela/> .
@prefix cproc: <http://sweetontology.net/procChemical/> .

<>      a                owl:Ontology ;
        rdfs:label       "SWEET Ontology" ;
        owl:imports      <procPhysical> , <stateSystem> , <rela> , <matrParticle> , <proc> ;
        owl:versionInfo  "3.1.0" .

cproc:Crystallization
        a                owl:Class ;
        rdfs:comment     "Crystallization is the (natural or artificial) process of formation of solid crystals precipitating from a solution, melt or more rarely deposited directly from a gas. [Wikipedia]"@en ;
        rdfs:subClassOf  cproc:ChemicalProcess .

cproc:Sorption  a            owl:Class ;
        owl:equivalentClass  [ a            owl:Class ;
                               owl:unionOf  ( cproc:Absorption cproc:Adsorption )
                             ] .

cproc:Leaching  a        owl:Class ;
        rdfs:comment     "In general, leaching is the extraction of certain materials from a carrier into a liquid (usually, but not always a solvent)."@en ;
        rdfs:subClassOf  cproc:ChemicalProcess .

cproc:Enrichment  a      owl:Class ;
        rdfs:subClassOf  cproc:ChemicalProcess .

cproc:Nitrification  a   owl:Class ;
        rdfs:subClassOf  cproc:Reaction .

cproc:Bond  a            owl:Class ;
        rdfs:subClassOf  cproc:ChemicalProcess .

cproc:Nucleation  a      owl:Class ;
        rdfs:comment     "Nucleation is the extremely localized budding of a distinct thermodynamic phase. Some examples of phases that may form via nucleation in liquids are gaseous bubbles, crystals, or glassy regions."@en ;
        rdfs:subClassOf  cproc:ChemicalProcess .

cproc:Triboluminescence
        a                owl:Class ;
        rdfs:comment     "Glows when struck"@en ;
        rdfs:subClassOf  cproc:Luminescence .

cproc:Phosphorescence
        a                owl:Class ;
        rdfs:comment     "Continues to glow after light source is removed"@en ;
        rdfs:subClassOf  cproc:Fluorescence .

cproc:ChemicalReaction
        a       owl:Class .

cproc:Absorption  a      owl:Class ;
        rdfs:subClassOf  cproc:ChemicalProcess .

cproc:Transmutation  a   owl:Class ;
        rdfs:subClassOf  cproc:ChemicalProcess .

cproc:ChargeExchange  a  owl:Class ;
        rdfs:subClassOf  cproc:ChemicalProcess .

cproc:Recrystalization
        a                owl:Class ;
        rdfs:subClassOf  cproc:Crystallization .

cproc:Acidification  a   owl:Class ;
        rdfs:comment     "Any process that decreases the pH value of a subtance."@en ;
        rdfs:subClassOf  cproc:ChemicalProcess .

cproc:Photodecomposition
        a       owl:Class .

cproc:Photodissociation
        a       owl:Class .

cproc:Adsorption  a      owl:Class ;
        rdfs:comment     "Adsorption is the accumulation of atoms or molecules on the surface of a material. This process creates a film of the adsorbate (the molecules or atoms being accumulated) on the adsorbent's surface. [Wikipedia]"@en ;
        rdfs:subClassOf  cproc:ChemicalProcess .

cproc:Luminescence  a    owl:Class ;
        rdfs:subClassOf  pproc:Radiation .

cproc:Bioluminescence
        a                owl:Class ;
        rdfs:subClassOf  cproc:Luminescence .

cproc:Titration  a       owl:Class ;
        rdfs:comment     "Titration is a common laboratory method of quantitative chemical analysis that is used to determine the unknown concentration of a known reactant."@en ;
        rdfs:subClassOf  cproc:ChemicalProcess .

cproc:ChemicalProcess
        a                    owl:Class ;
        rdfs:comment         "A chemical process is a method or means of somehow changing one or more chemicals or chemical compounds.  [Wikipedia]"@en ;
        rdfs:subClassOf      proc:Process ;
        owl:equivalentClass  cproc:ChemicalReaction , cproc:Reaction .

cproc:Calcification  a   owl:Class ;
        rdfs:comment     "Any process that increases the calcium concentration of a subtance."@en ;
        rdfs:subClassOf  cproc:ChemicalProcess .

cproc:Dissolution  a         owl:Class ;
        rdfs:comment         "Dissolution or solvation is the process of dissolving a solid substance into a solvent to yield a solution. [Wikipedia]"@en ;
        rdfs:subClassOf      cproc:ChemicalProcess ;
        owl:equivalentClass  cproc:Solvation .

cproc:Dilution  a        owl:Class ;
        rdfs:subClassOf  cproc:ChemicalProcess .

cproc:Thermoluminescence
        a                owl:Class ;
        rdfs:comment     "Glows when heated"@en ;
        rdfs:subClassOf  cproc:Luminescence .

cproc:Fluorescence  a    owl:Class ;
        rdfs:comment     "Fluorescence is a luminescence that is mostly found as an optical phenomenon in cold bodies, in which the molecular absorption of a photon triggers the emission of another photon with a longer wavelength. The energy difference between the absorbed and emitted photons ends up as molecular vibrations or heat. Usually the absorbed photon is in the ultraviolet range, and the emitted light is in the visible range, but this depends on the absorbance curve and Stokes shift of the particular fluorophore. Fluorescence is named after the mineral fluorite, composed of calcium fluoride, which often exhibits this phenomenon."@en ;
        rdfs:subClassOf  cproc:Luminescence .

cproc:Calcination  a     owl:Class ;
        rdfs:subClassOf  cproc:ChemicalProcess .

cproc:Electrolysis  a    owl:Class ;
        rdfs:comment     "Electrolysis is a method of using an electric current to drive an otherwise non-spontaneous chemical reaction."@en ;
        rdfs:subClassOf  cproc:ChemicalProcess .

cproc:Neutralization  a  owl:Class ;
        rdfs:comment     "In chemistry, neutralization is a chemical reaction (also called a water forming reaction since a water molecule is formed during the process) in which an acid and a base or alkali (soluble base) react to produce salt and water (H2O). During the process, hydrogen ions H+ (a bare proton) from the acid (proton donor) or a hydronium ion H3O+ and hydroxide ions OH_ or oxide ions O2_ from the base (proton acceptor) react together to form a water molecule H2O. [Wikipedia]"@en ;
        rdfs:subClassOf  cproc:ChemicalProcess .

cproc:Corrosion  a       owl:Class ;
        rdfs:subClassOf  cproc:ChemicalProcess .

cproc:Hydrolysis  a      owl:Class ;
        rdfs:comment     "Hydrolysis is a chemical reaction during which molecules of water (H2O) are split into hydrogen (H) and hydroxide anions (OHâˆ’) in the process of a chemical mechanism."@en ;
        rdfs:subClassOf  cproc:ChemicalProcess .

cproc:Reduction  a        owl:Class ;
        rdfs:subClassOf   cproc:ChemicalProcess ;
        owl:disjointWith  cproc:Oxidation .

cproc:Dehydration  a      owl:Class ;
        rdfs:subClassOf   cproc:ChemicalProcess ;
        owl:disjointWith  cproc:Hydration .

cproc:Photolysis  a          owl:Class ;
        rdfs:comment         "Photodissociation, photolysis, or photodecomposition is a chemical reaction in which a chemical compound is broken down by photons. It is defined as the interaction of one or more photons with one target molecule. [Wikipedia]"@en ;
        rdfs:subClassOf      cproc:ChemicalProcess ;
        rdfs:subClassOf      [ a                  owl:Restriction ;
                               owl:allValuesFrom  cproc:Absorption ;
                               owl:onProperty     rela:hasProcess
                             ] ;
        owl:equivalentClass  cproc:Photodecomposition , cproc:Photodissociation .

cproc:Solvation  a  owl:Class .

cproc:Combustion  a      owl:Class ;
        rdfs:subClassOf  cproc:ChemicalProcess .

cproc:Reaction  a  owl:Class .

cproc:Outgas  a          owl:Class ;
        rdfs:subClassOf  cproc:ChemicalProcess .

cproc:Fixation  a        owl:Class ;
        rdfs:subClassOf  cproc:ChemicalProcess .

cproc:Burning  a         owl:Class ;
        rdfs:subClassOf  cproc:ChemicalProcess .

cproc:Oxidation  a       owl:Class ;
        rdfs:comment     "Reaction of a substance with oxygen or incorporation of oxygen into a molecule."@en ;
        rdfs:subClassOf  cproc:Reaction .

cproc:NuclearFusion  a   owl:Class ;
        rdfs:subClassOf  cproc:ChemicalProcess .

cproc:Hydration  a       owl:Class ;
        rdfs:subClassOf  cproc:ChemicalProcess .

cproc:Desalinization  a  owl:Class ;
        rdfs:subClassOf  cproc:ChemicalProcess .
