@base          <http://sweetontology.net/propMass> .
@prefix mrela: <http://sweetontology.net/relaMath/> .
@prefix mult:  <http://sweetontology.net/propSpaceMultidimensional/> .
@prefix quan:  <http://sweetontology.net/propQuantity/> .
@prefix owl:   <http://www.w3.org/2002/07/owl#> .
@prefix pstate: <http://sweetontology.net/statePhysical/> .
@prefix xsd:   <http://www.w3.org/2001/XMLSchema#> .
@prefix rdfs:  <http://www.w3.org/2000/01/rdf-schema#> .
@prefix units: <http://sweetontology.net/reprSciUnits/> .
@prefix conc:  <http://sweetontology.net/propMass/> .
@prefix rdf:   <http://www.w3.org/1999/02/22-rdf-syntax-ns#> .
@prefix prop:  <http://sweetontology.net/prop/> .
@prefix oper:  <http://sweetontology.net/reprMathOperation/> .
@prefix rela:  <http://sweetontology.net/rela/> .
@prefix screla: <http://sweetontology.net/relaSci/> .

conc:SpecificVolume  a   owl:Class ;
        rdfs:comment     "1. The ratio of the mass of any substance to the volume occupied by it (usually expressed in kilograms per cubic meter, but any other unit system may be used); the reciprocal of specific volume."@en ;
        rdfs:subClassOf  quan:IntensiveProperty ;
        rdfs:subClassOf  [ a               owl:Restriction ;
                           owl:hasValue    units:meterCubedPerKilogram ;
                           owl:onProperty  screla:hasDefaultUnit
                         ] .

conc:Consistency  a  owl:Class .

conc:MassContent  a      owl:Class ;
        rdfs:subClassOf  conc:Content ;
        rdfs:subClassOf  [ a               owl:Restriction ;
                           owl:hasValue    units:kilogramPerMeterSquared ;
                           owl:onProperty  screla:hasDefaultUnit
                         ] ;
        rdfs:subClassOf  [ a                  owl:Restriction ;
                           owl:allValuesFrom  conc:Mass ;
                           owl:onProperty     mrela:hasFirstOperand
                         ] .

conc:Plasticity  a       owl:Class ;
        rdfs:subClassOf  conc:StrengthProperty .

conc:DryWeight  a        owl:Class ;
        rdfs:subClassOf  conc:Mass ;
        rdfs:subClassOf  [ a               owl:Restriction ;
                           owl:hasValue    pstate:Dry ;
                           owl:onProperty  rela:hasState
                         ] .

conc:Solidity  a             owl:Class ;
        rdfs:subClassOf      conc:StrengthProperty ;
        owl:equivalentClass  conc:Solidness .

conc:Solidness  a  owl:Class .

conc:BulkDensity  a      owl:Class ;
        rdfs:subClassOf  conc:Density .

conc:SigmaT  a           owl:Class ;
        rdfs:subClassOf  conc:Density .

conc:ConsistenceProperty
        a                owl:Class ;
        rdfs:subClassOf  conc:MaterialProperty .

conc:StrengthProperty
        a                owl:Class ;
        rdfs:subClassOf  conc:SolidProperty .

conc:Moles  a            owl:Class ;
        rdfs:subClassOf  quan:Quantity ;
        rdfs:subClassOf  [ a               owl:Restriction ;
                           owl:hasValue    units:mole ;
                           owl:onProperty  screla:hasDefaultUnit
                         ] .

conc:Grade  a            owl:Class ;
        rdfs:subClassOf  conc:MassConcentration .

conc:MeanMolecularWeight
        a                owl:Class ;
        rdfs:subClassOf  conc:MolecularWeight .

conc:Softness  a         owl:Class ;
        rdfs:subClassOf  conc:StrengthProperty .

conc:Flexure  a          owl:Class ;
        rdfs:subClassOf  conc:StrengthProperty .

<>      a                owl:Ontology ;
        rdfs:label       "SWEET Ontology" ;
        owl:imports      <propQuantity> , <reprSciUnits> , <relaMath> , <rela> , <prop> , <statePhysical> , <relaSci> , <reprMathOperation> , <propSpaceMultidimensional> ;
        owl:versionInfo  "3.1.0" .

conc:DissolvedConcentration
        a                owl:Class ;
        rdfs:subClassOf  conc:MassConcentration .

conc:Malleability  a     owl:Class ;
        rdfs:subClassOf  conc:StrengthProperty .

conc:MolecularWeight  a  owl:Class ;
        rdfs:subClassOf  conc:MassConcentration .

conc:Structure  a        owl:Class ;
        rdfs:subClassOf  conc:StrengthProperty .

conc:PotentialDensity
        a                owl:Class ;
        rdfs:comment     "The density of a unit of water after it is raised by an adiabatic process to the surface, i.e., determined from in-situ salinity and potential temperature (AGI, 1980). Density that would be reached by a compressible fluid if it were adiabatically compressed or expanded to a standard pressure."@en ;
        rdfs:subClassOf  conc:Density .

conc:Consistence  a          owl:Class ;
        rdfs:subClassOf      conc:ConsistenceProperty ;
        owl:equivalentClass  conc:Consistency .

conc:Texture  a          owl:Class ;
        rdfs:subClassOf  conc:ConsistenceProperty .

conc:Elasticity  a       owl:Class ;
        rdfs:subClassOf  conc:StrengthProperty .

conc:Density  a          owl:Class ;
        rdfs:comment     "1. The ratio of the mass of any substance to the volume occupied by it (usually expressed in kilograms per cubic meter, but any other unit system may be used); the reciprocal of specific volume."@en ;
        rdfs:subClassOf  quan:IntensiveProperty ;
        rdfs:subClassOf  [ a               owl:Restriction ;
                           owl:hasValue    units:kilogramPerMeterCubed ;
                           owl:onProperty  screla:hasDefaultUnit
                         ] .

conc:Dosage  a               owl:Class ;
        rdfs:subClassOf      conc:Mass ;
        owl:equivalentClass  conc:Dose .

conc:Dose  a    owl:Class .

conc:Hardness  a         owl:Class ;
        rdfs:subClassOf  conc:StrengthProperty .

conc:Mass  a             owl:Class ;
        rdfs:subClassOf  quan:ExtensiveProperty ;
        rdfs:subClassOf  [ a               owl:Restriction ;
                           owl:hasValue    units:kilogram ;
                           owl:onProperty  screla:hasDefaultUnit
                         ] .

conc:Content  a          owl:Class ;
        rdfs:subClassOf  conc:MassConcentration , oper:Ratio ;
        rdfs:subClassOf  [ a                  owl:Restriction ;
                           owl:allValuesFrom  mult:Area ;
                           owl:onProperty     mrela:hasSecondOperand
                         ] .

conc:SolidProperty  a    owl:Class ;
        rdfs:subClassOf  conc:MaterialProperty .

conc:Roughness  a        owl:Class ;
        rdfs:subClassOf  conc:MaterialProperty .

conc:Ductibility  a      owl:Class ;
        rdfs:subClassOf  conc:StrengthProperty .

conc:OpticalMass  a      owl:Class ;
        rdfs:comment     "The vertical integral of the density of absorbers between two altitudes; used mainly in determining the transmission through an absorbing gas."@en ;
        rdfs:subClassOf  quan:RadiationMediumInteractionQuantity ;
        rdfs:subClassOf  [ a               owl:Restriction ;
                           owl:hasValue    units:kilogram ;
                           owl:onProperty  screla:hasDefaultUnit
                         ] .

conc:MaterialProperty
        a                owl:Class ;
        rdfs:subClassOf  prop:PhysicalProperty .

conc:MassConcentration
        a                    owl:Class ;
        owl:equivalentClass  conc:Density .
