@base          <http://sweetontology.net/propRotation> .
@prefix mrela: <http://sweetontology.net/relaMath/> .
@prefix quan:  <http://sweetontology.net/propQuantity/> .
@prefix owl:   <http://www.w3.org/2002/07/owl#> .
@prefix dyna:  <http://sweetontology.net/propSpeed/> .
@prefix freq:  <http://sweetontology.net/propTimeFrequency/> .
@prefix xsd:   <http://www.w3.org/2001/XMLSchema#> .
@prefix rdfs:  <http://www.w3.org/2000/01/rdf-schema#> .
@prefix units: <http://sweetontology.net/reprSciUnits/> .
@prefix func:  <http://sweetontology.net/reprMathFunction/> .
@prefix rdf:   <http://www.w3.org/1999/02/22-rdf-syntax-ns#> .
@prefix rot:   <http://sweetontology.net/propRotation/> .
@prefix prop:  <http://sweetontology.net/prop/> .
@prefix oper:  <http://sweetontology.net/reprMathOperation/> .
@prefix screla: <http://sweetontology.net/relaSci/> .

rot:CoriolisParameter
        a                owl:Class ;
        rdfs:subClassOf  quan:PhysicalConstant , freq:Frequency .

rot:AbsoluteVorticity
        a                owl:Class ;
        rdfs:label       "Absolute Vorticity" ;
        rdfs:subClassOf  rot:Vorticity .

rot:MomentOfInertia  a   owl:Class ;
        rdfs:subClassOf  quan:PhysicalQuantity , prop:AngularMotionProperty .

rot:Helicity  a          owl:Class ;
        rdfs:subClassOf  oper:VectorFieldOperation ;
        rdfs:subClassOf  [ a               owl:Restriction ;
                           owl:hasValue    units:meterPerSecondSquared ;
                           owl:onProperty  screla:hasDefaultUnit
                         ] .

rot:ErtelPotentialVorticity
        a                owl:Class ;
        rdfs:subClassOf  rot:PotentialVorticity ;
        rdfs:subClassOf  [ a               owl:Restriction ;
                           owl:hasValue    units:perKilogramMeterSquaredPerSecondKelvin ;
                           owl:onProperty  screla:hasDefaultUnit
                         ] .

rot:Torque  a            owl:Class ;
        rdfs:subClassOf  quan:VectorQuantity , prop:AngularMotionProperty ;
        rdfs:subClassOf  [ a               owl:Restriction ;
                           owl:hasValue    units:newtonMeter ;
                           owl:onProperty  screla:hasDefaultUnit
                         ] .

rot:AngularVelocity  a   owl:Class ;
        rdfs:subClassOf  quan:VectorQuantity , prop:AngularMotionProperty ;
        rdfs:subClassOf  [ a               owl:Restriction ;
                           owl:hasValue    units:radianPerSecond ;
                           owl:onProperty  screla:hasDefaultUnit
                         ] .

rot:Circulation  a       owl:Class ;
        rdfs:subClassOf  oper:LineIntegral ;
        rdfs:subClassOf  [ a                  owl:Restriction ;
                           owl:allValuesFrom  func:VectorField ;
                           owl:onProperty     mrela:hasInput
                         ] .

rot:RelativeVorticity
        a                owl:Class ;
        rdfs:comment     "The vorticity as measured in a system of coordinates fixed on the earth's surface.  Usually, only the vertical component of the vorticity is meant."@en ;
        rdfs:subClassOf  rot:Vorticity .

rot:Enstrophy  a         owl:Class ;
        rdfs:subClassOf  quan:PhysicalQuantity , prop:AngularMotionProperty .

rot:Curl  a              owl:Class ;
        rdfs:subClassOf  oper:VectorFieldOperation ;
        rdfs:subClassOf  [ a                  owl:Restriction ;
                           owl:allValuesFrom  func:VectorField ;
                           owl:onProperty     mrela:hasOutput
                         ] .

rot:Vorticity  a         owl:Class ;
        rdfs:subClassOf  oper:VectorFieldOperation ;
        rdfs:subClassOf  [ a               owl:Restriction ;
                           owl:hasValue    units:perSecond ;
                           owl:onProperty  screla:hasDefaultUnit
                         ] .

rot:AngularMomentum  a   owl:Class ;
        rdfs:comment     "In physics, the angular momentum of an object rotating about some reference point is the measure of the extent to which the object will continue to rotate about that point unless acted upon by an external torque. In particular, if a point mass rotates about an axis, then the angular momentum with respect to a point on the axis is related to the mass of the object, the velocity and the distance of the mass to the axis. While the motion associated with linear momentum has no absolute frame of reference, the rotation associated with angular momentum is sometimes spoken of as being measured relative to the fixed stars."@en ;
        rdfs:subClassOf  dyna:Momentum ;
        rdfs:subClassOf  [ a               owl:Restriction ;
                           owl:hasValue    units:kilogramRadianPerSecond ;
                           owl:onProperty  screla:hasDefaultUnit
                         ] .

rot:AngularAcceleration
        a                owl:Class ;
        rdfs:subClassOf  quan:VectorQuantity , prop:AngularMotionProperty ;
        rdfs:subClassOf  [ a               owl:Restriction ;
                           owl:hasValue    units:radianPerSecondSquared ;
                           owl:onProperty  screla:hasDefaultUnit
                         ] .

rot:Gyrofrequency  a         owl:Class ;
        rdfs:subClassOf      freq:Frequency ;
        owl:equivalentClass  rot:CyclotronFrequency .

rot:Spin  a              owl:Class ;
        rdfs:subClassOf  prop:AngularMotionProperty .

<>      a                owl:Ontology ;
        rdfs:label       "SWEET Ontology" ;
        owl:imports      <propTimeFrequency> , <propSpeed> , <reprMathOperation> , <relaSci> , <propQuantity> , <reprSciUnits> , <relaMath> , <reprMathFunction> , <prop> ;
        owl:versionInfo  "3.1.0" .

rot:PotentialVorticity
        a                owl:Class ;
        rdfs:comment     "The vertically averaged vorticity of a layer divided by layer thickness."@en ;
        rdfs:subClassOf  quan:PhysicalQuantity , prop:AngularMotionProperty .

rot:CyclotronFrequency
        a       owl:Class .
