@base          <http://sweetontology.net/propMassFlux> .
@prefix crela: <http://sweetontology.net/relaChemical/> .
@prefix quan:  <http://sweetontology.net/propQuantity/> .
@prefix rdf:   <http://www.w3.org/1999/02/22-rdf-syntax-ns#> .
@prefix owl:   <http://www.w3.org/2002/07/owl#> .
@prefix mflux: <http://sweetontology.net/propMassFlux/> .
@prefix mass:  <http://sweetontology.net/propMass/> .
@prefix xsd:   <http://www.w3.org/2001/XMLSchema#> .
@prefix rdfs:  <http://www.w3.org/2000/01/rdf-schema#> .

mflux:NetPrimaryProductivity
        a                    owl:Class ;
        rdfs:subClassOf      mflux:PrimaryProductivity ;
        owl:equivalentClass  mflux:NPP .

mflux:DarcyFlux  a       owl:Class ;
        rdfs:subClassOf  mflux:MassFlux .

<>      a                owl:Ontology ;
        rdfs:label       "SWEET Ontology" ;
        owl:imports      <propQuantity> , <relaChemical> , <propMass> ;
        owl:versionInfo  "3.1.0" .

mflux:DifferentialFlux
        a                owl:Class ;
        rdfs:subClassOf  mflux:MassFlux .

mflux:PermeabilityCoefficent
        a                owl:Class ;
        rdfs:comment     "The rate of flow of water through a unit cross-sectional area under a unit hydraulic gradient at the prevailing temperature (field permeability coefficient) or adjusted to a temperature of 150C (60-F)."@en ;
        rdfs:subClassOf  mflux:Permeability .

mflux:Productivity  a    owl:Class ;
        rdfs:subClassOf  mflux:MassFlux .

mflux:MassFlux  a        owl:Class ;
        rdfs:subClassOf  quan:Flux ;
        rdfs:subClassOf  [ a                  owl:Restriction ;
                           owl:allValuesFrom  mass:Mass ;
                           owl:onProperty     crela:hasSubstance
                         ] .

mflux:SpecificDischarge
        a                owl:Class ;
        rdfs:comment     "The rate of discharge of groundwater per unit area of a porous medium measured at right angle to the direction of flow."@en ;
        rdfs:subClassOf  mflux:MassFlux .

mflux:SpecificCapacity
        a                owl:Class ;
        rdfs:comment     "The rate of discharge of water from the well divided by the drawdown of the water level within the well."@en ;
        rdfs:subClassOf  mflux:MassFlux .

mflux:PrimaryProductivity
        a                owl:Class ;
        rdfs:subClassOf  mflux:Productivity .

mflux:GrossPrimaryProductivity
        a                    owl:Class ;
        rdfs:subClassOf      mflux:PrimaryProductivity ;
        owl:equivalentClass  mflux:GPP .

mflux:SpecificPermeability
        a                owl:Class ;
        rdfs:comment     "The permeability measured when the rock contains only one fluid."@en ;
        rdfs:subClassOf  mflux:Permeability .

mflux:Permeability  a    owl:Class ;
        rdfs:subClassOf  mflux:MassFlux .

mflux:IntrinsicPermeability
        a                owl:Class ;
        rdfs:comment     "A measure of the relative ease with which a porous medium can transmit a fluid under a potential gradient and is a property of the medium alone (after Lohman and others, 1972). The property of a porous medium itself that expresses the ease with which gases, liquids, or other substances can pass through it."@en ;
        rdfs:subClassOf  mflux:Permeability .

mflux:EffectivePermeability
        a                owl:Class ;
        rdfs:comment     "The observed permeability of a porous medium to one fluid phase under conditions of physical interaction between this phase and other fluid phases present."@en ;
        rdfs:subClassOf  mflux:Permeability .

mflux:GPP  a    owl:Class .

mflux:NPP  a    owl:Class .
