@base          <http://sweetontology.net/propDiffusivity> .
@prefix proc:  <http://sweetontology.net/procPhysical/> .
@prefix func:  <http://sweetontology.net/reprMathFunction/> .
@prefix quan:  <http://sweetontology.net/propQuantity/> .
@prefix rate:  <http://sweetontology.net/propTimeFrequency/> .
@prefix rdf:   <http://www.w3.org/1999/02/22-rdf-syntax-ns#> .
@prefix owl:   <http://www.w3.org/2002/07/owl#> .
@prefix xsd:   <http://www.w3.org/2001/XMLSchema#> .
@prefix diff:  <http://sweetontology.net/propDiffusivity/> .
@prefix rdfs:  <http://www.w3.org/2000/01/rdf-schema#> .
@prefix units: <http://sweetontology.net/reprSciUnits/> .
@prefix screla: <http://sweetontology.net/relaSci/> .
@prefix rela:  <http://sweetontology.net/rela/> .
@prefix wave:  <http://sweetontology.net/phenFluidDynamics/> .

diff:Transmissivity  a   owl:Class ;
        rdfs:subClassOf  diff:DiffusivityQuantity .

<>      a                owl:Ontology ;
        rdfs:label       "SWEET Ontology" ;
        owl:imports      <propQuantity> , <rela> , <relaSci> , <reprSciUnits> , <phenFluidDynamics> , <procPhysical> , <propTimeFrequency> , <reprMathFunction> ;
        owl:versionInfo  "3.1.0" .

diff:ThermalDiffusivity
        a                owl:Class ;
        rdfs:subClassOf  quan:ThermodynamicQuantity , diff:Diffusivity .

diff:Confluence  a       owl:Class ;
        rdfs:comment     "The rate at which adjacent flow is converging along an axis oriented normal to the flow at the point in question."@en ;
        rdfs:subClassOf  diff:DiffusivityQuantity ;
        rdfs:subClassOf  [ a                   owl:Restriction ;
                           owl:onProperty      rela:hasPhenomena ;
                           owl:someValuesFrom  rate:Convergence
                         ] .

diff:DiffusivityQuantity
        a                owl:Class ;
        rdfs:subClassOf  quan:PhysicalQuantity ;
        rdfs:subClassOf  [ a               owl:Restriction ;
                           owl:hasValue    units:meterSquaredPerSecond ;
                           owl:onProperty  screla:hasDefaultUnit
                         ] .

diff:VelocityPotential
        a                owl:Class ;
        rdfs:subClassOf  func:VectorQuantity , diff:DiffusivityQuantity .

diff:KinematicViscosity
        a                owl:Class ;
        rdfs:subClassOf  diff:DiffusivityQuantity ;
        rdfs:subClassOf  [ a                  owl:Restriction ;
                           owl:allValuesFrom  proc:ViscousForce ;
                           owl:onProperty     screla:measureOf
                         ] .

diff:Diffluence  a       owl:Class ;
        rdfs:comment     "The rate at which adjacent flow diverges along an axis oriented normal to the flow at the point in question; the opposite of confluence."@en ;
        rdfs:subClassOf  diff:DiffusivityQuantity ;
        rdfs:subClassOf  [ a                   owl:Restriction ;
                           owl:onProperty      rela:hasPhenomena ;
                           owl:someValuesFrom  rate:Divergence
                         ] .

diff:Diffusivity  a      owl:Class ;
        rdfs:subClassOf  diff:DiffusivityQuantity .

diff:MeridionalOvertuningStreamfunction
        a                owl:Class ;
        rdfs:subClassOf  diff:Streamfunction .

diff:Streamfunction  a   owl:Class ;
        rdfs:subClassOf  func:VectorQuantity ;
        rdfs:subClassOf  [ a               owl:Restriction ;
                           owl:hasValue    units:meterCubedPerSecond ;
                           owl:onProperty  screla:hasDefaultUnit
                         ] .

diff:EddyDiffusivity  a  owl:Class ;
        rdfs:comment     "The exchange coefficient for the diffusion of a conservative property by eddies in a turbulent flow."@en ;
        rdfs:subClassOf  diff:Diffusivity ;
        rdfs:subClassOf  [ a                   owl:Restriction ;
                           owl:onProperty      rela:hasPhenomena ;
                           owl:someValuesFrom  wave:Eddy
                         ] .
