@base          <http://sweetontology.net/propEnergy> .
@prefix mrela: <http://sweetontology.net/relaMath/> .
@prefix mult:  <http://sweetontology.net/propSpaceMultidimensional/> .
@prefix quan:  <http://sweetontology.net/propQuantity/> .
@prefix owl:   <http://www.w3.org/2002/07/owl#> .
@prefix phys:  <http://sweetontology.net/procPhysical/> .
@prefix prela: <http://sweetontology.net/relaPhysical/> .
@prefix mass:  <http://sweetontology.net/propMass/> .
@prefix xsd:   <http://www.w3.org/2001/XMLSchema#> .
@prefix rdfs:  <http://www.w3.org/2000/01/rdf-schema#> .
@prefix units: <http://sweetontology.net/reprSciUnits/> .
@prefix rdf:   <http://www.w3.org/1999/02/22-rdf-syntax-ns#> .
@prefix prop:  <http://sweetontology.net/prop/> .
@prefix ener:  <http://sweetontology.net/propEnergy/> .
@prefix oper:  <http://sweetontology.net/reprMathOperation/> .
@prefix time:  <http://sweetontology.net/reprTime/> .
@prefix rela:  <http://sweetontology.net/rela/> .
@prefix screla: <http://sweetontology.net/relaSci/> .
@prefix statec: <http://sweetontology.net/procStateChange/> .

ener:SpecificPotentialEnergy
        a                owl:Class ;
        rdfs:subClassOf  ener:SpecificEnergy ;
        rdfs:subClassOf  [ a                  owl:Restriction ;
                           owl:allValuesFrom  ener:PotentialEnergy ;
                           owl:onProperty     mrela:hasFirstOperand
                         ] .

ener:LatentHeat  a       owl:Class ;
        rdfs:subClassOf  ener:Heat .

ener:KineticEnergy  a    owl:Class ;
        rdfs:subClassOf  prop:MotionProperty , ener:Energy .

ener:Heat  a                 owl:Class ;
        rdfs:subClassOf      quan:ThermodynamicQuantity , ener:Energy ;
        owl:equivalentClass  ener:ThermalEnergy , ener:HeatEnergy .

ener:Energy  a           owl:Class ;
        rdfs:subClassOf  quan:ExtensiveProperty ;
        rdfs:subClassOf  [ a               owl:Restriction ;
                           owl:hasValue    units:joule ;
                           owl:onProperty  screla:hasDefaultUnit
                         ] .

ener:TotalSoilWaterPotential
        a                owl:Class ;
        rdfs:comment     "The sum of the energy-related components of a soil-water system; i.e., the sum of the gravitational, matric, and osmotic components."@en ;
        rdfs:subClassOf  prop:HydrogeologicalProperty .

ener:EnergyBudget  a     owl:Class ;
        rdfs:subClassOf  quan:Budget ;
        rdfs:subClassOf  [ a                  owl:Restriction ;
                           owl:allValuesFrom  ener:Energy ;
                           owl:onProperty     rela:hasProperty
                         ] .

ener:Work  a             owl:Class ;
        rdfs:comment     "A form of energy arising from the motion of a system against a force, existing only in the process of energy conversion."@en ;
        rdfs:subClassOf  ener:Energy .

<>      a                owl:Ontology ;
        rdfs:label       "SWEET Ontology" ;
        owl:imports      <reprTime> , <reprMathOperation> , <reprSciUnits> , <relaMath> , <relaSci> , <relaPhysical> , <propSpaceMultidimensional> , <procStateChange> , <propQuantity> , <prop> , <rela> , <propMass> , <procPhysical> ;
        owl:versionInfo  "3.1.0" .

ener:BindingEnergy  a    owl:Class ;
        rdfs:subClassOf  ener:ChemicalEnergy , ener:PotentialEnergy .

ener:ChemicalEnergy  a   owl:Class ;
        rdfs:subClassOf  prop:ChemicalProperty , ener:Energy .

ener:RadiantEnergy  a    owl:Class ;
        rdfs:comment     "Infrequently, any energy propagated by a physical quantity governed by a wave equation."@en ;
        rdfs:subClassOf  ener:Energy ;
        rdfs:subClassOf  [ a                  owl:Restriction ;
                           owl:allValuesFrom  phys:Radiation ;
                           owl:onProperty     rela:hasProcess
                         ] .

ener:Lagrangian  a       owl:Class ;
        rdfs:subClassOf  ener:Energy .

ener:IonizationEnergy
        a                    owl:Class ;
        rdfs:subClassOf      ener:ChemicalEnergy , ener:PotentialEnergy ;
        owl:equivalentClass  ener:IonizationPotential .

ener:Power  a            owl:Class ;
        rdfs:subClassOf  oper:Ratio , quan:ExtensiveProperty ;
        rdfs:subClassOf  [ a               owl:Restriction ;
                           owl:hasValue    units:watt ;
                           owl:onProperty  screla:hasDefaultUnit
                         ] ;
        rdfs:subClassOf  [ a                  owl:Restriction ;
                           owl:allValuesFrom  time:Time ;
                           owl:onProperty     mrela:hasSecondOperand
                         ] ;
        rdfs:subClassOf  [ a                  owl:Restriction ;
                           owl:allValuesFrom  ener:Energy ;
                           owl:onProperty     mrela:hasFirstOperand
                         ] .

ener:SpecificEnergy  a   owl:Class ;
        rdfs:subClassOf  oper:Ratio , quan:IntensiveProperty ;
        rdfs:subClassOf  [ a               owl:Restriction ;
                           owl:hasValue    units:joulePerKilogram ;
                           owl:onProperty  screla:hasDefaultUnit
                         ] ;
        rdfs:subClassOf  [ a                  owl:Restriction ;
                           owl:allValuesFrom  mass:Mass ;
                           owl:onProperty     mrela:hasSecondOperand
                         ] ;
        rdfs:subClassOf  [ a                  owl:Restriction ;
                           owl:allValuesFrom  ener:Energy ;
                           owl:onProperty     mrela:hasFirstOperand
                         ] .

ener:SensibleHeat  a     owl:Class ;
        rdfs:subClassOf  ener:Heat .

ener:ConvectiveInhibition
        a                owl:Class ;
        rdfs:comment     "The energy needed to lift an air parcel vertically and pseudoadiabatically from its originating level to its level of free convection (LFC)."@en ;
        rdfs:subClassOf  ener:Energy .

ener:EvaporativeAvailablePotentialEnergy
        a                owl:Class ;
        rdfs:comment     "Analogous to convective available potential energy, except that it is related to the negative buoyancy associated with evaporative cooling of liquid water within a sinking cloudy air parcel."@en ;
        rdfs:subClassOf  ener:AvailablePotentialEnergy ;
        rdfs:subClassOf  [ a                  owl:Restriction ;
                           owl:allValuesFrom  statec:Evaporation ;
                           owl:onProperty     prela:hasStateChange
                         ] .

ener:HeatBudget  a       owl:Class ;
        rdfs:subClassOf  ener:EnergyBudget ;
        rdfs:subClassOf  [ a                  owl:Restriction ;
                           owl:allValuesFrom  ener:Heat ;
                           owl:onProperty     rela:hasProperty
                         ] .

ener:GravitationalPotential
        a                owl:Class ;
        rdfs:subClassOf  quan:ScalarPotential ;
        rdfs:subClassOf  [ a               owl:Restriction ;
                           owl:hasValue    units:meterSquaredPerSecondSquared ;
                           owl:onProperty  screla:hasDefaultUnit
                         ] ;
        rdfs:subClassOf  [ a                  owl:Restriction ;
                           owl:allValuesFrom  phys:Gravity ;
                           owl:onProperty     rela:hasProcess
                         ] .

ener:Enthalpy  a         owl:Class ;
        rdfs:subClassOf  ener:ChemicalEnergy .

ener:HeatEnergy  a  owl:Class .

ener:IonizationPotential
        a       owl:Class .

ener:Luminosity  a       owl:Class ;
        rdfs:subClassOf  ener:Power , quan:ElectromagneticRadiationQuantity .

ener:AvailablePotentialEnergy
        a                owl:Class ;
        rdfs:comment     "That portion of the total potential energy that may be converted to kinetic energy in an adiabatically enclosed system."@en ;
        rdfs:subClassOf  ener:PotentialEnergy .

ener:InternalEnergy  a   owl:Class ;
        rdfs:subClassOf  ener:Energy .

ener:ThermochemicalEnergy
        a                owl:Class ;
        rdfs:subClassOf  ener:ChemicalEnergy .

ener:GibbsFreeEnergy  a  owl:Class ;
        rdfs:subClassOf  ener:ChemicalEnergy .

ener:Entropy  a          owl:Class ;
        rdfs:subClassOf  ener:Energy .

ener:PotentialEnergy  a  owl:Class ;
        rdfs:subClassOf  ener:Energy .

ener:ThermalEnergy  a  owl:Class .

ener:EnergyDensity  a    owl:Class ;
        rdfs:comment     "Energy per unit area."@en ;
        rdfs:subClassOf  oper:Ratio , quan:IntensiveProperty ;
        rdfs:subClassOf  [ a                  owl:Restriction ;
                           owl:allValuesFrom  mult:Area ;
                           owl:onProperty     mrela:hasSecondOperand
                         ] ;
        rdfs:subClassOf  [ a                  owl:Restriction ;
                           owl:allValuesFrom  ener:Energy ;
                           owl:onProperty     mrela:hasFirstOperand
                         ] ;
        rdfs:subClassOf  [ a               owl:Restriction ;
                           owl:hasValue    units:joulePerMeterSquared ;
                           owl:onProperty  screla:hasDefaultUnit
                         ] .

ener:Hamiltonian  a      owl:Class ;
        rdfs:subClassOf  ener:Energy .

ener:MatricPotential  a  owl:Class ;
        rdfs:comment     "The energy required to extract water from a porous medium to overcome the capillary and adsorptive forces."@en ;
        rdfs:subClassOf  ener:Energy , mass:ConsistenceProperty .

ener:Geopotential  a     owl:Class ;
        rdfs:subClassOf  ener:GravitationalPotential .
