@base          <http://sweetontology.net/propEnergyFlux> .
@prefix repr:  <http://sweetontology.net/repr/> .
@prefix star:  <http://sweetontology.net/phenStar/> .
@prefix quan:  <http://sweetontology.net/propQuantity/> .
@prefix owl:   <http://www.w3.org/2002/07/owl#> .
@prefix prela: <http://sweetontology.net/relaPhysical/> .
@prefix screla2: <http://sweetontology.net/relaSci/> .
@prefix xsd:   <http://www.w3.org/2001/XMLSchema#> .
@prefix seis:  <http://sweetontology.net/phenGeolSeismicity/> .
@prefix rdfs:  <http://www.w3.org/2000/01/rdf-schema#> .
@prefix units: <http://sweetontology.net/reprSciUnits/> .
@prefix eflux: <http://sweetontology.net/propEnergyFlux/> .
@prefix rdf:   <http://www.w3.org/1999/02/22-rdf-syntax-ns#> .
@prefix rela:  <http://sweetontology.net/rela/> .
@prefix screla: <http://sweetontology.net/relaSci/> .
@prefix energy: <http://sweetontology.net/propEnergy/> .

eflux:LuminousFlux  a    owl:Class ;
        rdfs:subClassOf  eflux:EnergyFlux ;
        rdfs:subClassOf  [ a               owl:Restriction ;
                           owl:hasValue    units:lumen ;
                           owl:onProperty  screla:hasDefaultUnit
                         ] .

eflux:FluxDensity  a         owl:Class ;
        rdfs:subClassOf      quan:Flux ;
        rdfs:subClassOf      [ a               owl:Restriction ;
                               owl:hasValue    units:wattPerMeterSquared ;
                               owl:onProperty  screla:hasDefaultUnit
                             ] ;
        owl:equivalentClass  eflux:Intensity .

eflux:RadiativeForcing
        a                owl:Class ;
        rdfs:comment     "In radiation, the net flux of radiation into or out of a system.  As a consequence of radiative forcing there must be some change to the nonradiative energy states of the system."@en ;
        rdfs:subClassOf  eflux:RadiantFlux , eflux:FluxDensity .

eflux:Insolation  a      owl:Class ;
        rdfs:subClassOf  eflux:SolarRadiation .

eflux:AbsorbedSolarRadiation
        a                owl:Class ;
        rdfs:comment     "Solar radiation absorbed by the atmosphere's constituent gases, suspended material, clouds, or by the earth's surface." ;
        rdfs:label       "Absorbed Solar Radiation" ;
        rdfs:subClassOf  eflux:SolarRadiation .

eflux:AbsorptionCoefficient
        a       owl:Class .

eflux:EnergyFlux_Wm2  a  owl:Class ;
        rdfs:subClassOf  eflux:EnergyFlux ;
        rdfs:subClassOf  [ a               owl:Restriction ;
                           owl:hasValue    units:wattPerMeterSquared ;
                           owl:onProperty  screla:hasUnit
                         ] .

eflux:ThermalFlux  a         owl:Class ;
        rdfs:subClassOf      quan:ThermodynamicQuantity , eflux:EnergyFlux ;
        owl:equivalentClass  eflux:HeatFlow , eflux:HeatFlux .

eflux:SolarFlux  a       owl:Class ;
        rdfs:subClassOf  eflux:RadiativeFlux .

eflux:TerrestrialRadiation
        a                owl:Class ;
        rdfs:comment     "Longwave radiation originating by thermal emission from a planetary surface and/or its atmosphere"@en ;
        rdfs:subClassOf  eflux:RadiativeFlux .

eflux:HeatFlow  a  owl:Class .

eflux:Irradiance  a      owl:Class ;
        rdfs:subClassOf  eflux:FluxDensity , quan:ElectromagneticRadiationQuantity .

eflux:Brightness  a          owl:Class ;
        rdfs:subClassOf      eflux:Luminance ;
        rdfs:subClassOf      [ a               owl:Restriction ;
                               owl:hasValue    units:wattPerMeterSquaredPerSteradianPerWavelength ;
                               owl:onProperty  screla:hasDefaultUnit
                             ] ;
        owl:equivalentClass  eflux:SpecificIntensity .

eflux:SolarForcing  a    owl:Class ;
        rdfs:subClassOf  eflux:RadiativeForcing .

eflux:Radiance  a        owl:Class ;
        rdfs:comment     "A radiometric term for the rate at which radiant energy in a set of directions confined to a unit solid angle around a particular direction is transferred across unit area of a surface (real or imaginary) projected onto this direction."@en ;
        rdfs:subClassOf  quan:ElectromagneticRadiationQuantity ;
        rdfs:subClassOf  [ a               owl:Restriction ;
                           owl:hasValue    units:wattPerMeterSquaredPerSteradian ;
                           owl:onProperty  screla:hasDefaultUnit
                         ] .

eflux:HeatFlux  a  owl:Class .

eflux:PoyntingVector  a  owl:Class ;
        rdfs:subClassOf  eflux:FluxDensity .

eflux:SolarConstant  a    quan:PhysicalConstant , eflux:RadiativeFlux ;
        screla:hasSource  star:Sun .

eflux:RichterScale  a    owl:Class ;
        rdfs:subClassOf  eflux:EarthquakeScale .

eflux:Illuminance  a     owl:Class ;
        rdfs:subClassOf  eflux:EnergyFlux ;
        rdfs:subClassOf  [ a               owl:Restriction ;
                           owl:hasValue    units:lux ;
                           owl:onProperty  screla:hasDefaultUnit
                         ] .

eflux:SolarRadiation  a  owl:Class ;
        rdfs:comment     "The total electromagnetic radiation emitted by the sun."@en ;
        rdfs:subClassOf  quan:ElectromagneticRadiationQuantity .

<>      a                owl:Ontology ;
        rdfs:label       "SWEET Ontology" ;
        owl:imports      <propQuantity> , <relaPhysical> , <reprSciUnits> , <relaSci> , <repr> , <rela> , <phenStar> , <propEnergy> , <phenGeolSeismicity> ;
        owl:versionInfo  "3.1.0" .

eflux:BulkHeatFlux  a    owl:Class ;
        rdfs:comment     "Heat flux averaged over a layer of air, such as the boundary layer; heat-flux divergence or difference between the top and bottom of a layer." ;
        rdfs:subClassOf  eflux:ThermalFlux .

eflux:EnergyFlux  a      owl:Class ;
        rdfs:subClassOf  quan:Flux ;
        rdfs:subClassOf  [ a                   owl:Restriction ;
                           owl:onProperty      prela:transportOf ;
                           owl:someValuesFrom  energy:Energy
                         ] .

eflux:Intensity  a  owl:Class .

eflux:Opacity  a             owl:Class ;
        rdfs:comment         "The extinction coefficient for a particular substance is a measure of how well it scatters and absorbs electromagnetic radiation (EM waves). If the EM wave can pass through very easily, the material has a low extinction coefficient. Conversely, if the radiation hardly penetrates the material, but rather quickly becomes extinct within it, the extinction coefficient is high." ;
        rdfs:subClassOf      quan:RadiationMediumInteractionQuantity ;
        rdfs:subClassOf      [ a               owl:Restriction ;
                               owl:hasValue    units:meterSquaredPerKilogram ;
                               owl:onProperty  screla:hasDefaultUnit
                             ] ;
        owl:equivalentClass  eflux:AbsorptionCoefficient .

eflux:Luminance  a       owl:Class ;
        rdfs:subClassOf  quan:ElectromagneticRadiationQuantity ;
        rdfs:subClassOf  [ a               owl:Restriction ;
                           owl:hasValue    units:candelaPerMeterSquared ;
                           owl:onProperty  screla:hasDefaultUnit
                         ] .

eflux:CloudForcing  a    owl:Class ;
        rdfs:subClassOf  eflux:RadiativeForcing .

eflux:EarthquakeScale
        a                owl:Class ;
        rdfs:subClassOf  repr:LogarithmicScale ;
        rdfs:subClassOf  [ a               owl:Restriction ;
                           owl:hasValue    units:db ;
                           owl:onProperty  screla:hasUnit
                         ] ;
        rdfs:subClassOf  [ a                  owl:Restriction ;
                           owl:allValuesFrom  seis:Earthquake ;
                           owl:onProperty     rela:hasPhenomena
                         ] .

eflux:LuminousIntensity
        a                owl:Class ;
        rdfs:subClassOf  quan:ElectromagneticRadiationQuantity ;
        rdfs:subClassOf  [ a               owl:Restriction ;
                           owl:hasValue    units:candela ;
                           owl:onProperty  screla:hasDefaultUnit
                         ] .

eflux:RadiativeFlux  a   owl:Class ;
        rdfs:subClassOf  eflux:EnergyFlux , eflux:RadiativeForcing .

eflux:RadiantFlux  a     owl:Class ;
        rdfs:comment     "Radiant energy per unit time passing some specified area from one side."@en ;
        rdfs:subClassOf  eflux:RadiativeForcing .

eflux:SpecificIntensity
        a       owl:Class .

eflux:SpectralRadiance
        a                owl:Class ;
        rdfs:comment     "The radiance per unit wavelength or wavenumber interval."@en ;
        rdfs:subClassOf  eflux:Radiance .
