@base          <http://sweetontology.net/propIndex> .
@prefix proc:  <http://sweetontology.net/proc/> .
@prefix clim:  <http://sweetontology.net/phenPlanetClimate/> .
@prefix role:  <http://sweetontology.net/stateRoleRepresentative/> .
@prefix quan:  <http://sweetontology.net/propQuantity/> .
@prefix owlt:  <http://www.w3.org/2006/time#> .
@prefix owl:   <http://www.w3.org/2002/07/owl#> .
@prefix xsd:   <http://www.w3.org/2001/XMLSchema#> .
@prefix rdfs:  <http://www.w3.org/2000/01/rdf-schema#> .
@prefix units: <http://sweetontology.net/reprSciUnits/> .
@prefix rdf:   <http://www.w3.org/1999/02/22-rdf-syntax-ns#> .
@prefix inst:  <http://sweetontology.net/phenFluidInstability/> .
@prefix prop:  <http://sweetontology.net/prop/> .
@prefix realm: <http://sweetontology.net/realm/> .
@prefix indi:  <http://sweetontology.net/propIndex/> .
@prefix screla: <http://sweetontology.net/relaSci/> .
@prefix rela:  <http://sweetontology.net/rela/> .
@prefix osc:   <http://sweetontology.net/phenCycle/> .
@prefix trans: <http://sweetontology.net/phenFluidTransport/> .
@prefix therm: <http://sweetontology.net/propTemperature/> .

indi:AuroralBoundaryIndex
        a                owl:Class ;
        rdfs:subClassOf  indi:GeomagneticIndex .

indi:EnvironmentalSustainabilityIndex
        a                    owl:Class ;
        rdfs:subClassOf      indi:EnvironmentalIndex ;
        owl:equivalentClass  indi:ESI .

indi:CoefficientOfHaze
        a                    owl:Class ;
        rdfs:subClassOf      indi:AirQualityIndex ;
        owl:equivalentClass  indi:COH .

indi:ForestFireDangerIndex
        a                owl:Class ;
        rdfs:subClassOf  indi:EnvironmentalIndex .

indi:EnvironmentalIndex
        a                owl:Class ;
        rdfs:subClassOf  indi:Index .

indi:EPI  a     owl:Class .

indi:BlockingIndex  a    owl:Class ;
        rdfs:subClassOf  indi:Index .

indi:CirculationIndex
        a                owl:Class ;
        rdfs:subClassOf  indi:Index .

indi:PHDI  a    owl:Class .

indi:KaplanSSTIndex  a   owl:Class ;
        rdfs:subClassOf  indi:Index ;
        rdfs:subClassOf  [ a                  owl:Restriction ;
                           owl:allValuesFrom  therm:Temperature ;
                           owl:onProperty     screla:measureOf
                         ] .

indi:PDI  a     owl:Class .

indi:BenthicIndex  a         owl:Class ;
        rdfs:subClassOf      indi:IBI ;
        owl:equivalentClass  indi:BIBI , indi:BenthicIndexOfBiologicalIntegrity .

indi:PC  a      owl:Class .

indi:ShallowConvectionParameter
        a                owl:Class ;
        rdfs:comment     "The representation in a numerical model of the turbulent transports of heat and moisture by nonprecipitating cumulus clouds with cloud tops below 3000 m above the surface."@en ;
        rdfs:subClassOf  quan:PhysicalConstant , trans:Transport .

indi:ComputationalComplexity
        a                owl:Class ;
        rdfs:subClassOf  prop:Metric .

indi:WaterQualityIndex
        a                owl:Class ;
        rdfs:subClassOf  indi:EnvironmentalIndex .

indi:StandardizedPrecipitationIndex
        a                owl:Class ;
        rdfs:subClassOf  indi:DroughtIndex .

indi:IndexDefinedByDifference
        a                owl:Class ;
        rdfs:subClassOf  indi:Index .

indi:PalmerHydrologicalDroughtIndex
        a                    owl:Class ;
        rdfs:subClassOf      indi:DroughtIndex ;
        owl:equivalentClass  indi:PHDI .

indi:GeophysicalIndex
        a                    owl:Class ;
        owl:equivalentClass  indi:GeomagneticIndex .

indi:IndexOfBioticIntegrity
        a       owl:Class .

indi:NaturalResourceManagementIndex
        a                    owl:Class ;
        rdfs:subClassOf      indi:EnvironmentalIndex ;
        owl:equivalentClass  indi:NRMI .

indi:IBI  a     owl:Class .

indi:ClimateIndicator
        a                owl:Class ;
        rdfs:subClassOf  indi:EnvironmentalIndicator ;
        rdfs:subClassOf  [ a                  owl:Restriction ;
                           owl:allValuesFrom  clim:Climate ;
                           owl:onProperty     screla:measureOf
                         ] .

indi:AkasofuEpsilon  a       owl:Class ;
        owl:equivalentClass  indi:GeomagneticIndex .

indi:GeomagneticForce
        a                owl:Class ;
        rdfs:subClassOf  proc:Force .

indi:IndexOfBiologicalIntegrity
        a                    owl:Class ;
        rdfs:subClassOf      indi:EnvironmentalIndex ;
        owl:equivalentClass  indi:IndexOfBioticIntegrity , indi:IBI .

indi:AirQualityIndex  a  owl:Class ;
        rdfs:subClassOf  indi:EnvironmentalIndex .

indi:AdaptiveCapacity
        a                owl:Class ;
        rdfs:subClassOf  prop:Metric .

indi:Hydropattern  a     owl:Class ;
        rdfs:comment     "The full range of hydrologic parameters, which include the depth of water, duration of inundation, and the timing and distribution of freshwater flow." ;
        rdfs:subClassOf  indi:Index ;
        rdfs:subClassOf  [ a                  owl:Restriction ;
                           owl:allValuesFrom  realm:Hydrosphere ;
                           owl:onProperty     rela:hasRealm
                         ] .

indi:VitalStatistics  a  owl:Class ;
        rdfs:subClassOf  indi:HealthIndex .

indi:PDSI  a    owl:Class .

indi:FireWeatherIndex
        a                owl:Class ;
        rdfs:subClassOf  indi:EnvironmentalIndex .

indi:Kp  a               owl:Class ;
        rdfs:subClassOf  indi:GeomagneticIndex .

indi:PolarCapIndex  a        owl:Class ;
        rdfs:subClassOf      indi:GeomagneticIndex ;
        owl:equivalentClass  indi:PC .

indi:BIBI  a    owl:Class .

indi:DroughtIndex  a     owl:Class ;
        rdfs:subClassOf  indi:ClimateIndicator ;
        rdfs:subClassOf  [ a                  owl:Restriction ;
                           owl:allValuesFrom  clim:Drought ;
                           owl:onProperty     screla:measureOf
                         ] .

indi:CommonSenseClimateIndex
        a                owl:Class ;
        rdfs:comment     "The Common Sense Climate Index is a simple measure of the degree (if any) to which practical climate change is occurring. The index is a composite of several everyday climate indicators. It is expected to have positive values when warming occurs and negative values for cooling. If the Index reaches and consistently maintains a value of 1 or more, the climate change should be noticeable to most people who have lived at that location for a few decades." ;
        rdfs:subClassOf  indi:ClimateIndicator .

indi:SurfaceMoistureIndex
        a                    owl:Class ;
        rdfs:subClassOf      indi:DroughtIndex ;
        owl:equivalentClass  indi:SMI .

indi:BoydenIndex  a      owl:Class ;
        rdfs:comment     "A measure of the mean thermodynamic stability in a layer beneath 700 mb." ;
        rdfs:subClassOf  indi:Index ;
        rdfs:subClassOf  [ a                  owl:Restriction ;
                           owl:allValuesFrom  inst:StaticStability ;
                           owl:onProperty     screla:measureOf
                         ] .

indi:Virulence  a        owl:Class ;
        rdfs:subClassOf  indi:HealthIndex .

indi:GeomagneticIndex
        a                owl:Class ;
        rdfs:subClassOf  indi:Index ;
        rdfs:subClassOf  [ a                  owl:Restriction ;
                           owl:allValuesFrom  indi:GeomagneticForce ;
                           owl:onProperty     screla:measureOf
                         ] .

indi:Storativity  a  owl:Class .

indi:NorthAtlanticOscillationIndex
        a                owl:Class ;
        rdfs:subClassOf  indi:IndexDefinedByDifference ;
        rdfs:subClassOf  [ a                  owl:Restriction ;
                           owl:allValuesFrom  osc:NAO ;
                           owl:onProperty     screla:measureOf
                         ] .

indi:PhysiologicalParameter
        a                owl:Class ;
        rdfs:subClassOf  indi:HealthIndex .

indi:UVIndex  a          owl:Class ;
        rdfs:subClassOf  indi:AirQualityIndex .

indi:RingelmannChart  a  owl:Class ;
        rdfs:subClassOf  indi:AirQualityIndex .

indi:ESI  a     owl:Class .

indi:ZonalIndex  a       owl:Class ;
        rdfs:comment     "A measure of strength of the middle-latitude westerlies, usually expressed as the horizontal pressure difference between 35 and 55N latitude, or as the corresponding geostrophic wind."@en ;
        rdfs:subClassOf  indi:IndexDefinedByDifference .

indi:EnvironmentalPerformanceIndex
        a                    owl:Class ;
        rdfs:subClassOf      indi:EnvironmentalIndex ;
        owl:equivalentClass  indi:EPI .

indi:PsychologicalParameter
        a                owl:Class ;
        rdfs:subClassOf  indi:HealthIndex .

indi:COH  a     owl:Class .

indi:PalmerDroughtIndex
        a       owl:Class .

indi:NorthPacificOscillationIndex
        a                owl:Class ;
        rdfs:subClassOf  indi:IndexDefinedByDifference ;
        rdfs:subClassOf  [ a                  owl:Restriction ;
                           owl:allValuesFrom  osc:PDO ;
                           owl:onProperty     screla:measureOf
                         ] .

indi:StorageCoefficient
        a                    owl:Class ;
        rdfs:comment         "The volume of water an aquifer releases from or takes into storage per unit surface area of the aquifer per unit change in head (virtually equal to the specific yield in an unconfined aquifer)."@en ;
        rdfs:subClassOf      prop:HydrogeologicalProperty ;
        owl:equivalentClass  indi:Storativity .

indi:HealthIndex  a      owl:Class ;
        rdfs:subClassOf  prop:BiologicalProperty , indi:Index .

<>      a                owl:Ontology ;
        rdfs:label       "SWEET Ontology" ;
        owl:imports      <relaSci> , <propTemperature> , <rela> , <propQuantity> , <phenFluidTransport> , <prop> , <reprSciUnits> , <phenPlanetClimate> , <realm> , <phen> , <phenFluidInstability> , <phenCycle> , <proc> , <stateRoleRepresentative> ;
        owl:versionInfo  "3.1.0" .

indi:Turbidity  a        owl:Class ;
        rdfs:comment     "The effect of (primarily) aerosols, through their total optical depth, in reducing the transmission of direct solar radiation to the surface below that through a purely molecular atmosphere.\n    Turbidity is the cloudiness or haziness of a fluid, or of air, caused by individual particles (suspended solids) that are generally invisible to the naked eye, similar to smoke in air."@en ;
        rdfs:subClassOf  quan:RadiationMediumInteractionQuantity ;
        rdfs:subClassOf  [ a               owl:Restriction ;
                           owl:hasValue    units:FTU ;
                           owl:onProperty  screla:hasDefaultUnit
                         ] .

indi:NRMI  a    owl:Class .

indi:BenthicIndexOfBiologicalIntegrity
        a       owl:Class .

indi:Index  a            owl:Class ;
        rdfs:subClassOf  prop:Property .

indi:EnvironmentalIndicator
        a                owl:Class ;
        rdfs:subClassOf  indi:Index ;
        rdfs:subClassOf  [ a               owl:Restriction ;
                           owl:hasValue    role:Indicator ;
                           owl:onProperty  rela:hasRole
                         ] .

indi:PalmerDroughtSeverityIndex
        a                    owl:Class ;
        rdfs:subClassOf      indi:DroughtIndex ;
        owl:equivalentClass  indi:PDI , indi:PalmerDroughtIndex , indi:PDSI .

indi:CropMoistureIndex
        a                owl:Class ;
        rdfs:subClassOf  indi:HealthIndex .

indi:SMI  a     owl:Class .
