@base          <http://sweetontology.net/propTimeFrequency> .
@prefix mrela: <http://sweetontology.net/relaMath/> .
@prefix quan:  <http://sweetontology.net/propQuantity/> .
@prefix owl:   <http://www.w3.org/2002/07/owl#> .
@prefix xsd:   <http://www.w3.org/2001/XMLSchema#> .
@prefix rdfs:  <http://www.w3.org/2000/01/rdf-schema#> .
@prefix units: <http://sweetontology.net/reprSciUnits/> .
@prefix func:  <http://sweetontology.net/reprMathFunction/> .
@prefix rate:  <http://sweetontology.net/propTimeFrequency/> .
@prefix rdf:   <http://www.w3.org/1999/02/22-rdf-syntax-ns#> .
@prefix inst:  <http://sweetontology.net/phenFluidInstability/> .
@prefix prop:  <http://sweetontology.net/prop/> .
@prefix oper:  <http://sweetontology.net/reprMathOperation/> .
@prefix time:  <http://sweetontology.net/reprTime/> .
@prefix screla: <http://sweetontology.net/relaSci/> .

rate:FrequencyBand  a    owl:Class ;
        rdfs:subClassOf  quan:IntervalQuantity ;
        rdfs:subClassOf  [ a                  owl:Restriction ;
                           owl:allValuesFrom  rate:Frequency ;
                           owl:onProperty     screla:rangeOf
                         ] .

<>      a                owl:Ontology ;
        rdfs:label       "SWEET Ontology" ;
        owl:imports      <relaSci> , <reprMathFunction> , <relaMath> , <reprTime> , <reprSciUnits> , <propQuantity> , <phenFluidInstability> , <reprMathOperation> ;
        owl:versionInfo  "3.1.0" .

rate:Convergence  a      owl:Class ;
        rdfs:subClassOf  oper:VectorFieldOperation ;
        rdfs:subClassOf  [ a                  owl:Restriction ;
                           owl:allValuesFrom  func:VectorField ;
                           owl:onProperty     mrela:hasOutput
                         ] .

rate:FrequencyBand_MHz
        a                owl:Class ;
        rdfs:subClassOf  rate:FrequencyBand ;
        rdfs:subClassOf  [ a               owl:Restriction ;
                           owl:hasValue    units:MHz ;
                           owl:onProperty  screla:hasUnit
                         ] .

rate:BruntVaisalaFrequency
        a                owl:Class ;
        rdfs:comment     "The frequency at which a displaced parcel will oscillate when displaced vertically within a statically stable environment."@en ;
        rdfs:subClassOf  rate:Frequency ;
        rdfs:subClassOf  [ a                  owl:Restriction ;
                           owl:allValuesFrom  inst:StaticStability ;
                           owl:onProperty     screla:measureOf
                         ] .

rate:Bandwidth  a        owl:Class ;
        rdfs:subClassOf  rate:Frequency , prop:WaveProperty .

rate:Tendency  a  owl:Class .

rate:Incidence  a        owl:Class ;
        rdfs:subClassOf  rate:Frequency .

rate:Rate  a                 owl:Class ;
        rdfs:subClassOf      oper:PartialDerivative ;
        rdfs:subClassOf      [ a               owl:Restriction ;
                               owl:hasValue    units:perSecond ;
                               owl:onProperty  screla:hasDefaultUnit
                             ] ;
        rdfs:subClassOf      [ a                  owl:Restriction ;
                               owl:allValuesFrom  time:Time ;
                               owl:onProperty     mrela:derivativeWithRespectTo
                             ] ;
        owl:equivalentClass  rate:Tendency .

rate:Cadence  a          owl:Class ;
        rdfs:subClassOf  rate:Frequency .

rate:Divergence  a       owl:Class ;
        rdfs:comment     "The expansion or spreading out of a vector field; also, a precise measure thereof."@en ;
        rdfs:subClassOf  oper:VectorFieldOperation ;
        rdfs:subClassOf  [ a                  owl:Restriction ;
                           owl:allValuesFrom  func:ScalarField ;
                           owl:onProperty     mrela:hasInput
                         ] ;
        rdfs:subClassOf  [ a                  owl:Restriction ;
                           owl:allValuesFrom  func:VectorField ;
                           owl:onProperty     mrela:hasOutput
                         ] .

rate:Fertility  a        owl:Class ;
        rdfs:subClassOf  rate:Rate .

rate:Frequency  a        owl:Class ;
        rdfs:comment     "The rate of recurrence of any periodic phenomenon, often associated with waves of all kinds. Without qualification frequency often means temporal frequency, the rate of recurrence of a time-varying function, but could mean spatial frequency, the rate of recurrence of a space-varying function. Spatial frequency is the reciprocal of the repeat distance (sometimes the wavelength). The dimensions of (temporal) frequency are inverse time. A common unit for frequency is cycle per second, formerly abbreviated cps, but superseded by hertz, abbreviated as Hz."@en ;
        rdfs:subClassOf  quan:PhysicalQuantity , rate:Rate ;
        rdfs:subClassOf  [ a               owl:Restriction ;
                           owl:hasValue    units:hertz ;
                           owl:onProperty  screla:hasDefaultUnit
                         ] .

rate:SpreadingRate  a    owl:Class ;
        rdfs:comment     "The spreading rate is a measure of how fast plate divergence is occurring. [Wikipedia]"@en ;
        rdfs:subClassOf  rate:Rate .
