@base          <http://sweetontology.net/propTemperature> .
@prefix mrela: <http://sweetontology.net/relaMath/> .
@prefix tstate: <http://sweetontology.net/stateThermodynamic/> .
@prefix crela: <http://sweetontology.net/relaChemical/> .
@prefix quan:  <http://sweetontology.net/propQuantity/> .
@prefix owl:   <http://www.w3.org/2002/07/owl#> .
@prefix part:  <http://sweetontology.net/matrParticle/> .
@prefix pstate: <http://sweetontology.net/statePhysical/> .
@prefix xsd:   <http://www.w3.org/2001/XMLSchema#> .
@prefix rdfs:  <http://www.w3.org/2000/01/rdf-schema#> .
@prefix units: <http://sweetontology.net/reprSciUnits/> .
@prefix seas:  <http://sweetontology.net/reprTimeSeason/> .
@prefix func:  <http://sweetontology.net/propFunction/> .
@prefix rdf:   <http://www.w3.org/1999/02/22-rdf-syntax-ns#> .
@prefix thermo: <http://sweetontology.net/propTemperature/> .
@prefix ener:  <http://sweetontology.net/propEnergy/> .
@prefix oper:  <http://sweetontology.net/reprMathOperation/> .
@prefix rela:  <http://sweetontology.net/rela/> .
@prefix screla: <http://sweetontology.net/relaSci/> .
@prefix wind:  <http://sweetontology.net/phenAtmoWind/> .

thermo:TemperatureRange
        a                owl:Class ;
        rdfs:subClassOf  quan:IntervalQuantity ;
        rdfs:subClassOf  [ a                  owl:Restriction ;
                           owl:allValuesFrom  thermo:Temperature ;
                           owl:onProperty     screla:rangeOf
                         ] .

thermo:MeanMonthlyTemperature
        a                owl:Class ;
        rdfs:subClassOf  thermo:Temperature , func:MonthlyAverage .

thermo:PseudoEquivalentTemperature
        a                owl:Class ;
        rdfs:subClassOf  thermo:Temperature ;
        rdfs:subClassOf  [ a                  owl:Restriction ;
                           owl:allValuesFrom  thermo:EquivalentTemperature ;
                           owl:onProperty     mrela:approximates
                         ] .

thermo:AntennaTemperature
        a                owl:Class ;
        rdfs:comment     "Antenna temperature is a way of expressing the brightness of a radiation source - it is proportional to the power per unit area emitted by the source. In most cases where it is used it corresponds to the thermodynamic or physical temperature of the source being observed. It thus relates the power emitted by the source to an interesting physical property of that source."@en ;
        rdfs:subClassOf  thermo:Temperature .

thermo:DewPoint  a           owl:Class ;
        rdfs:comment         "The temperature to which a given air parcel must be cooled at constant pressure and constant water vapor content in order for saturation to occur."@en ;
        rdfs:subClassOf      thermo:Temperature ;
        owl:equivalentClass  thermo:DewPointTemperature .

thermo:MeanAnnualTemperature
        a                owl:Class ;
        rdfs:subClassOf  thermo:Temperature , func:AnnualAverage .

thermo:VirtualPotentialTemperature
        a                owl:Class ;
        rdfs:subClassOf  thermo:PotentialTemperature .

thermo:StaticTemperature
        a                owl:Class ;
        rdfs:subClassOf  thermo:Temperature .

thermo:IonTemperature
        a                owl:Class ;
        rdfs:subClassOf  thermo:Temperature ;
        rdfs:subClassOf  [ a               owl:Restriction ;
                           owl:hasValue    pstate:IonizedState ;
                           owl:onProperty  rela:hasState
                         ] .

thermo:WindChillIndex
        a                    owl:Class ;
        rdfs:comment         "A means of quantifying the threat of rapid cooling during breezy or windy conditions that may result in hypothermia in cold conditions."@en ;
        rdfs:subClassOf      thermo:Temperature ;
        rdfs:subClassOf      [ a                  owl:Restriction ;
                               owl:allValuesFrom  wind:Wind ;
                               owl:onProperty     screla:measureOf
                             ] ;
        owl:equivalentClass  thermo:WindChill .

thermo:EffectiveTemperature
        a                owl:Class ;
        rdfs:comment     "The temperature at which motionless saturated air would induce, in a sedentary worker wearing ordinary indoor clothing, the same sensation of comfort as that induced by the actual conditions of temperature, humidity, and air movement. Effective temperature is used as a guide in air-conditioning practice, and, on the comfort chart (American Society of Heating and Air Conditioning Engineers), it appears as a family of curves that serves as one coordinate in defining comfort zones."@en ;
        rdfs:subClassOf  thermo:Temperature .

thermo:EquivalentTemperature
        a                owl:Class ;
        rdfs:subClassOf  thermo:Temperature .

thermo:MeltingPoint  a   owl:Class ;
        rdfs:subClassOf  thermo:Temperature .

thermo:DewPointTemperature
        a       owl:Class .

<>      a                owl:Ontology ;
        rdfs:label       "SWEET Ontology" ;
        owl:imports      <stateThermodynamic> , <reprTimeSeason> , <relaMath> , <reprSciUnits> , <matrParticle> , <relaSci> , <propQuantity> , <propFunction> , <phenAtmoWind> , <propEnergy> , <relaChemical> , <statePhysical> , <reprMathOperation> , <rela> ;
        owl:versionInfo  "3.1.0" .

thermo:BoilingPoint  a   owl:Class ;
        rdfs:subClassOf  thermo:Temperature .

thermo:DryBulbTemperature
        a                owl:Class ;
        rdfs:subClassOf  thermo:Temperature .

thermo:ElectronTemperature
        a                owl:Class ;
        rdfs:subClassOf  thermo:Temperature ;
        rdfs:subClassOf  [ a                  owl:Restriction ;
                           owl:allValuesFrom  part:Electron ;
                           owl:onProperty     crela:hasSubstance
                         ] .

thermo:ColdestMonthTemperature
        a                owl:Class ;
        rdfs:subClassOf  thermo:Temperature ;
        rdfs:subClassOf  [ a                   owl:Restriction ;
                           owl:onProperty      rela:hasPhenomena ;
                           owl:someValuesFrom  seas:ColdestMonth
                         ] .

thermo:TriplePoint  a    owl:Class ;
        rdfs:subClassOf  thermo:Temperature .

thermo:PotentialTemperature
        a                owl:Class ;
        rdfs:comment     "The temperature that a parcel would have if brought adiabatically and reversibly from its initial state to a standard reference pressure, typically 100 kPa."@en ;
        rdfs:subClassOf  thermo:Temperature ;
        rdfs:subClassOf  [ a               owl:Restriction ;
                           owl:hasValue    tstate:Adiabatic ;
                           owl:onProperty  rela:hasState
                         ] .

thermo:EquivalentPotentialTemperature
        a                owl:Class ;
        rdfs:subClassOf  thermo:PotentialTemperature .

thermo:WetBulbTemperature
        a                owl:Class ;
        rdfs:subClassOf  thermo:Temperature .

thermo:DewPointDepression
        a                owl:Class ;
        rdfs:subClassOf  oper:Subtraction , thermo:Temperature ;
        rdfs:subClassOf  [ a                  owl:Restriction ;
                           owl:allValuesFrom  thermo:DryBulbTemperature ;
                           owl:onProperty     mrela:hasFirstOperand
                         ] ;
        rdfs:subClassOf  [ a                  owl:Restriction ;
                           owl:allValuesFrom  thermo:DewPointTemperature ;
                           owl:onProperty     mrela:hasSecondOperand
                         ] .

thermo:WetBulbPotentialTemperature
        a                owl:Class ;
        rdfs:comment     "The temperature an air parcel would have if cooled from its initial state adiabatically to saturation, and thence brought to 1000 mb by a moist-adiabatic process."@en ;
        rdfs:subClassOf  thermo:PotentialTemperature .

thermo:BrightnessTemperature
        a                owl:Class ;
        rdfs:comment     "A descriptive measure of radiation in terms of the temperature of a hypothetical blackbody emitting an identical amount of radiation at the same wavelength."@en ;
        rdfs:subClassOf  thermo:Temperature .

thermo:GlobalWarmingPotential
        a                owl:Class ;
        rdfs:subClassOf  thermo:Temperature .

thermo:Temperature  a    owl:Class ;
        rdfs:subClassOf  quan:ThermodynamicQuantity ;
        rdfs:subClassOf  [ a                  owl:Restriction ;
                           owl:allValuesFrom  ener:Heat ;
                           owl:onProperty     screla:measureOf
                         ] ;
        rdfs:subClassOf  [ a               owl:Restriction ;
                           owl:hasValue    units:kelvin ;
                           owl:onProperty  screla:hasDefaultUnit
                         ] .

thermo:WarmestMonthTemperature
        a                owl:Class ;
        rdfs:subClassOf  thermo:Temperature ;
        rdfs:subClassOf  [ a                   owl:Restriction ;
                           owl:onProperty      rela:hasPhenomena ;
                           owl:someValuesFrom  seas:WarmestMonth
                         ] .

thermo:VirtualTemperature
        a                owl:Class ;
        rdfs:subClassOf  thermo:Temperature .

thermo:PseudoEquivalentPotentialTemperature
        a                owl:Class ;
        rdfs:subClassOf  thermo:Temperature ;
        rdfs:subClassOf  [ a                  owl:Restriction ;
                           owl:allValuesFrom  thermo:EquivalentPotentialTemperature ;
                           owl:onProperty     mrela:approximates
                         ] .

thermo:KineticTemperature
        a                owl:Class ;
        rdfs:subClassOf  thermo:Temperature .

thermo:WindChill  a  owl:Class .

thermo:NeutralTemperature
        a                owl:Class ;
        rdfs:subClassOf  thermo:Temperature ;
        rdfs:subClassOf  [ a               owl:Restriction ;
                           owl:hasValue    pstate:NeutralState ;
                           owl:onProperty  rela:hasState
                         ] .

thermo:TotalTemperature
        a                owl:Class ;
        rdfs:subClassOf  thermo:Temperature .
