@base          <http://sweetontology.net/propSpeed> .
@prefix quan:  <http://sweetontology.net/propQuantity/> .
@prefix owl:   <http://www.w3.org/2002/07/owl#> .
@prefix dyna:  <http://sweetontology.net/propSpeed/> .
@prefix xsd:   <http://www.w3.org/2001/XMLSchema#> .
@prefix rdfs:  <http://www.w3.org/2000/01/rdf-schema#> .
@prefix units: <http://sweetontology.net/reprSciUnits/> .
@prefix sdir:  <http://sweetontology.net/reprSpaceDirection/> .
@prefix srela: <http://sweetontology.net/relaSpace/> .
@prefix rdf:   <http://www.w3.org/1999/02/22-rdf-syntax-ns#> .
@prefix prop:  <http://sweetontology.net/prop/> .
@prefix math:  <http://sweetontology.net/reprMath/> .
@prefix screla: <http://sweetontology.net/relaSci/> .
@prefix rela:  <http://sweetontology.net/rela/> .
@prefix wind:  <http://sweetontology.net/phenAtmoWind/> .

dyna:IonVelocity  a      owl:Class ;
        rdfs:subClassOf  dyna:Velocity .

dyna:Inertia  a          owl:Class ;
        rdfs:subClassOf  dyna:Momentum .

dyna:MagnetiCurvatureDrift
        a                owl:Class ;
        rdfs:subClassOf  dyna:Drift , quan:ElectromagneticQuantity .

dyna:TerminalVelocity
        a                owl:Class ;
        rdfs:subClassOf  dyna:Velocity .

dyna:GroundSpeed  a      owl:Class ;
        rdfs:comment     "Ground speed is the speed of an aircraft relative to the ground. It is the sum of the aircraft's true airspeed and the current wind and weather conditions; a headwind subtracts from the ground speed, while a tailwind adds to it. Winds at other angles to the heading will have components of either headwind or tailwind as well as a crosswind component." ;
        rdfs:subClassOf  dyna:Speed .

dyna:AlfvenVelocity  a   owl:Class ;
        rdfs:subClassOf  dyna:Velocity .

dyna:ThermalVelocity  a  owl:Class ;
        rdfs:subClassOf  dyna:Velocity .

dyna:NeutralVelocity  a  owl:Class ;
        rdfs:subClassOf  dyna:Velocity .

dyna:Omega  a            owl:Class ;
        rdfs:subClassOf  dyna:VerticalVelocity .

dyna:ProperMotion  a     owl:Class ;
        rdfs:subClassOf  dyna:Speed .

dyna:EscapeVelocity  a   owl:Class ;
        rdfs:subClassOf  dyna:Velocity .

dyna:Velocity  a         owl:Class ;
        rdfs:comment     "The time rate of change of a position vector; that is, a change of position expressed in terms of speed and direction."@en ;
        rdfs:subClassOf  math:Vector , quan:PhysicalQuantity , prop:MotionProperty ;
        rdfs:subClassOf  [ a               owl:Restriction ;
                           owl:hasValue    units:meterPerSecond ;
                           owl:onProperty  screla:hasDefaultUnit
                         ] .

dyna:Momentum  a         owl:Class ;
        rdfs:subClassOf  quan:PhysicalQuantity , prop:MotionProperty ;
        rdfs:subClassOf  [ a               owl:Restriction ;
                           owl:hasValue    units:kilogramMeterPerSecond ;
                           owl:onProperty  screla:hasDefaultUnit
                         ] .

dyna:Speed  a            owl:Class ;
        rdfs:subClassOf  quan:PhysicalQuantity , prop:MotionProperty ;
        rdfs:subClassOf  [ a               owl:Restriction ;
                           owl:hasValue    units:meterPerSecond ;
                           owl:onProperty  screla:hasDefaultUnit
                         ] .

dyna:RadialVelocity  a   owl:Class ;
        rdfs:comment     "The component of a three-dimensional velocity vector oriented along the radial direction from the origin point or axis in polar, cylindrical, or spherical coordinates.  In connection with Doppler radar, the radial velocity component is called Doppler velocity."@en ;
        rdfs:subClassOf  dyna:Velocity .

<>      a                owl:Ontology ;
        rdfs:label       "SWEET Ontology" ;
        owl:imports      <phenAtmoWind> , <relaSpace> , <prop> , <reprSpaceDirection> , <propQuantity> , <relaSci> , <rela> , <reprSciUnits> , <reprMath> ;
        owl:versionInfo  "3.1.0" .

dyna:DopplerVelocity  a  owl:Class ;
        rdfs:subClassOf  dyna:Velocity .

dyna:Airspeed  a         owl:Class ;
        rdfs:comment     "Airspeed is the speed of an aircraft relative to the air. There are several different measures of airspeed: indicated airspeed, calibrated airspeed, equivalent airspeed and true airspeed." ;
        rdfs:subClassOf  dyna:Speed .

dyna:SeepageVelocity  a  owl:Class ;
        rdfs:subClassOf  dyna:Velocity , prop:HydrogeologicalProperty .

dyna:Drift  a            owl:Class ;
        rdfs:subClassOf  dyna:Velocity .

dyna:PhaseVelocity  a    owl:Class ;
        rdfs:subClassOf  dyna:Velocity , prop:WaveProperty .

dyna:WindShear  a        owl:Class ;
        rdfs:subClassOf  prop:FluidProperty .

dyna:TangentialAcceleration
        a                owl:Class ;
        rdfs:comment     "The component of the acceleration directed along the velocity vector (streamline), with magnitude equal to the rate of change of speed of the parcel dV/dt, where V is the speed."@en ;
        rdfs:subClassOf  dyna:Acceleration .

dyna:WindSpeed  a        owl:Class ;
        rdfs:subClassOf  dyna:Speed ;
        rdfs:subClassOf  [ a                  owl:Restriction ;
                           owl:allValuesFrom  wind:Wind ;
                           owl:onProperty     rela:hasPhenomena
                         ] .

dyna:GroupVelocity  a    owl:Class ;
        rdfs:subClassOf  dyna:Velocity , prop:WaveProperty .

dyna:Acceleration  a     owl:Class ;
        rdfs:comment     "The rate of change with time of the velocity vector of a particle." ;
        rdfs:label       "Acceleration" ;
        rdfs:subClassOf  quan:PhysicalQuantity , prop:MotionProperty ;
        rdfs:subClassOf  [ a               owl:Restriction ;
                           owl:hasValue    units:meterPerSecondSquared ;
                           owl:onProperty  screla:hasDefaultUnit
                         ] .

dyna:VerticalVelocity
        a                owl:Class ;
        rdfs:subClassOf  dyna:Velocity ;
        rdfs:subClassOf  [ a               owl:Restriction ;
                           owl:hasValue    sdir:Vertical ;
                           owl:onProperty  srela:hasDirection
                         ] .
