@base          <http://sweetontology.net/realmLandAeolian> .
@prefix crela: <http://sweetontology.net/relaChemical/> .
@prefix chem:  <http://sweetontology.net/matr/> .
@prefix owl:   <http://www.w3.org/2002/07/owl#> .
@prefix xsd:   <http://www.w3.org/2001/XMLSchema#> .
@prefix rdfs:  <http://www.w3.org/2000/01/rdf-schema#> .
@prefix aeol:  <http://sweetontology.net/realmLandAeolian/> .
@prefix ht:    <http://sweetontology.net/propSpaceHeight/> .
@prefix srela: <http://sweetontology.net/relaSpace/> .
@prefix sed:   <http://sweetontology.net/matrSediment/> .
@prefix phen:  <http://sweetontology.net/phen/> .
@prefix rdf:   <http://www.w3.org/1999/02/22-rdf-syntax-ns#> .
@prefix geomor: <http://sweetontology.net/phenGeolGeomorphology/> .
@prefix land:  <http://sweetontology.net/realmLandform/> .
@prefix rela:  <http://sweetontology.net/rela/> .

aeol:Seif  a             owl:Class ;
        rdfs:subClassOf  aeol:Dune .

aeol:Aeolian  a              owl:Class ;
        rdfs:comment         "Aeolian (or Eolian or Ã†olian) processes pertain to the activity of the winds and more specifically, to the winds' ability to shape the surface of the Earth and other planets. Winds may erode, transport, and deposit materials, and are effective agents in regions with sparse vegetation and a large supply of unconsolidated sediments. [Wikipedia]"@en ;
        rdfs:subClassOf      geomor:Weathering ;
        owl:equivalentClass  aeol:Eolian .

aeol:Yardang  a          owl:Class ;
        rdfs:subClassOf  aeol:AeolianLandform .

aeol:Dune  a                 owl:Class ;
        rdfs:comment         "A dune is a hill of sand built by eolian processes. Dunes are subject to different forms and sizes based on their interaction with the wind. Most kinds of dune are longer on the windward side where the sand is pushed up the dune, and a shorter slip face in the lee of the wind. The valley or trough between dunes is called a slack. A dune field is an area covered by extensive sand dunes. Large dune fields are known as ergs"@en ;
        rdfs:subClassOf      aeol:AeolianLandform ;
        rdfs:subClassOf      [ a                  owl:Restriction ;
                               owl:allValuesFrom  sed:Sand ;
                               owl:onProperty     crela:hasSubstance
                             ] ;
        owl:equivalentClass  aeol:SandDune .

aeol:Erg  a              owl:Class ;
        rdfs:subClassOf  aeol:AeolianLandform .

aeol:SandDune  a  owl:Class .

aeol:Barchan  a          owl:Class ;
        rdfs:subClassOf  aeol:Dune .

<>      a                owl:Ontology ;
        rdfs:label       "SWEET Ontology" ;
        owl:imports      <relaSpace> , <realmLandform> , <phenGeolGeomorphology> , <matrSediment> , <rela> , <relaChemical> , <phen> , <propSpaceHeight> , <matr> ;
        owl:versionInfo  "3.1.0" .

aeol:AeolianLandform  a  owl:Class ;
        rdfs:subClassOf  land:Landform ;
        rdfs:subClassOf  [ a                  owl:Restriction ;
                           owl:allValuesFrom  aeol:Eolian ;
                           owl:onProperty     rela:hasPhenomena
                         ] .

aeol:HighDesert  a       owl:Class ;
        rdfs:subClassOf  aeol:Desert ;
        rdfs:subClassOf  [ a                  owl:Restriction ;
                           owl:allValuesFrom  ht:Elevation ;
                           owl:onProperty     srela:hasSpatialExtent
                         ] .

aeol:SlipFace  a         owl:Class ;
        rdfs:subClassOf  aeol:AeolianLandform .

aeol:Slack  a            owl:Class ;
        rdfs:subClassOf  aeol:AeolianLandform .

aeol:Eolian  a  owl:Class .

aeol:Desert  a           owl:Class ;
        rdfs:comment     "A desert is a landscape form or region that receives very little precipitation."@en ;
        rdfs:subClassOf  aeol:AeolianLandform .
