@base          <http://sweetontology.net/realmLandVolcanic> .
@prefix crela: <http://sweetontology.net/relaChemical/> .
@prefix owl:   <http://www.w3.org/2002/07/owl#> .
@prefix planet: <http://sweetontology.net/realm/> .
@prefix volc:  <http://sweetontology.net/realmLandVolcanic/> .
@prefix xsd:   <http://www.w3.org/2001/XMLSchema#> .
@prefix rdfs:  <http://www.w3.org/2000/01/rdf-schema#> .
@prefix geol:  <http://sweetontology.net/realmGeol/> .
@prefix ign:   <http://sweetontology.net/matrRockIgneous/> .
@prefix fail:  <http://sweetontology.net/phenSolid/> .
@prefix vol:   <http://sweetontology.net/phenGeolVolcano/> .
@prefix rdf:   <http://www.w3.org/1999/02/22-rdf-syntax-ns#> .
@prefix land:  <http://sweetontology.net/realmLandform/> .
@prefix ener:  <http://sweetontology.net/propEnergy/> .
@prefix rela:  <http://sweetontology.net/rela/> .

<>      a                owl:Ontology ;
        rdfs:label       "SWEET Ontology" ;
        owl:imports      <realmGeol> , <relaChemical> , <realmLandform> , <propEnergy> , <matrRockIgneous> , <realm> , <phenSolid> , <phenGeolVolcano> , <rela> ;
        owl:versionInfo  "3.1.0" .

volc:LinearVolcanicChain
        a                owl:Class ;
        rdfs:comment     "Where this association of flood basalts with continental rifting is observed, it is not uncommon to find linear chains of volcanic islands  [Wikipedia]"@en ;
        rdfs:subClassOf  volc:VolcanicChain .

volc:VolcanicSystem  a   owl:Class ;
        rdfs:subClassOf  geol:GeologicFeature .

volc:Monogenetic  a      owl:Class ;
        rdfs:comment     "A volcano built by a single eruption."@en ;
        rdfs:subClassOf  volc:Volcano .

volc:SubmarineVolcano
        a       owl:Class .

volc:Fumarole  a         owl:Class ;
        rdfs:subClassOf  volc:Vent .

volc:Vent  a             owl:Class ;
        rdfs:subClassOf  fail:Crack , geol:GeologicFeature .

volc:Geyser  a           owl:Class ;
        rdfs:subClassOf  volc:Vent .

volc:Stratovolcano  a    owl:Class ;
        rdfs:comment     "A volcano composed of both lava flows and pyroclastic material."@en ;
        rdfs:subClassOf  volc:Volcano .

volc:VolcanicChain  a        owl:Class ;
        rdfs:comment         "Island arcs that develop along the edges of a continent (for example, large parts of the Andes/ Central American/ Canadian mountain chain) may be known as a volcanic arc or volcanic chain. [Wikipedia]"@en ;
        rdfs:subClassOf      geol:GeologicProvince ;
        owl:equivalentClass  volc:VolcanicArc .

volc:Geothermal  a       owl:Class ;
        rdfs:comment     "In geology, geothermal refers to heat sources within the planet. Strictly speaking, geo-thermal necessarily refers to the Earth but the concept may be applied to other planets. Geothermal is technically an adjective (e.g., geothermal energy) but in U.S. English the word has attained frequent use as a noun (otherwise expressed as g. heat, g. source, or geotherm). The planet's internal heat was originally generated during its accretion, due to gravitational binding energy, and since then additional heat has continued to be generated by the radioactive decay of elements such as uranium, thorium, and potassium. The heat flow from the interior to the surface is only 1/20,000 as great as the energy received from the Sun."@en ;
        rdfs:subClassOf  geol:GeologicFeature , ener:Heat .

volc:LavaPlain  a        owl:Class ;
        rdfs:subClassOf  geol:GeologicFeature .

volc:Volcano  a          owl:Class ;
        rdfs:comment     "A volcano is an opening, or rupture, in a planet's surface or crust, which allows hot, molten rock, ash, and gases to escape from below the surface. Volcanic activity involving the extrusion of rock tends to form mountains or features like mountains over a period of time. [Wikipedia]"@en ;
        rdfs:subClassOf  volc:VolcanicField ;
        rdfs:subClassOf  [ a                   owl:Restriction ;
                           owl:onProperty      crela:hasPrimarySubstance ;
                           owl:someValuesFrom  ign:Magma
                         ] .

volc:CompoundVolcano  a      owl:Class ;
        rdfs:comment         "A volcano that consists of a complex of two or more vents, or a volcano that has an associated volcanic dome, either in its crater or on its flanks."@en ;
        rdfs:subClassOf      volc:Volcano ;
        owl:equivalentClass  volc:CompositeVolcano .

volc:Tumulus  a          owl:Class ;
        rdfs:comment     "A doming or small mound on the crest of a lava flow caused by pressure due to the difference in the rate of flow between the cooler crust and the more fluid lava below."@en ;
        rdfs:subClassOf  land:Landform .

volc:CentralVolcano  a   owl:Class ;
        rdfs:comment     "A volcano constructed by the ejection of debris and lava flows from a central point, forming a more or less symmetrical volcano."@en ;
        rdfs:subClassOf  volc:Volcano .

volc:Caldera  a          owl:Class ;
        rdfs:subClassOf  geol:GeologicFeature .

volc:SubaqueousVolcano
        a                    owl:Class ;
        rdfs:subClassOf      volc:Volcano ;
        rdfs:subClassOf      [ a                  owl:Restriction ;
                               owl:allValuesFrom  planet:Ocean ;
                               owl:onProperty     rela:hasRealm
                             ] ;
        owl:equivalentClass  volc:SubmarineVolcano .

volc:CompositeVolcano
        a       owl:Class .

volc:ShieldVolcano  a    owl:Class ;
        rdfs:subClassOf  volc:Volcano .

volc:VolcanicField  a    owl:Class ;
        rdfs:comment     "A volcanic field is a spot of the earth's crust that is prone to localized volcanic activity. They usually contain 10 to 100 volcanoes, such as cinder cones and are usually in clusters. Lava flows may also occur. They may occur as a monogenetic volcanic field or a polygenetic volcanic field. [Wikipedia]"@en ;
        rdfs:subClassOf  geol:GeologicProvince .

volc:HotSpot  a          owl:Class ;
        rdfs:comment     "In geology, a hotspot is a location on the Earth's surface that has experienced active volcanism for a long period of time. [Wikipedia]"@en ;
        rdfs:subClassOf  geol:GeologicFeature ;
        rdfs:subClassOf  [ a                  owl:Restriction ;
                           owl:allValuesFrom  ign:AnorogenicIgneousRock ;
                           owl:onProperty     crela:hasSubstance
                         ] ;
        rdfs:subClassOf  [ a                  owl:Restriction ;
                           owl:allValuesFrom  volc:LinearVolcanicChain ;
                           owl:onProperty     rela:hasRealm
                         ] .

volc:VolcanicArc  a  owl:Class .
