@base          <http://sweetontology.net/realmHydroBody> .
@prefix crela: <http://sweetontology.net/relaChemical/> .
@prefix chem:  <http://sweetontology.net/matr/> .
@prefix owl:   <http://www.w3.org/2002/07/owl#> .
@prefix planet: <http://sweetontology.net/realm/> .
@prefix body2: <http://sweetontology.net/realmHydroBody/> .
@prefix xsd:   <http://www.w3.org/2001/XMLSchema#> .
@prefix rdfs:  <http://www.w3.org/2000/01/rdf-schema#> .
@prefix cryo:  <http://sweetontology.net/realmCryo/> .
@prefix body:  <http://sweetontology.net/realmHydroBody/> .
@prefix water: <http://sweetontology.net/matrWater/> .
@prefix hydr:  <http://sweetontology.net/realmHydro/> .
@prefix sed:   <http://sweetontology.net/matrSediment/> .
@prefix cstate: <http://sweetontology.net/stateChemical/> .
@prefix rdf:   <http://www.w3.org/1999/02/22-rdf-syntax-ns#> .
@prefix fluv:  <http://sweetontology.net/realmLandFluvial/> .
@prefix plant: <http://sweetontology.net/matrPlant/> .
@prefix state: <http://sweetontology.net/state/> .
@prefix screla: <http://sweetontology.net/relaSci/> .
@prefix rela:  <http://sweetontology.net/rela/> .

body:Wetland  a          owl:Class ;
        rdfs:comment     "In physical geography, a wetland is an environment at the interface between truly terrestrial ecosystems and aquatic systems making them inherently different from each other yet highly dependent on both. In essence, wetlands are ecotones. Wetlands often host considerable biodiversity and endemism. The US Army Corps of Engineers and the US Environmental Protection Agency jointly define wetlands as: Those areas that are inundated or saturated by surface or ground water at a frequency and duration sufficient to support, and that under normal circumstances do support, a prevalence of vegetation typically adapted for life in saturated soil conditions. Wetlands generally include swamps, marshes, bogs, and similar areas."@en ;
        rdfs:subClassOf  body:BodyOfWater .

body:Bog  a              owl:Class ;
        rdfs:subClassOf  body:Wetland .

body:Pond  a             owl:Class ;
        rdfs:subClassOf  body:Channel , body:BodyOfWater .

body:ValleyBog  a        owl:Class ;
        rdfs:subClassOf  body:Bog .

body:Estuary  a          owl:Class ;
        rdfs:comment     "An estuary is a semi-enclosed coastal body of water with one or more rivers or streams flowing into it, and with a free connection to the open sea. Estuaries are often associated with high rates of biological productivity. An estuary is where the river meets the sea. An estuary is typically the tidal mouth of a river, and estuaries are often characterized by sedimentation or silt carried in from terrestrial runoff and, frequently, from offshore. They are made up of brackish water. Estuaries are more likely to occur on submerged coasts, where the sea level has risen in relation to the land; this process floods valleys to form rias and fjords. These can become estuaries if there is a stream or river flowing into them."@en ;
        rdfs:subClassOf  body:BodyOfWater ;
        rdfs:subClassOf  [ a                  owl:Restriction ;
                           owl:allValuesFrom  sed:Sediment ;
                           owl:onProperty     crela:hasSubstance
                         ] ;
        rdfs:subClassOf  [ a                   owl:Restriction ;
                           owl:onProperty      crela:hasSubstance ;
                           owl:someValuesFrom  water:BrackishWater
                         ] .

body:Aqueduct  a         owl:Class ;
        rdfs:subClassOf  body:Channel .

body:Swamp  a            owl:Class ;
        rdfs:comment     "A swamp is a wetland that features temporary or permanent inundation of large areas of land by shallow bodies of water, generally with a substantial number of hammocks, or dry-land protrusions, and covered by aquatic vegetation, or vegetation that tolerates periodical inundation.The water of a swamp may be fresh water or salt water. A swamp is also generally defined as having no substantial peat deposits."@en ;
        rdfs:subClassOf  body:Wetland ;
        rdfs:subClassOf  [ a               owl:Restriction ;
                           owl:hasValue    cstate:Saturation ;
                           owl:onProperty  rela:hasState
                         ] ;
        rdfs:subClassOf  [ a                  owl:Restriction ;
                           owl:allValuesFrom  plant:Vegetation ;
                           owl:onProperty     screla:hasSpecies
                         ] .

body:Marsh  a            owl:Class ;
        rdfs:comment     "In geography, a marsh, or morass, is a type of wetland which is subject to frequent or continuous inundation. Typically a marsh features grasses, rushes, reeds, typhas, sedges, and other herbaceous plants (possibly with low-growing woody plants) in a context of shallow water. A marsh is different from a swamp, which has a greater proportion of open water surface, and is generally deeper than a marsh. In North America, the term swamp is used for wetland dominated by trees rather than grasses and low herbs"@en ;
        rdfs:subClassOf  body:Wetland .

body:FreshwaterLake  a   owl:Class ;
        rdfs:subClassOf  body:Lake ;
        rdfs:subClassOf  [ a                  owl:Restriction ;
                           owl:allValuesFrom  water:FreshWater ;
                           owl:onProperty     crela:hasSubstance
                         ] .

body:Lake  a             owl:Class ;
        rdfs:subClassOf  body:BodyOfWater .

<>      a                owl:Ontology ;
        rdfs:label       "SWEET Ontology" ;
        owl:imports      <stateChemical> , <matrSediment> , <realm> , <realmCryo> , <state> , <matrWater> , <realmLandFluvial> , <relaSci> , <realmHydro> , <rela> , <matr> , <relaChemical> , <matrPlant> ;
        owl:versionInfo  "3.1.0" .

body:Bay  a              owl:Class ;
        rdfs:subClassOf  body:BodyOfWater .

body:BarrierLagoon  a    owl:Class ;
        rdfs:subClassOf  body:Lagoon .

body:Dam  a              owl:Class ;
        rdfs:subClassOf  body:BodyOfWater .

body:CarbonateCompensationLevel
        a                    owl:Class ;
        owl:equivalentClass  body:WaterBodyBoundary .

body:Lagoon  a           owl:Class ;
        rdfs:comment     "A lagoon is a body of comparatively shallow salt or brackish water separated from the deeper sea by a shallow or exposed sandbank, coral reef, or similar feature. Thus, the enclosed body of water behind a barrier reef or barrier islands or enclosed by an atoll reef is called a lagoon. Lagoon refers to both coastal lagoons formed by the build-up of sandbanks or reefs along shallow coastal waters, and the lagoons in atolls, formed by the growth of coral reefs on slowly sinking central islands. Lagoons that are fed by freshwater streams are also called estuaries"@en ;
        rdfs:subClassOf  body:BodyOfWater .

body:Mouth  a            owl:Class ;
        rdfs:subClassOf  body:BodyOfWater .

body:BodyOfWater  a      owl:Class ;
        rdfs:subClassOf  hydr:HydrosphereFeature .

body:Inlet  a            owl:Class ;
        rdfs:comment     "An inlet is a narrow body between islands or leading inland from a larger body of water, often leading to an enclosed body of water, such as a sound, bay, lagoon or marsh. In sea coasts an inlet usually refers to the actual connection between a bay and the ocean and is often called an entrance."@en ;
        rdfs:subClassOf  body:Estuary .

body:FramStrait  a  body:Strait .

body:CheckDam  a         owl:Class ;
        rdfs:subClassOf  body:Dam .

body:BlanketBog  a       owl:Class ;
        rdfs:subClassOf  body:Bog .

body:Spring  a           owl:Class ;
        rdfs:comment     "A spring is a point where groundwater flows out of the ground, and is thus where the aquifer surface meets the ground surface. Dependent upon the constancy of the water source (rainfall or snowmelt that infiltrates the earth), a spring may be ephemeral (intermittent) or perennial (continuous)."@en ;
        rdfs:subClassOf  body:BodyOfWater .

body:SeaSurface  a       owl:Class ;
        rdfs:subClassOf  planet:PlanetarySurface , body:WaterBodyBoundary .

body:Stream  a           owl:Class ;
        rdfs:comment     "A stream is a body of water with a current, confined within a bed and banks. Streams are important as conduits in the water cycle, instruments in aquifer recharge, and corridors for fish and wildlife migration. The biological habitat in the immediate vicinity of a stream is called a riparian zone. Given the status of the ongoing Holocene extinction event, streams play an important corridor role in connecting fragmented habitats and thus in conserving biodiversity. Stream is also an umbrella term used in the scientific community for all flowing natural waters, regardless of size. The study of streams and waterways in general is known as surface hydrology and is a core element of environmental geography"@en ;
        rdfs:subClassOf  body:BodyOfWater .

body:Fjord  a                owl:Class ;
        rdfs:comment         "A fjord (or fiord) is a long, narrow estuary with steep sides, made when a glacial valley is filled by rising sea water levels. The seeds of a fjord are laid when a glacier cuts a U-shaped valley through abrasion of the surrounding bedrock by the sediment it carries. Many such valleys were formed during recent ice age when the sea was at a much lower level than it is today. At the end of the ice age, the climate warmed up again and glaciers retreated. Sea level rose due to an influx of water from melting ice sheets and glaciers around the world (it rose over 100 m after the last ice age), inundating the vacated valleys with seawater to form fjords."@en ;
        rdfs:subClassOf      body:Estuary ;
        rdfs:subClassOf      [ a                  owl:Restriction ;
                               owl:allValuesFrom  fluv:Valley ;
                               owl:onProperty     rela:hasRealm
                             ] ;
        rdfs:subClassOf      [ a                  owl:Restriction ;
                               owl:allValuesFrom  cryo:Glacier ;
                               owl:onProperty     rela:hasRealm
                             ] ;
        owl:equivalentClass  body:Fiord .

body:WaterBodyBoundary
        a                owl:Class ;
        rdfs:subClassOf  planet:PlanetaryBoundary ;
        rdfs:subClassOf  [ a                  owl:Restriction ;
                           owl:allValuesFrom  planet:Ocean ;
                           owl:onProperty     rela:hasRealm
                         ] .

body:Arroyo  a           owl:Class ;
        rdfs:subClassOf  body:BodyOfWater .

body:Sound  a            owl:Class ;
        rdfs:subClassOf  body:BodyOfWater .

body:Canal  a            owl:Class ;
        rdfs:subClassOf  body:BodyOfWater .

body:Basin  a            owl:Class ;
        rdfs:subClassOf  body:BodyOfWater .

body:Fiord  a   owl:Class .

body:Creek  a            owl:Class ;
        rdfs:subClassOf  body:Stream .

body:Peatland  a         owl:Class ;
        rdfs:comment     "Peat forms in wetlands or peatlands, variously called bogs, moors, muskegs, pocosins, mires, and peat swamp forests"@en ;
        rdfs:subClassOf  body:Wetland ;
        rdfs:subClassOf  [ a                  owl:Restriction ;
                           owl:allValuesFrom  sed:Peat ;
                           owl:onProperty     crela:hasSubstance
                         ] .

body:Reservoir  a        owl:Class ;
        rdfs:subClassOf  body:BodyOfWater .

body:River  a            owl:Class ;
        rdfs:comment     "A river is a natural waterway that transits water through a landscape from higher to lower elevations called divides. The divide determines which way a river will flow. It is an integral component of the water cycle. The water within a river is generally collected from precipitation through surface runoff, groundwater recharge (as seen at baseflow conditions / during periods of lack of precipitation) and release of stored water in natural reservoirs, such as a glacier"@en ;
        rdfs:subClassOf  body:BodyOfWater .

body:Bolson  a           owl:Class ;
        rdfs:subClassOf  body:Basin .

body:RaisedBog  a        owl:Class ;
        rdfs:subClassOf  body:Bog .

body:Strait  a           owl:Class ;
        rdfs:subClassOf  body:Channel .

body:Channel  a          owl:Class ;
        rdfs:comment     "In physical geography, a channel is the physical confine of a river, slough or ocean strait consisting of a bed and banks. A channel is also the natural or man-made deeper course through a reef, bar, bay, or any shallow body of water. It is especially used as a Nautical term to mean the dredged and marked lane of safe travel which a cognizant governmental entity guarantees to have a minimum depth across its specified minimum width to all vessels transiting a body of water. The term not only includes the deep-dredged ship-navigable parts of an estuary or river leading to port facilities, but also to lesser channels accessing boat port-facilities such as marinas. When dredged channels traverse bay mud or sandy bottoms, repeated dredging is often necessary because of the unstable subsequent movement of benthic soils."@en ;
        rdfs:subClassOf  body:BodyOfWater .
