@base          <http://sweetontology.net/realmOcean> .
@prefix mrela: <http://sweetontology.net/relaMath/> .
@prefix bproc: <http://sweetontology.net/phenBiol/> .
@prefix owl:   <http://www.w3.org/2002/07/owl#> .
@prefix xsd:   <http://www.w3.org/2001/XMLSchema#> .
@prefix rdfs:  <http://www.w3.org/2000/01/rdf-schema#> .
@prefix cryo:  <http://sweetontology.net/realmCryo/> .
@prefix med:   <http://sweetontology.net/propIndex/> .
@prefix conc:  <http://sweetontology.net/propChemical/> .
@prefix srela: <http://sweetontology.net/relaSpace/> .
@prefix ocean: <http://sweetontology.net/realmOcean/> .
@prefix rdf:   <http://www.w3.org/1999/02/22-rdf-syntax-ns#> .
@prefix thermo: <http://sweetontology.net/propTemperatureGradient/> .
@prefix realm: <http://sweetontology.net/realm/> .
@prefix oper:  <http://sweetontology.net/reprMathOperation/> .
@prefix xten:  <http://sweetontology.net/propSpaceDistance/> .
@prefix screla: <http://sweetontology.net/relaSci/> .
@prefix rela:  <http://sweetontology.net/rela/> .

ocean:AphoticZone  a     owl:Class ;
        rdfs:comment     "The aphotic zone is the portion of a lake or ocean where there is little or no sunlight. It is formally defined as the depths beyond which less than 1% of sunlight penetrates. Consequently, bioluminescence is essentially the only light found in this zone. Most food comes from dead organisms sinking to the bottom of the lake or ocean from other zones. The depth of the aphotic zone can be greatly affected by such things as turbidity and the season of the year. The aphotic zone underlies the photic zone, which is that portion of the ocean directly affected by sunlight."@en ;
        rdfs:subClassOf  ocean:WaterBodyLayer ;
        rdfs:subClassOf  [ a                  owl:Restriction ;
                           owl:allValuesFrom  med:Turbidity ;
                           owl:onProperty     screla:hasQuantity
                         ] ;
        rdfs:subClassOf  [ a                  owl:Restriction ;
                           owl:allValuesFrom  ocean:PhoticZone ;
                           owl:onProperty     srela:below
                         ] .

ocean:EuphoticZone  a        owl:Class ;
        owl:equivalentClass  ocean:PhoticZone .

ocean:MixedLayer  a      owl:Class ;
        rdfs:subClassOf  ocean:WaterBodyLayer .

ocean:Polynya  a         owl:Class ;
        rdfs:comment     "A polynya is any non-linear area of open water surrounded by sea ice. It is now used as geographical term for areas of sea in Arctic or Antarctic regions which remain unfrozen for much of the year." ;
        rdfs:subClassOf  ocean:OceanRegion ;
        rdfs:subClassOf  [ a                  owl:Restriction ;
                           owl:allValuesFrom  cryo:SeaIce ;
                           owl:onProperty     srela:surroundedBy
                         ] .

ocean:ProfundalZone  a   owl:Class ;
        rdfs:comment     "The profundal zone is a deep zone of a body of water, such as an ocean or a lake, located below the range of effective light penetration. This is typically below the thermocline, the vertical zone in the water through which temperature drops rapidly. The lack of light in the profundal zone determines the type of biological community that can live in this region, which is distinctly different from the community in the overlying waters. The profundal zone is part of the aphotic zone."@en ;
        rdfs:subClassOf  ocean:WaterBodyLayer ;
        rdfs:subClassOf  [ a                  owl:Restriction ;
                           owl:allValuesFrom  ocean:AphoticZone ;
                           owl:onProperty     rela:hasRealm
                         ] .

ocean:PelagicSubZone  a  owl:Class ;
        rdfs:subClassOf  ocean:OceanRegion ;
        rdfs:subClassOf  [ a                  owl:Restriction ;
                           owl:allValuesFrom  ocean:PelagicZone ;
                           owl:onProperty     rela:partOf
                         ] .

ocean:Pycnocline  a      owl:Class ;
        rdfs:comment     "A pycnocline is a layer across which there is a rapid change in water density with depth. In freshwater environments such as lakes this density change is primarily caused by water temperature, while in seawater environments such as oceans the density change may be caused by changes in water temperature and/or salinity"@en ;
        rdfs:subClassOf  ocean:WaterBodyLayer ;
        rdfs:subClassOf  [ a                  owl:Restriction ;
                           owl:allValuesFrom  conc:Salinity ;
                           owl:onProperty     mrela:hasGradient
                         ] .

ocean:PelagicZone  a     owl:Class ;
        rdfs:comment     "The pelagic zone is the part of the open sea or ocean that is not near the coast." ;
        rdfs:subClassOf  ocean:OceanRegion .

ocean:LimneticZone  a    owl:Class ;
        rdfs:comment     "The limnetic zone is the well-lit, open surface waters farther from shore in a lake. It is surrounded by the littoral zone and above the profundal zone"@en ;
        rdfs:subClassOf  ocean:WaterBodyLayer ;
        rdfs:subClassOf  [ a                  owl:Restriction ;
                           owl:allValuesFrom  ocean:ProfundalZone ;
                           owl:onProperty     srela:above
                         ] .

ocean:OpenOcean  a       owl:Class ;
        rdfs:subClassOf  ocean:OceanRegion .

ocean:Bathyal  a         owl:Class ;
        rdfs:subClassOf  ocean:WaterBodyLayer .

ocean:BarrierLayer  a    owl:Class ;
        rdfs:comment     "The depth range, where it exists, between the bottom of the oceanic surface mixed layer and the thermocline, usually at a depth between 30 and 80 m."@en ;
        rdfs:subClassOf  ocean:WaterBodyLayer .

ocean:Abyssal  a  owl:Class .

ocean:Thermocline  a     owl:Class ;
        rdfs:comment     "The thermocline (sometimes metalimnion) is a layer within a body of water or air where the temperature changes rapidly with depth."@en ;
        rdfs:subClassOf  ocean:WaterBodyLayer ;
        rdfs:subClassOf  [ a                  owl:Restriction ;
                           owl:allValuesFrom  thermo:TemperatureGradient ;
                           owl:onProperty     screla:hasQuantity
                         ] .

ocean:NeriticZone  a     owl:Class ;
        rdfs:subClassOf  ocean:WaterBodyLayer .

ocean:BathypelagicZone
        a                owl:Class ;
        rdfs:subClassOf  ocean:WaterBodyLayer .

ocean:Halocline  a       owl:Class ;
        rdfs:comment     "In oceanography, a Halocline is a strong, vertical salinity gradient. Because salinity (in concert with temperature) affects the density of seawater, it can play a role in its vertical stratification."@en ;
        rdfs:subClassOf  ocean:WaterBodyLayer ;
        rdfs:subClassOf  [ a                  owl:Restriction ;
                           owl:allValuesFrom  conc:Salinity ;
                           owl:onProperty     mrela:hasGradient
                         ] .

ocean:BenthicZone  a     owl:Class ;
        rdfs:comment     "Benthic means anything associated with or happening on the bottom of a body of water. The Benthic Zone of the ocean is the bottom ocean zone ranging from the deepest parts of the ocean to the tidal affected areas. The most productive region of the benthic zone is the area over the continental margin, which is unaffected by the tides."@en ;
        rdfs:subClassOf  ocean:WaterBodyLayer ;
        rdfs:subClassOf  [ a                  owl:Restriction ;
                           owl:allValuesFrom  ocean:DemersalZone ;
                           owl:onProperty     srela:below
                         ] .

ocean:PhoticZone  a      owl:Class ;
        rdfs:comment     "The photic zone or euphotic zone is the depth of the water whether in a lake or an ocean, that is exposed to sufficient sunlight for photosynthesis to occur. The depth of the euphotic zone can be greatly affected by seasonal turbidity."@en ;
        rdfs:subClassOf  ocean:WaterBodyLayer ;
        rdfs:subClassOf  [ a                  owl:Restriction ;
                           owl:allValuesFrom  ocean:AphoticZone ;
                           owl:onProperty     srela:above
                         ] ;
        rdfs:subClassOf  [ a                  owl:Restriction ;
                           owl:allValuesFrom  bproc:Photosynthesis ;
                           owl:onProperty     rela:hasPhenomena
                         ] ;
        rdfs:subClassOf  [ a                  owl:Restriction ;
                           owl:allValuesFrom  med:Turbidity ;
                           owl:onProperty     screla:hasQuantity
                         ] .

ocean:WaterBodyLayer  a  owl:Class ;
        rdfs:subClassOf  realm:PlanetaryLayer ;
        rdfs:subClassOf  [ a                  owl:Restriction ;
                           owl:allValuesFrom  realm:Ocean ;
                           owl:onProperty     rela:hasRealm
                         ] .

ocean:DemersalZone  a    owl:Class ;
        rdfs:comment     "The demersal zone is the part of the sea or ocean (or deep lake) comprising the water column that is near to (and is significantly affected by) the seabed and the benthos. The demersal zone is just above the benthic zone and forms a layer of the larger profundal zone."@en ;
        rdfs:subClassOf  ocean:WaterBodyLayer ;
        rdfs:subClassOf  [ a                  owl:Restriction ;
                           owl:allValuesFrom  ocean:ProfundalZone ;
                           owl:onProperty     rela:hasRealm
                         ] ;
        rdfs:subClassOf  [ a                  owl:Restriction ;
                           owl:allValuesFrom  ocean:BenthicZone ;
                           owl:onProperty     srela:above
                         ] .

<>      a                owl:Ontology ;
        rdfs:label       "SWEET Ontology" ;
        owl:imports      <phenBiol> , <reprMathOperation> , <relaSpace> , <rela> , <propChemical> , <propIndex> , <relaMath> , <realmCryo> , <realm> , <relaSci> , <propSpaceDistance> , <propTemperatureGradient> ;
        owl:versionInfo  "3.1.0" .

ocean:OceanRegion  a     owl:Class ;
        rdfs:subClassOf  realm:PlanetaryRealm ;
        rdfs:subClassOf  [ a                  owl:Restriction ;
                           owl:allValuesFrom  realm:Ocean ;
                           owl:onProperty     rela:hasRealm
                         ] .

ocean:Abyss  a               owl:Class ;
        rdfs:subClassOf      ocean:WaterBodyLayer ;
        owl:equivalentClass  ocean:Abyssal .

ocean:Hadal  a           owl:Class ;
        rdfs:subClassOf  ocean:WaterBodyLayer .

ocean:AbyssopelagicZone
        a                owl:Class ;
        rdfs:subClassOf  ocean:WaterBodyLayer .

ocean:MesopelagicZone
        a                owl:Class ;
        rdfs:subClassOf  ocean:WaterBodyLayer .
