@base          <http://sweetontology.net/realm> .
@prefix comp:  <http://sweetontology.net/matrCompound/> .
@prefix obj3d: <http://sweetontology.net/reprSpaceGeometry3D/> .
@prefix astro2: <http://sweetontology.net/realmAstroBody/> .
@prefix crela: <http://sweetontology.net/relaChemical/> .
@prefix owl:   <http://www.w3.org/2002/07/owl#> .
@prefix pstate: <http://sweetontology.net/statePhysical/> .
@prefix xsd:   <http://www.w3.org/2001/XMLSchema#> .
@prefix rdfs:  <http://www.w3.org/2000/01/rdf-schema#> .
@prefix geom:  <http://sweetontology.net/reprSpaceGeometry/> .
@prefix water: <http://sweetontology.net/matrWater/> .
@prefix srela: <http://sweetontology.net/relaSpace/> .
@prefix astro: <http://sweetontology.net/realmAstroBody/> .
@prefix rdf:   <http://www.w3.org/1999/02/22-rdf-syntax-ns#> .
@prefix realm: <http://sweetontology.net/realm/> .
@prefix state: <http://sweetontology.net/state/> .
@prefix rela:  <http://sweetontology.net/rela/> .

realm:PlanetaryStructure
        a                owl:Class ;
        rdfs:subClassOf  realm:PlanetaryRealm .

realm:PlanetaryLayer  a      owl:Class ;
        rdfs:subClassOf      obj3d:Layer ;
        owl:equivalentClass  realm:GlobalPlanetaryLayer .

realm:Earth  a  astro:Planet .

realm:Land  a            owl:Class ;
        rdfs:comment     "The part of a planetary surface that is a solid"@en ;
        rdfs:subClassOf  realm:Geosphere ;
        rdfs:subClassOf  [ a               owl:Restriction ;
                           owl:hasValue    pstate:Solid ;
                           owl:onProperty  rela:hasState
                         ] .

realm:Geosphere  a       owl:Class ;
        rdfs:comment     "The term Geosphere is often used to refer to the densest (solid) parts of a planet, which consist mostly of rock and regolith [Wikipedia]"@en ;
        rdfs:subClassOf  realm:PlanetaryRealm ;
        rdfs:subClassOf  [ a                  owl:Restriction ;
                           owl:allValuesFrom  realm:PlanetarySurface ;
                           owl:onProperty     srela:hasUpperBoundary
                         ] ;
        rdfs:subClassOf  [ a               owl:Restriction ;
                           owl:hasValue    pstate:Solid ;
                           owl:onProperty  rela:hasState
                         ] .

realm:PlanetaryRealm  a  owl:Class ;
        rdfs:subClassOf  realm:Realm .

realm:PlanetarySurface
        a                    owl:Class ;
        rdfs:comment         "The surface of the planet defined by solid and/or liquid layers"@en ;
        rdfs:subClassOf      realm:PlanetarySurfaceLevel ;
        owl:equivalentClass  realm:Subaerial .

realm:Ring  a            owl:Class ;
        rdfs:subClassOf  realm:PlanetaryRealm ;
        rdfs:subClassOf  [ a               owl:Restriction ;
                           owl:hasValue    pstate:Solid ;
                           owl:onProperty  rela:hasState
                         ] .

realm:PlanetarySurfaceLevel
        a                    owl:Class ;
        rdfs:comment         "A qusai-horizontal surface spanning all or part of a planet that corresponds to a constant value of some parameter"@en ;
        rdfs:subClassOf      realm:CriticalZone , geom:Surface ;
        owl:equivalentClass  realm:PlanetaryBoundary .

realm:Subaerial  a  owl:Class .

realm:CriticalZone  a    owl:Class ;
        rdfs:subClassOf  realm:PlanetaryRealm .

realm:GlobalPlanetaryLayer
        a       owl:Class .

realm:PlanetaryBoundary
        a       owl:Class .

realm:Hydrosphere  a     owl:Class ;
        rdfs:comment     "A hydrosphere in physical geography describes the combined mass of water found on, under, and over the surface of a planet. [Wikipedia]"@en ;
        rdfs:subClassOf  realm:PlanetaryRealm ;
        rdfs:subClassOf  [ a               owl:Restriction ;
                           owl:hasValue    comp:Water ;
                           owl:onProperty  crela:hasSubstance
                         ] .

realm:Cryosphere  a      owl:Class ;
        rdfs:comment     "The cryosphere collectively describes the portions of a planetary surface in frozen form, including sea ice, lake ice, river ice, snow cover, glaciers, ice caps and ice sheets, and frozen ground (which includes permafrost).  [Wikipedia]"@en ;
        rdfs:subClassOf  realm:Hydrosphere ;
        rdfs:subClassOf  [ a                  owl:Restriction ;
                           owl:allValuesFrom  realm:PlanetarySurface ;
                           owl:onProperty     srela:hasUpperBoundary
                         ] ;
        rdfs:subClassOf  [ a                  owl:Restriction ;
                           owl:allValuesFrom  water:Ice ;
                           owl:onProperty     crela:hasSubstance
                         ] .

realm:Atmosphere  a      owl:Class ;
        rdfs:comment     "An atmosphere is a layer of gases that may surround a material body of sufficient mass,[1] by the gravity of the body, and are retained for a longer duration if gravity is high and the atmosphere's temperature is low. [Wikipedia]"@en ;
        rdfs:subClassOf  realm:PlanetaryRealm ;
        rdfs:subClassOf  [ a                  owl:Restriction ;
                           owl:allValuesFrom  realm:PlanetarySurface ;
                           owl:onProperty     srela:hasLowerBoundary
                         ] ;
        rdfs:subClassOf  [ a               owl:Restriction ;
                           owl:hasValue    pstate:Gas ;
                           owl:onProperty  rela:hasState
                         ] .

realm:Realm  a  owl:Class .

realm:Ocean  a           owl:Class ;
        rdfs:comment     "An ocean is a major body of saline water, and a principal component of the hydrosphere. [Wikipedia]"@en ;
        rdfs:subClassOf  realm:Hydrosphere ;
        rdfs:subClassOf  [ a                  owl:Restriction ;
                           owl:allValuesFrom  realm:PlanetarySurface ;
                           owl:onProperty     srela:hasUpperBoundary
                         ] ;
        rdfs:subClassOf  [ a               owl:Restriction ;
                           owl:hasValue    pstate:Liquid ;
                           owl:onProperty  rela:hasState
                         ] .

<>      a                owl:Ontology ;
        rdfs:label       "SWEET Ontology" ;
        owl:imports      <relaChemical> , <reprSpaceGeometry3D> , <relaSpace> , <realmAstroBody> , <state> , <rela> , <statePhysical> , <matrCompound> , <reprSpaceGeometry> , <matrWater> ;
        owl:versionInfo  "3.1.0" .
