@base          <http://sweetontology.net/realmLandform> .
@prefix vis:   <http://sweetontology.net/stateVisibility/> .
@prefix srela: <http://sweetontology.net/relaSpace/> .
@prefix obj3d: <http://sweetontology.net/reprSpaceGeometry3D/> .
@prefix rdf:   <http://www.w3.org/1999/02/22-rdf-syntax-ns#> .
@prefix owl:   <http://www.w3.org/2002/07/owl#> .
@prefix obj:   <http://sweetontology.net/reprSpaceGeometry/> .
@prefix prela: <http://sweetontology.net/relaPhysical/> .
@prefix xsd:   <http://www.w3.org/2001/XMLSchema#> .
@prefix land:  <http://sweetontology.net/realmLandform/> .
@prefix rdfs:  <http://www.w3.org/2000/01/rdf-schema#> .

land:Prarie  a           owl:Class ;
        rdfs:subClassOf  land:Plain .

land:RockyPitFloorCrater
        a                owl:Class ;
        rdfs:subClassOf  land:PitCrater .

land:Dryland  a          owl:Class ;
        rdfs:subClassOf  land:LandRegion .

land:Lamination  a       owl:Class ;
        rdfs:subClassOf  land:Landform .

land:PitCrater  a        owl:Class ;
        rdfs:subClassOf  land:Crater .

land:SurfaceRegion  a  owl:Class .

land:Landscape  a        owl:Class ;
        rdfs:comment     "A landscape comprises the visible features of an area of land, including physical elements such as landforms, living elements of flora and fauna, abstract elements such as lighting and weather conditions, and human elements, for instance human activity or the built environment. Landscape may also signify the objects around one in a building."@en ;
        rdfs:subClassOf  land:Landform .

land:DeflationZone  a    owl:Class ;
        rdfs:subClassOf  land:LandRegion .

land:ImpactCrater  a     owl:Class ;
        rdfs:subClassOf  land:Crater .

land:Spall  a            owl:Class ;
        rdfs:subClassOf  land:Landform .

land:LandRegion  a  owl:Class .

land:Land  a                 owl:Class ;
        rdfs:subClassOf      obj:Region ;
        owl:equivalentClass  land:LandSurface , land:SurfaceRegion , land:LandRegion .

land:Mare  a             owl:Class ;
        rdfs:subClassOf  land:Plain ;
        rdfs:subClassOf  [ a               owl:Restriction ;
                           owl:hasValue    vis:Dark ;
                           owl:onProperty  prela:hasVisibility
                         ] .

land:ComplexCrater  a    owl:Class ;
        rdfs:subClassOf  land:Crater .

land:Highland  a         owl:Class ;
        rdfs:subClassOf  land:Landform .

land:ImpactBasin  a      owl:Class ;
        rdfs:subClassOf  land:Landform .

land:Landform  a         owl:Class ;
        rdfs:comment     "A landform comprises a geomorphological unit, and is largely defined by its surface form and location in the landscape, as part of the terrain, and as such, is typically an element of topography. Landforms are categorised by features such as elevation, slope, orientation, stratification, rock exposure, and soil type. They include berms, mounds, hills, cliffs, valleys, rivers and numerous other elements."@en ;
        rdfs:subClassOf  land:LandRegion .

land:PedestalCrater  a   owl:Class ;
        rdfs:subClassOf  land:Crater .

land:Plain  a            owl:Class ;
        rdfs:subClassOf  land:Landform ;
        rdfs:subClassOf  [ a               owl:Restriction ;
                           owl:hasValue    <stateSpaceConfiguration/Flat> ;
                           owl:onProperty  srela:hasSpatialConfiguration
                         ] .

land:LandSurface  a  owl:Class .

land:DebrisBasin  a      owl:Class ;
        rdfs:subClassOf  land:LandRegion .

land:ShatterCone  a      owl:Class ;
        rdfs:subClassOf  land:Landform .

land:Crater  a           owl:Class ;
        rdfs:subClassOf  obj3d:Cavity , land:Landform .

land:LandCover  a        owl:Class ;
        rdfs:comment     "Land cover is the physical material at the surface of the earth. Land covers include grass, asphalt, trees, bare ground, water, etc. [Wikipedia]"@en ;
        rdfs:subClassOf  land:Landform .

land:Lowland  a           owl:Class ;
        rdfs:subClassOf   land:Landform ;
        owl:disjointWith  land:Highland .

land:Field  a            owl:Class ;
        rdfs:comment     "Field (agriculture), an area of land used to cultivate crops, or to keep livestock [Wikipedia]"@en ;
        rdfs:subClassOf  land:Landform .

land:CentralCreekCrater
        a                owl:Class ;
        rdfs:subClassOf  land:Crater .

land:Continent  a        owl:Class ;
        rdfs:comment     "A continent is one of several large landmasses. [Wikipedia]"@en ;
        rdfs:subClassOf  land:LandRegion .

<>      a                owl:Ontology ;
        rdfs:label       "SWEET Ontology" ;
        owl:imports      <relaSpace> , <relaPhysical> , <stateVisibility> , <reprSpaceGeometry3D> , <reprSpaceGeometry> ;
        owl:versionInfo  "3.1.0" .
