@base          <http://sweetontology.net/realmGeolOrogen> .
@prefix chem:  <http://sweetontology.net/matr/> .
@prefix crela: <http://sweetontology.net/relaChemical/> .
@prefix def:   <http://sweetontology.net/phenSolid/> .
@prefix owl:   <http://www.w3.org/2002/07/owl#> .
@prefix prela: <http://sweetontology.net/relaPhysical/> .
@prefix petr:  <http://sweetontology.net/matrRock/> .
@prefix tecp:  <http://sweetontology.net/phenGeolTectonic/> .
@prefix xsd:   <http://www.w3.org/2001/XMLSchema#> .
@prefix rdfs:  <http://www.w3.org/2000/01/rdf-schema#> .
@prefix basin: <http://sweetontology.net/realmGeolBasin/> .
@prefix geol:  <http://sweetontology.net/phenGeol/> .
@prefix geom:  <http://sweetontology.net/reprSpaceGeometry/> .
@prefix dir:   <http://sweetontology.net/propSpaceDirection/> .
@prefix geolr: <http://sweetontology.net/realmGeol/> .
@prefix oro:   <http://sweetontology.net/realmGeolOrogen/> .
@prefix ign:   <http://sweetontology.net/matrRockIgneous/> .
@prefix srela: <http://sweetontology.net/relaSpace/> .
@prefix tec:   <http://sweetontology.net/realmLandTectonic/> .
@prefix phen:  <http://sweetontology.net/phen/> .
@prefix rdf:   <http://www.w3.org/1999/02/22-rdf-syntax-ns#> .
@prefix geomor: <http://sweetontology.net/phenGeolGeomorphology/> .
@prefix rela:  <http://sweetontology.net/rela/> .

oro:RearArc  a               owl:Class ;
        owl:equivalentClass  oro:BackArc .

oro:ArcAxis  a           owl:Class ;
        rdfs:comment     "In a Back-arc basin the arc axis is the line where spreading occurs on the overlying plate of the subduction zone. [Wikipedia]"@en ;
        rdfs:subClassOf  dir:Axis .

oro:RetroArc  a              owl:Class ;
        owl:equivalentClass  oro:BackArc .

oro:RemnantArc  a        owl:Class ;
        rdfs:comment     "The remnant arc is what is left on the rear side of the speading zone as athe basin broadens. [Wikipedia]"@en ;
        rdfs:subClassOf  oro:Arc .

oro:BackArc  a           owl:Class ;
        rdfs:comment     "Back-arc basins (or retro-arc basins) are geologic features, submarine basins associated with island arcs and subduction zones. They are found at some convergent plate boundaries, presently concentrated in the Western Pacific ocean. [Wikipedia]"@en ;
        rdfs:subClassOf  oro:Arc .

oro:ForeArc  a           owl:Class ;
        rdfs:comment     "A forearc is a depression in the sea floor located between a subduction zone and an associated volcanic arc. It is typically filled with sediments from the adjacent landmass and the island arc in addition to trapped oceanic crustal material.  [Wikipedia]"@en ;
        rdfs:subClassOf  tec:SupraSubductionZoneComplex , oro:Arc .

oro:Orogen  a            owl:Class ;
        rdfs:subClassOf  geolr:GeologicProvince ;
        rdfs:subClassOf  [ a                   owl:Restriction ;
                           owl:onProperty      crela:hasSubstance ;
                           owl:someValuesFrom  petr:Melange
                         ] ;
        rdfs:subClassOf  [ a                   owl:Restriction ;
                           owl:onProperty      rela:hasPhenomena ;
                           owl:someValuesFrom  def:Deformation
                         ] ;
        rdfs:subClassOf  [ a                   owl:Restriction ;
                           owl:onProperty      rela:hasPhenomena ;
                           owl:someValuesFrom  geol:Orogeny
                         ] ;
        rdfs:subClassOf  [ a                   owl:Restriction ;
                           owl:onProperty      rela:hasPhenomena ;
                           owl:someValuesFrom  geol:OrogenicCollapse
                         ] ;
        rdfs:subClassOf  [ a                   owl:Restriction ;
                           owl:onProperty      prela:hasPlanetaryStructure ;
                           owl:someValuesFrom  tec:Suture
                         ] ;
        rdfs:subClassOf  [ a                   owl:Restriction ;
                           owl:onProperty      prela:hasPlanetaryStructure ;
                           owl:someValuesFrom  tec:ThrustSystem
                         ] ;
        rdfs:subClassOf  [ a                   owl:Restriction ;
                           owl:onProperty      prela:hasPlanetaryStructure ;
                           owl:someValuesFrom  basin:ForelandBasin
                         ] ;
        rdfs:subClassOf  [ a                   owl:Restriction ;
                           owl:onProperty      prela:hasPlanetaryStructure ;
                           owl:someValuesFrom  tecp:Terrane
                         ] .

<>      a                owl:Ontology ;
        rdfs:label       "SWEET Ontology" ;
        owl:imports      <phenGeolTectonic> , <relaSpace> , <relaChemical> , <realmGeolBasin> , <phen> , <realmGeol> , <matrRock> , <matrRockIgneous> , <reprSpaceGeometry> , <phenSolid> , <relaPhysical> , <propSpaceDirection> , <rela> , <phenGeol> , <matr> , <realmLandTectonic> , <phenGeolGeomorphology> ;
        owl:versionInfo  "3.1.0" .

oro:Arc  a               owl:Class ;
        rdfs:subClassOf  geolr:GeologicFeature , geom:Arc .

oro:MagmaticArc  a       owl:Class ;
        rdfs:subClassOf  oro:Arc ;
        rdfs:subClassOf  [ a                  owl:Restriction ;
                           owl:allValuesFrom  oro:ArcAxis ;
                           owl:onProperty     srela:hasAxis
                         ] ;
        rdfs:subClassOf  [ a                   owl:Restriction ;
                           owl:onProperty      prela:hasPlanetaryStructure ;
                           owl:someValuesFrom  oro:RearArc
                         ] ;
        rdfs:subClassOf  [ a                   owl:Restriction ;
                           owl:onProperty      prela:hasPlanetaryStructure ;
                           owl:someValuesFrom  oro:ForeArc
                         ] .
