@base          <http://sweetontology.net/realmLandFluvial> .
@prefix obj3d: <http://sweetontology.net/reprSpaceGeometry3D/> .
@prefix phen:  <http://sweetontology.net/phen/> .
@prefix rdf:   <http://www.w3.org/1999/02/22-rdf-syntax-ns#> .
@prefix owl:   <http://www.w3.org/2002/07/owl#> .
@prefix fluv:  <http://sweetontology.net/realmLandFluvial/> .
@prefix xsd:   <http://www.w3.org/2001/XMLSchema#> .
@prefix land:  <http://sweetontology.net/realmLandform/> .
@prefix rdfs:  <http://www.w3.org/2000/01/rdf-schema#> .
@prefix geol:  <http://sweetontology.net/phenGeol/> .
@prefix geom:  <http://sweetontology.net/phenGeolGeomorphology/> .
@prefix rela:  <http://sweetontology.net/rela/> .

fluv:DrainageBasin  a  owl:Class .

<>      a                owl:Ontology ;
        rdfs:label       "SWEET Ontology" ;
        owl:imports      <rela> , <phen> , <phenGeolGeomorphology> , <phenGeol> , <realmLandform> , <reprSpaceGeometry3D> ;
        owl:versionInfo  "3.1.0" .

fluv:Wash  a             owl:Class ;
        rdfs:subClassOf  fluv:PiedmontSlope .

fluv:Wall  a             owl:Class ;
        rdfs:subClassOf  fluv:FluvialLandform .

fluv:AlluvialPlain  a    owl:Class ;
        rdfs:subClassOf  fluv:PiedmontSlope , fluv:FluvialPlain .

fluv:SaltLake  a             owl:Class ;
        owl:equivalentClass  fluv:Playa .

fluv:PiedmontSlope  a    owl:Class ;
        rdfs:subClassOf  fluv:FluvialLandform .

fluv:Sabkha  a           owl:Class ;
        rdfs:subClassOf  fluv:SaltFlat .

fluv:RiverBed  a         owl:Class ;
        rdfs:subClassOf  fluv:Bedform .

fluv:SaltFlat  a         owl:Class ;
        rdfs:subClassOf  fluv:FluvialLandform .

fluv:LacustrinePlain  a  owl:Class ;
        rdfs:subClassOf  fluv:FluvialPlain .

fluv:Turbidite  a        owl:Class ;
        rdfs:subClassOf  fluv:FluvialLandform .

fluv:ScrollPlain  a      owl:Class ;
        rdfs:subClassOf  fluv:FluvialPlain .

fluv:Gorge  a            owl:Class ;
        rdfs:subClassOf  fluv:Canyon .

fluv:FluvialPlain  a     owl:Class ;
        rdfs:subClassOf  land:Plain .

fluv:DryLake  a              owl:Class ;
        owl:equivalentClass  fluv:Playa .

fluv:Bedform  a          owl:Class ;
        rdfs:subClassOf  fluv:FluvialLandform .

fluv:Watershed  a            owl:Class ;
        rdfs:comment         "A watershed refers to a divide that separates one drainage area from another drainage area. However, in the US and Canada, the term is often used to mean a drainage basin or catchment area itself. [Wikipedia]"@en ;
        rdfs:subClassOf      land:LandRegion ;
        owl:equivalentClass  fluv:DrainageBasin .

fluv:Catchment  a        owl:Class ;
        rdfs:comment     "A catchment, or drainage basin, is an extent of land where water from precipitation drains into a body of water [Wikipedia]"@en ;
        rdfs:subClassOf  fluv:Watershed .

fluv:Playa  a            owl:Class ;
        rdfs:subClassOf  fluv:FluvialPlain .

fluv:Tunnel  a           owl:Class ;
        rdfs:subClassOf  obj3d:Tube , fluv:FluvialLandform .

fluv:AlluvialFan  a      owl:Class ;
        rdfs:subClassOf  fluv:PiedmontSlope .

fluv:Trench  a           owl:Class ;
        rdfs:comment     "A trench is a type of excavation or depression in the ground. Trenches are generally defined by being deeper than they are wide (as opposed to a wider gully or ditch), and by being narrow compared to their length (as opposed to a simple hole). Trenches are a natural feature in many landscapes. Some are created by rivers in flow (which may have long since fallen dry), others are features created by geological movement, such as oceanic trenches. The latter form is relatively deep, linear and narrow, and is formed by plate subduction. [Wikipedia]"@en ;
        rdfs:subClassOf  fluv:Canyon .

fluv:Ripple  a           owl:Class ;
        rdfs:subClassOf  fluv:Bedform .

fluv:Bajada  a           owl:Class ;
        rdfs:subClassOf  fluv:PiedmontSlope .

fluv:FloodPlain  a       owl:Class ;
        rdfs:subClassOf  fluv:FluvialPlain .

fluv:Gulley  a           owl:Class ;
        rdfs:subClassOf  fluv:FluvialLandform .

fluv:FluvialLandform  a  owl:Class ;
        rdfs:subClassOf  land:Landform .

fluv:Alluvial  a         owl:Class ;
        rdfs:comment     "The process of depositing soil or sediments by a river or other running water. [Wikipedia]"@en ;
        rdfs:subClassOf  geom:SedimentFormation .

fluv:KarstLandform  a    owl:Class ;
        rdfs:comment     "Karst topography is a landscape shaped by the dissolution of a layer or layers of soluble bedrock, usually carbonate rock such as limestone or dolomite. [Wikipedia]"@en ;
        rdfs:subClassOf  land:Landform ;
        rdfs:subClassOf  [ a                   owl:Restriction ;
                           owl:onProperty      rela:hasPhenomena ;
                           owl:someValuesFrom  geom:Karst
                         ] .

fluv:Valley  a           owl:Class ;
        rdfs:comment     "A valley (also called a vale, dale, glen or strath and near or in Appalachia, a draw) is a depression with predominant extent in one direction. [Wikipedia]"@en ;
        rdfs:subClassOf  fluv:FluvialLandform .

fluv:Cave  a             owl:Class ;
        rdfs:subClassOf  obj3d:Cavity , fluv:FluvialLandform ;
        rdfs:subClassOf  [ a                   owl:Restriction ;
                           owl:onProperty      rela:contains ;
                           owl:someValuesFrom  fluv:Tunnel
                         ] .

fluv:Canyon  a           owl:Class ;
        rdfs:comment     "A canyon, or gorge, is a deep valley between cliffs often carved from the landscape by a river. Most canyons were formed by a process of long-time erosion from a plateau level. [Wikipedia]"@en ;
        rdfs:subClassOf  fluv:FluvialLandform .
