@base          <http://sweetontology.net/realmAtmoWeather> .
@prefix owl:   <http://www.w3.org/2002/07/owl#> .
@prefix planet: <http://sweetontology.net/realm/> .
@prefix prela: <http://sweetontology.net/relaPhysical/> .
@prefix xsd:   <http://www.w3.org/2001/XMLSchema#> .
@prefix rdfs:  <http://www.w3.org/2000/01/rdf-schema#> .
@prefix ht:    <http://sweetontology.net/propSpaceHeight/> .
@prefix prec:  <http://sweetontology.net/phenAtmoPrecipitation/> .
@prefix rdf:   <http://www.w3.org/1999/02/22-rdf-syntax-ns#> .
@prefix weat:  <http://sweetontology.net/realmAtmoWeather/> .
@prefix inst:  <http://sweetontology.net/phenFluidInstability/> .
@prefix atmo:  <http://sweetontology.net/realmAtmo/> .
@prefix atmp:  <http://sweetontology.net/phenAtmo/> .
@prefix rela:  <http://sweetontology.net/rela/> .
@prefix statec: <http://sweetontology.net/procStateChange/> .

weat:ConvectiveCondensationLevel
        a                owl:Class ;
        rdfs:comment     "On a thermodynamic diagram, the point of intersection of a sounding curve (representing the vertical distribution of temperature in an atmospheric column) with the saturation mixing ratio line corresponding to the average mixing ratio in the surface layer."@en ;
        rdfs:subClassOf  weat:CondensationLevel .

weat:CondensationLevel
        a                owl:Class ;
        rdfs:comment     "Level at which water vapor to condense" ;
        rdfs:label       "Condensation Level" ;
        rdfs:subClassOf  ht:Level .

weat:SnowGeneratingLevel
        a                owl:Class ;
        rdfs:comment     "A layer in the middle or upper troposphere in widespread precipitation in which ice crystals form in small convective cells and fall to lower altitudes."@en ;
        rdfs:subClassOf  planet:PlanetarySurfaceLevel ;
        rdfs:subClassOf  [ a                  owl:Restriction ;
                           owl:allValuesFrom  prec:Snowfall ;
                           owl:onProperty     rela:hasPhenomena
                         ] .

<>      a                owl:Ontology ;
        rdfs:label       "SWEET Ontology" ;
        owl:imports      <propSpaceHeight> , <procStateChange> , <relaPhysical> , <realmAtmo> , <phenFluidInstability> , <phenAtmo> , <rela> , <phenAtmoPrecipitation> , <realm> ;
        owl:versionInfo  "3.1.0" .

weat:CloudTop  a         owl:Class ;
        rdfs:subClassOf  planet:PlanetaryBoundary .

weat:MeltingLayer  a     owl:Class ;
        rdfs:comment     "The altitude interval throughout which ice-phase precipitation melts as it descends. The top of the melting layer is the melting level. The melting layer may be several hundred meters deep, reflecting the time it takes for all the hydrometeors to undergo the transition from solid to liquid phase. The temperature of the melting layer is typically 0?C or slightly warmer. See bright band."@en ;
        rdfs:subClassOf  planet:PlanetaryLayer ;
        rdfs:subClassOf  [ a                  owl:Restriction ;
                           owl:allValuesFrom  statec:Melting ;
                           owl:onProperty     prela:hasStateChange
                         ] .

weat:ZoneOfMaximumPrecipitation
        a                owl:Class ;
        rdfs:comment     "The elevation band on a mountain or orographic barrier that receives the greatest precipitation for a seasonal or annual average."@en ;
        rdfs:subClassOf  atmo:AtmosphereLayer .

weat:MeltingLevel  a     owl:Class ;
        rdfs:comment     "The altitude at which ice crystals and snowflakes begin to melt as they descend through the atmosphere. In cloud physics and in radar meteorology, this is the accepted term for the 0?C constant-temperature surface (see bright band). It is physically more apt than the corresponding operational term, freezing level, for melting of pure ice must begin very near 0?C, but freezing of liquid water can occur over a broad range of temperatures (between 0? and -40?C; see supercooling). See also freezing point, ice point, melting point."@en ;
        rdfs:subClassOf  planet:PlanetarySurfaceLevel ;
        rdfs:subClassOf  [ a                  owl:Restriction ;
                           owl:allValuesFrom  statec:Melting ;
                           owl:onProperty     prela:hasStateChange
                         ] .

weat:FreezingLevel  a    owl:Class ;
        rdfs:subClassOf  atmp:MeteorologicalPhenomena , planet:PlanetarySurfaceLevel .

weat:ConvectiveCloudBase
        a                owl:Class ;
        rdfs:subClassOf  planet:PlanetaryBoundary .

weat:LevelOfFreeConvection
        a       owl:Class .

weat:FreeConvectiveLayer
        a                owl:Class ;
        rdfs:subClassOf  atmo:AtmosphereLayer ;
        rdfs:subClassOf  [ a                  owl:Restriction ;
                           owl:allValuesFrom  inst:FreeInstability ;
                           owl:onProperty     rela:hasPhenomena
                         ] .

weat:AdiabaticCondensationLevel
        a                owl:Class ;
        rdfs:subClassOf  weat:CondensationLevel .

weat:MaximumWindSpeedLevel
        a                owl:Class ;
        rdfs:subClassOf  planet:PlanetarySurfaceLevel .

weat:ConvectiveCloudTop
        a                owl:Class ;
        rdfs:subClassOf  planet:PlanetaryBoundary .

weat:LFC  a                  owl:Class ;
        rdfs:comment         "Level of free convection" ;
        rdfs:subClassOf      planet:PlanetarySurfaceLevel ;
        owl:equivalentClass  weat:LevelOfFreeConvection .

weat:CloudBase  a        owl:Class ;
        rdfs:subClassOf  planet:PlanetaryBoundary .
