@base          <http://sweetontology.net/reprSciModel> .
@prefix repr:  <http://sweetontology.net/repr/> .
@prefix res:   <http://sweetontology.net/humanResearch/> .
@prefix mod:   <http://sweetontology.net/reprSciModel/> .
@prefix rdf:   <http://www.w3.org/1999/02/22-rdf-syntax-ns#> .
@prefix owl:   <http://www.w3.org/2002/07/owl#> .
@prefix atmo:  <http://sweetontology.net/phenAtmo/> .
@prefix xsd:   <http://www.w3.org/2001/XMLSchema#> .
@prefix rdfs:  <http://www.w3.org/2000/01/rdf-schema#> .
@prefix rela:  <http://sweetontology.net/rela/> .

mod:WeatherForecast  a   owl:Class ;
        rdfs:subClassOf  mod:Forecast ;
        rdfs:subClassOf  [ a                  owl:Restriction ;
                           owl:allValuesFrom  atmo:Weather ;
                           owl:onProperty     rela:hasPhenomena
                         ] .

mod:SpectralElement  a   owl:Class ;
        rdfs:subClassOf  mod:Model .

mod:ReactionPathModel
        a                owl:Class ;
        rdfs:comment     "A simulation approach to studying the chemical evolution of a (natural) system."@en ;
        rdfs:subClassOf  mod:Model .

mod:BoussinesqApproximation
        a                owl:Class ;
        rdfs:comment     "An approximation to the dynamical equations of motion whereby density is assumed to be constant except in the buoyancy term of the vertical velocity equation."@en ;
        rdfs:subClassOf  mod:PhysicalApproximation .

mod:Hypothesis  a        owl:Class ;
        rdfs:subClassOf  res:ExperimentActivity .

mod:FluxCorrection  a    owl:Class ;
        rdfs:subClassOf  mod:PhysicalApproximation .

<>      a                owl:Ontology ;
        rdfs:label       "SWEET Ontology" ;
        owl:imports      <phenAtmo> , <rela> , <repr> , <humanResearch> ;
        owl:versionInfo  "3.1.0" .

mod:Theory  a                owl:Class ;
        rdfs:subClassOf      res:ExperimentActivity ;
        owl:equivalentClass  mod:Theoretical .

mod:Parcel  a            owl:Class ;
        rdfs:comment     "An imaginary volume of fluid to which may be assigned various thermodynamic and kinematic quantities."@en ;
        rdfs:subClassOf  mod:Model .

mod:Estimate  a          owl:Class ;
        rdfs:subClassOf  mod:Prediction .

mod:ScientificModel  a  owl:Class .

mod:Prediction  a  owl:Class .

mod:GeneralCirculationModel
        a                    owl:Class ;
        rdfs:subClassOf      mod:Model ;
        owl:equivalentClass  mod:GCM .

mod:Parameterization  a  owl:Class ;
        rdfs:subClassOf  mod:Model .

mod:ClimateModel  a      owl:Class ;
        rdfs:subClassOf  mod:Model .

mod:Spectral  a          owl:Class ;
        rdfs:subClassOf  mod:Model .

mod:PhysicalApproximation
        a                owl:Class ;
        rdfs:subClassOf  mod:Model .

mod:GCM  a      owl:Class .

mod:Predict  a               owl:Class ;
        rdfs:subClassOf      res:ExperimentActivity ;
        owl:equivalentClass  mod:Prediction .

mod:ExtendedForecast  a  owl:Class ;
        rdfs:comment     "A forecast of weather conditions for a period extending beyond three or more days from the day of issuance."@en ;
        rdfs:subClassOf  mod:WeatherForecast .

mod:EnsembleForecast  a  owl:Class ;
        rdfs:comment     "A set of different forecasts all valid at the same forecast time(s)."@en ;
        rdfs:subClassOf  mod:Forecast .

mod:MixingScheme  a      owl:Class ;
        rdfs:subClassOf  mod:Parameterization .

mod:Forecast  a          owl:Class ;
        rdfs:subClassOf  mod:Prediction .

mod:Model  a                 owl:Class ;
        rdfs:subClassOf      repr:Representation ;
        owl:equivalentClass  mod:ScientificModel .

mod:RigidLidApproximation
        a                owl:Class ;
        rdfs:subClassOf  mod:PhysicalApproximation .

mod:Theoretical  a  owl:Class .

mod:FiniteElement  a     owl:Class ;
        rdfs:subClassOf  mod:Model .
