@base          <http://sweetontology.net/reprSciLaw> .
@prefix law:   <http://sweetontology.net/reprSciLaw/> .
@prefix mod:   <http://sweetontology.net/reprSciModel/> .
@prefix pres:  <http://sweetontology.net/propPressure/> .
@prefix velo:  <http://sweetontology.net/propSpeed/> .
@prefix owl:   <http://www.w3.org/2002/07/owl#> .
@prefix pstate: <http://sweetontology.net/statePhysical/> .
@prefix xsd:   <http://www.w3.org/2001/XMLSchema#> .
@prefix rdfs:  <http://www.w3.org/2000/01/rdf-schema#> .
@prefix wave:  <http://sweetontology.net/procWave/> .
@prefix prec:  <http://sweetontology.net/phenAtmoPrecipitation/> .
@prefix rdf:   <http://www.w3.org/1999/02/22-rdf-syntax-ns#> .
@prefix know:  <http://sweetontology.net/repr/> .
@prefix rela:  <http://sweetontology.net/rela/> .
@prefix wind:  <http://sweetontology.net/phenAtmoWind/> .

law:PhysicalLaw  a       owl:Class ;
        rdfs:subClassOf  know:Knowledge .

law:DarcysLaw  a         owl:Class ;
        rdfs:subClassOf  law:EmpiricalLaw .

law:EmpiricalLaw  a      owl:Class ;
        rdfs:subClassOf  know:Knowledge .

law:Z_RRelation  a       owl:Class ;
        rdfs:comment     "A relationship between radar reflectivity factor Z (mm6 m-3) and rain rate R (mm h-1)."@en ;
        rdfs:subClassOf  law:EmpiricalLaw ;
        rdfs:subClassOf  [ a                  owl:Restriction ;
                           owl:allValuesFrom  prec:Rainfall ;
                           owl:onProperty     rela:hasPhenomena
                         ] .

law:BernoulliTheorem  a  owl:Class ;
        rdfs:comment     "As originally formulated, a statement of the conservation of energy (per unit mass) for an inviscid fluid in steady motion."@en ;
        rdfs:subClassOf  law:PhysicalLaw ;
        rdfs:subClassOf  [ a                   owl:Restriction ;
                           owl:onProperty      rela:hasProperty ;
                           owl:someValuesFrom  velo:Velocity
                         ] .

<>      a                owl:Ontology ;
        rdfs:label       "SWEET Ontology" ;
        owl:imports      <phenAtmoWind> , <propPressure> , <repr> , <propSpeed> , <procWave> , <reprSciModel> , <phenAtmoPrecipitation> , <statePhysical> , <rela> ;
        owl:versionInfo  "3.1.0" .

law:HookesLaw  a         owl:Class ;
        rdfs:subClassOf  law:EmpiricalLaw .

law:WalthersLaw  a       owl:Class ;
        rdfs:subClassOf  law:EmpiricalLaw .

law:BouguerLaw  a        owl:Class ;
        rdfs:comment     "Attenuation of a beam of light by an optically homogeneous (transparent) medium." ;
        rdfs:subClassOf  law:EmpiricalLaw ;
        rdfs:subClassOf  [ a                  owl:Restriction ;
                           owl:allValuesFrom  wave:Attenuation ;
                           owl:onProperty     rela:hasProcess
                         ] .

law:MathematicalTheorem
        a                owl:Class ;
        rdfs:subClassOf  know:Knowledge .

law:IdealGasLaw  a       owl:Class ;
        rdfs:subClassOf  law:PhysicalLaw ;
        rdfs:subClassOf  [ a               owl:Restriction ;
                           owl:hasValue    pstate:Gas ;
                           owl:onProperty  rela:hasState
                         ] .

law:StokesLaw  a         owl:Class ;
        rdfs:subClassOf  mod:PhysicalApproximation .

law:BuysBallotLaw  a     owl:Class ;
        rdfs:comment     "A law describing the relationship of the horizontal wind direction in the atmosphere to the pressure distribution."@en ;
        rdfs:subClassOf  law:EmpiricalLaw ;
        rdfs:subClassOf  [ a                   owl:Restriction ;
                           owl:onProperty      rela:hasProperty ;
                           owl:someValuesFrom  pres:Pressure
                         ] ;
        rdfs:subClassOf  [ a                  owl:Restriction ;
                           owl:allValuesFrom  wind:Wind ;
                           owl:onProperty     rela:hasPhenomena
                         ] .
