@base          <http://sweetontology.net/stateSystem> .
@prefix rdf:   <http://www.w3.org/1999/02/22-rdf-syntax-ns#> .
@prefix owl:   <http://www.w3.org/2002/07/owl#> .
@prefix sstate: <http://sweetontology.net/stateSystem/> .
@prefix xsd:   <http://www.w3.org/2001/XMLSchema#> .
@prefix rdfs:  <http://www.w3.org/2000/01/rdf-schema#> .
@prefix state: <http://sweetontology.net/state/> .
@prefix ordi:  <http://sweetontology.net/propOrdinal/> .
@prefix screla: <http://sweetontology.net/relaSci/> .
@prefix rela:  <http://sweetontology.net/rela/> .

sstate:Eruptive  a             ordi:ActivityLevel ;
        screla:moreActiveThan  sstate:Inactive .

sstate:Chaotic  a   sstate:SystemState ;
        owl:sameAs  sstate:Chaos .

sstate:Random  a  sstate:SystemState .

sstate:Quiet  a                ordi:ActivityLevel ;
        screla:moreActiveThan  sstate:Extinct .

<>      a                owl:Ontology ;
        rdfs:label       "SWEET Ontology" ;
        owl:imports      <state> , <propOrdinal> , <rela> , <relaSci> ;
        owl:versionInfo  "3.1.0" .

sstate:Natural  a  sstate:SystemState .

sstate:Reversible  a  sstate:SystemState .

sstate:Inactive  a  ordi:ActivityLevel .

sstate:Critical  a  sstate:SystemState .

sstate:Hyperactive  a          ordi:ActivityLevel ;
        screla:moreActiveThan  sstate:Active .

sstate:Balanced  a  sstate:SystemState ;
        owl:sameAs  sstate:Balance .

sstate:Irreversible  a     sstate:SystemState ;
        owl:differentFrom  sstate:Reversible .

sstate:Balance  a  sstate:SystemState .

sstate:Independent  a  sstate:SystemState .

sstate:Incomplete  a       sstate:SystemState ;
        owl:differentFrom  sstate:Complete .

sstate:Excess  a         owl:Class ;
        rdfs:subClassOf  sstate:SystemState .

sstate:Stochastic  a       sstate:SystemState ;
        owl:differentFrom  sstate:Deterministic .

sstate:Stable  a             owl:Class ;
        rdfs:comment         "The characteristic of a system if sufficiently small disturbances have only small effects, either decreasing in amplitude or oscillating periodically; it is asymptotically stable if the effect of small disturbances vanishes for long time periods."@en ;
        rdfs:subClassOf      sstate:SystemState ;
        owl:equivalentClass  sstate:Stability .

sstate:Equilibrium  a  sstate:SystemState ;
        rdfs:comment  "In mechanics, a state in which the vector sum of all forces, that is, the acceleration vector, is zero.\nIn hydrodynamics, it is usually further required that a steady state exist throughout the atmospheric or fluid model. The equilibrium may be stable or unstable with respect to displacements therefrom. See also hydrostatic equilibrium, geostrophic equilibrium, instability. 2. In thermodynamics, any state of a system that would not undergo change if the system were to be isolated." .

sstate:Deterministic  a  sstate:SystemState .

sstate:Chaos  a  sstate:SystemState .

sstate:Homogeneous  a      sstate:SystemState ;
        owl:differentFrom  sstate:Heterogeneous .

sstate:NonLinear  a  sstate:SystemState .

sstate:Instability  a  owl:Class .

sstate:Static  a           sstate:SystemState ;
        owl:differentFrom  sstate:Dynamic .

sstate:Active  a               ordi:ActivityLevel ;
        screla:moreActiveThan  sstate:Inactive .

sstate:Native  a  sstate:SystemState .

sstate:Dynamic  a   sstate:SystemState ;
        owl:sameAs  sstate:TimeDependent , sstate:TimeVarying .

sstate:Deficit  a         owl:Class ;
        rdfs:subClassOf   sstate:SystemState ;
        owl:disjointWith  sstate:Excess .

sstate:Hysteresis  a  sstate:SystemState .

sstate:Resilient  a      owl:Class ;
        rdfs:subClassOf  sstate:SystemState .

sstate:TimeDependent  a  sstate:SystemState .

sstate:Closed  a           sstate:SystemState ;
        owl:differentFrom  sstate:Open .

sstate:Complete  a  sstate:SystemState .

sstate:Extinct  a  ordi:ActivityLevel .

sstate:NonEquilibrium
        a                  sstate:SystemState ;
        owl:differentFrom  sstate:Equilibrium .

sstate:Coupled  a  sstate:SystemState .

sstate:Exogenous  a  sstate:SystemState .

sstate:Homeostasis  a    owl:Class ;
        rdfs:subClassOf  sstate:SystemState .

sstate:SystemState  a    owl:Class ;
        rdfs:subClassOf  state:State .

sstate:TimeVarying  a  sstate:SystemState .

sstate:Disturbed  a  sstate:SystemState .

sstate:Inhomogeneous  a  sstate:SystemState .

sstate:Dependent  a        sstate:SystemState ;
        owl:differentFrom  sstate:Independent .

sstate:Dormant  a              ordi:ActivityLevel ;
        screla:moreActiveThan  sstate:Inactive .

sstate:Artificial  a       sstate:SystemState ;
        owl:differentFrom  sstate:Natural .

sstate:Heterogeneous  a    sstate:SystemState ;
        owl:differentFrom  sstate:Inhomogeneous .

sstate:Open  a  sstate:SystemState .

sstate:Intermittent  a  sstate:SystemState .

sstate:Broken  a  sstate:SystemState .

sstate:Coherent  a       owl:Class ;
        rdfs:subClassOf  sstate:SystemState .

sstate:Stability  a  owl:Class .

sstate:Endogenous  a       sstate:SystemState ;
        owl:differentFrom  sstate:Exogenous .

sstate:EquilibriumState
        a                owl:Class ;
        rdfs:subClassOf  sstate:SystemState ;
        rdfs:subClassOf  [ a               owl:Restriction ;
                           owl:hasValue    sstate:Equilibrium ;
                           owl:onProperty  rela:hasState
                         ] .

sstate:Overflow  a       owl:Class ;
        rdfs:subClassOf  sstate:SystemState .

sstate:Unstable  a           owl:Class ;
        rdfs:comment         "property describing unstable conditions, such as in the atmosphere" ;
        rdfs:subClassOf      sstate:SystemState ;
        owl:disjointWith     sstate:Stability ;
        owl:equivalentClass  sstate:Instability .

sstate:Complex  a        owl:Class ;
        rdfs:comment     "A complex system is a system composed of interconnected parts that as a whole exhibit one or more properties (behavior among the possible properties) not obvious from the properties" ;
        rdfs:subClassOf  sstate:SystemState .
