<?xml version="1.0" encoding="UTF-8"?>

<!DOCTYPE rdf:RDF [
   <!ENTITY func "http://sweet.jpl.nasa.gov/2.0/mathFunction.owl">  
   <!ENTITY phys "http://sweet.jpl.nasa.gov/2.0/phys.owl">  
   <!ENTITY ener "http://sweet.jpl.nasa.gov/2.0/physEnergy.owl">  
   <!ENTITY orog "http://sweet.jpl.nasa.gov/2.0/landOrographic.owl">  
   <!ENTITY space "http://sweet.jpl.nasa.gov/2.0/space.owl">  
   <!ENTITY xten "http://sweet.jpl.nasa.gov/2.0/spaceExtent.owl">  
   <!ENTITY sol "http://sweet.jpl.nasa.gov/2.0/mathSolution.owl">  
   <!ENTITY state "http://sweet.jpl.nasa.gov/2.0/sciSystemState.owl">  
   <!ENTITY planet "http://sweet.jpl.nasa.gov/2.0/astroPlanet.owl">  
   <!ENTITY front "http://sweet.jpl.nasa.gov/2.0/atmoFront.owl">  
   <!ENTITY static "http://sweet.jpl.nasa.gov/2.0/physFluid.owl">  
   <!ENTITY atmo "http://sweet.jpl.nasa.gov/2.0/atmo.owl">  
   <!ENTITY thermo "http://sweet.jpl.nasa.gov/2.0/physThermo.owl">
   <!ENTITY astab "http://sweet.jpl.nasa.gov/2.0/atmoStability.owl">
   <!ENTITY statec "http://sweet.jpl.nasa.gov/2.0/chemStateChange.owl">
   <!ENTITY owl "http://www.w3.org/2002/07/owl#">
   <!ENTITY rdf "http://www.w3.org/1999/02/22-rdf-syntax-ns#">
   <!ENTITY rdfs "http://www.w3.org/2000/01/rdf-schema#">
   <!ENTITY xsd "http://www.w3.org/2001/XMLSchema#">

]>

<rdf:RDF xml:base="&astab;"
         xmlns:owl="&owl;"
         xmlns:rdf="&rdf;"
         xmlns:rdfs="&rdfs;"
	 xmlns:xsd = "&xsd;"
         xmlns:front="&front;"  
         xmlns:static="&static;"  
         xmlns:thermo="&thermo;"
         xmlns:orog="&orog;"
         xmlns:astab="&astab;"
	 xmlns:sol="&sol;"
	 xmlns:state="&state;"
	 xmlns:planet="&planet;"
	 xmlns:func="&func;"
	 xmlns:atmo="&atmo;"
	 xmlns:phys="&phys;"
	 xmlns:ener="&ener;"
    	 xmlns:xten="&xten;"
    	 xmlns:statec="&statec;">

<!-- Ontology Information -->
  <owl:Ontology rdf:about=""
                owl:versionInfo="2.0">
     <owl:imports rdf:resource="&func;"/>
     <owl:imports rdf:resource="&xten;"/>
     <owl:imports rdf:resource="&sol;"/>
     <owl:imports rdf:resource="&state;"/>
     <owl:imports rdf:resource="&planet;"/>
     <owl:imports rdf:resource="&phys;"/>
     <owl:imports rdf:resource="&ener;"/>
     <owl:imports rdf:resource="&atmo;"/>
     <owl:imports rdf:resource="&orog;"/>
     <owl:imports rdf:resource="&thermo;"/>     
     <owl:imports rdf:resource="&front;"/>     
     <owl:imports rdf:resource="&static;"/>     
     <owl:imports rdf:resource="&statec;"/>     
  </owl:Ontology>

<!-- Properties -->
  <owl:Class rdf:about="#AutoConvectiveLapseRate">
    <rdfs:subClassOf rdf:resource="#EnvironmentalLapseRate" />
    <rdfs:comment xml:lang="en">The environmental lapse rate of temperature in an atmosphere in which the density is constant with height (homogeneous atmosphere), equal to g/R, where g is the acceleration of gravity and R the gas constant.
    </rdfs:comment>
  </owl:Class>

  <owl:Class rdf:about="#EquivalentPotentialTemperature">
    <rdfs:subClassOf rdf:resource="#PotentialTemperature"/>
  </owl:Class>

  <owl:Class rdf:about="#PotentialTemperature">
    <rdfs:subClassOf rdf:resource="&thermo;#Temperature"/>
    <rdfs:subClassOf>
      <owl:Restriction>
        <owl:onProperty rdf:resource="&phys;#hasPhysicalProcess" />
        <owl:allValuesFrom rdf:resource="&thermo;#Adiabatic" />
      </owl:Restriction>
    </rdfs:subClassOf>
    <rdfs:comment xml:lang="en">The temperature that a parcel would have if brought adiabatically and reversibly from its initial state to a standard reference pressure, typically 100 kPa.</rdfs:comment>
  </owl:Class>

  <owl:Class rdf:about="#PseudoEquivalentPotentialTemperature">
    <rdfs:subClassOf rdf:resource="&thermo;#Temperature"/>
    <rdfs:subClassOf>
      <owl:Restriction>
        <owl:onProperty rdf:resource="&sol;#approximates" />
        <owl:allValuesFrom rdf:resource="#EquivalentPotentialTemperature" />
      </owl:Restriction>
    </rdfs:subClassOf>
  </owl:Class>

  <owl:Class rdf:about="#VirtualPotentialTemperature">
    <rdfs:subClassOf rdf:resource="#PotentialTemperature"/>
  </owl:Class>

  <owl:Class rdf:about="#WetBulbPotentialTemperature">
    <rdfs:subClassOf rdf:resource="#PotentialTemperature"/>
    <rdfs:comment xml:lang="en">The temperature an air parcel would have if cooled from its initial state adiabatically to saturation, and thence brought to 1000 mb by a moist-adiabatic process.</rdfs:comment>
  </owl:Class>

  <owl:Class rdf:about="#DryAdiabaticLapseRate">
    <rdfs:subClassOf rdf:resource="#LapseRate"/>
    <rdfs:subClassOf>
      <owl:Restriction>
        <owl:onProperty rdf:resource="&phys;#hasPhysicalProcess" />
        <owl:allValuesFrom rdf:resource="#DryAdiabaticProcess" />
      </owl:Restriction>
    </rdfs:subClassOf>
    <rdfs:comment xml:lang="en">A process lapse rate of temperature, the rate of decrease of temperature with height of a parcel of dry air lifted by a reversible adiabatic process through an atmosphere in hydrostatic equilibrium.</rdfs:comment>
  </owl:Class>

  <owl:Class rdf:about="#EnvironmentalLapseRate">
    <rdfs:subClassOf rdf:resource="#LapseRate"/>
    <rdfs:comment xml:lang="en">The rate of decrease of temperature with elevation</rdfs:comment>
  </owl:Class>

  <owl:Class rdf:about="#EvaporativeAvailablePotentialEnergy">
    <rdfs:subClassOf rdf:resource="&static;#AvailablePotentialEnergy" />
    <rdfs:subClassOf>
      <owl:Restriction>
        <owl:onProperty rdf:resource="&statec;#hasStateChange" />
        <owl:allValuesFrom rdf:resource="&statec;#Evaporation" />
      </owl:Restriction>
    </rdfs:subClassOf>
    <rdfs:comment xml:lang="en">Analogous to convective available potential energy, except that it is related to the negative buoyancy associated with evaporative cooling of liquid water within a sinking cloudy air parcel.</rdfs:comment>
  </owl:Class>

  <owl:Class rdf:about="#LapseRate">
    <rdfs:subClassOf rdf:resource="&thermo;#TemperatureHeightDerivative"/>
  </owl:Class>

  <owl:Class rdf:about="#BoydenIndex">
    <rdfs:subClassOf rdf:resource="&state;#Stability"/>
    <rdfs:comment>A measure of the mean thermodynamic stability in a layer beneath 700 mb.</rdfs:comment>
  </owl:Class>

  <owl:Class rdf:about="#LFC">
    <rdfs:subClassOf rdf:resource="&xten;#Level" />
    <rdfs:comment>Level of free convection</rdfs:comment>
    <owl:equivalentClass rdf:resource="#LevelOfFreeConvection"/>
  </owl:Class>
  <owl:Class rdf:about="#LevelOfFreeConvection"/>

<!-- Phenomena -->
  <owl:Class rdf:about="#Cap">
    <rdfs:subClassOf rdf:resource="&xten;#Level" />
    <rdfs:comment> A region of negative buoyancy below an existing level of free convection (LFC) where energy must be supplied to the parcel to maintain its ascent.</rdfs:comment>
  </owl:Class>

  <owl:Class rdf:about="#ConvectiveInhibition">
    <rdfs:subClassOf rdf:resource="&ener;#Energy" />
    <rdfs:comment xml:lang="en">The energy needed to lift an air parcel vertically and pseudoadiabatically from its originating level to its level of free convection (LFC).</rdfs:comment>
  </owl:Class>

  <owl:Class rdf:about="#DryAdiabat">
    <rdfs:subClassOf rdf:resource="&func;#Isopleth" />
    <rdfs:subClassOf>
      <owl:Restriction>
        <owl:onProperty rdf:resource="&phys;#hasPhysicalProperty" />
        <owl:allValuesFrom rdf:resource="#PotentialTemperature" />
      </owl:Restriction>
    </rdfs:subClassOf>
    <rdfs:comment xml:lang="en">A line of constant potential temperature on a thermodynamic diagram.</rdfs:comment>
  </owl:Class>

  <owl:Class rdf:about="#AdiabaticAtmosphere">
    <rdfs:subClassOf rdf:resource="&planet;#Atmosphere" />
    <rdfs:subClassOf>
      <owl:Restriction>
        <owl:onProperty rdf:resource="&phys;#hasPhysicalProperty" />
        <owl:allValuesFrom rdf:resource="#DryAdiabaticLapseRate" />
      </owl:Restriction>
    </rdfs:subClassOf>
    <rdfs:label>Adiabatic Atmosphere</rdfs:label>
    <rdfs:comment>A model atmosphere characterized by a dry-adiabatic lapse rate throughout its vertical extent.
    </rdfs:comment>
  </owl:Class>

  <owl:Class rdf:about="#Lift">
    <rdfs:subClassOf rdf:resource="&atmo;#MeteorologicalPhenomena" />
    <owl:equivalentClass rdf:resource="#Lifting"/>
  </owl:Class>
  <owl:Class rdf:about="#Lifting"/>

  <owl:Class rdf:about="#OrographicLifting">
    <rdfs:subClassOf rdf:resource="#Lifting" />
    <rdfs:subClassOf>
      <owl:Restriction>
        <owl:onProperty rdf:resource="&phys;#hasPhysicalProcess" />
        <owl:someValuesFrom rdf:resource="&orog;#Orographic" />
      </owl:Restriction>
    </rdfs:subClassOf>
    <rdfs:comment xml:lang="en">Ascending air flow caused by mountains.  Mechanisms that produce the lifting fall into two broad categories: 1) the upward deflection of horizontal larger-scale flow by the orography acting as an obstacle or barrier; or 2) the daytime heating of mountain surfaces to produce anabatic flow along the slopes and updrafts in the vicinity of the peaks.</rdfs:comment>
  </owl:Class>

  <owl:Class rdf:about="#ConditionalInstability">
    <rdfs:subClassOf rdf:resource="&state;#Instability" />
    <rdfs:comment xml:lang="en">The state of a layer of unsaturated air when its lapse rate of temperature is less than the dry-adiabatic lapse rate but greater than the moist-adiabatic lapse rate.</rdfs:comment>
  </owl:Class>

  <owl:Class rdf:about="#FreeInstability">
    <rdfs:subClassOf rdf:resource="&state;#Instability" />
    <rdfs:comment xml:lang="en">The state of a layer of unsaturated air when its lapse rate of temperature is less than the dry-adiabatic lapse rate but greater than the moist-adiabatic lapse rate.</rdfs:comment>
  </owl:Class>

  <owl:Class rdf:about="#FrontalInversion">
    <rdfs:subClassOf>
      <owl:Restriction>
        <owl:onProperty rdf:resource="&atmo;#hasMeteorologicalPhenomena" />
        <owl:allValuesFrom rdf:resource="&front;#Front" />
      </owl:Restriction>
    </rdfs:subClassOf>
    <rdfs:subClassOf rdf:resource="#Inversion" />
    <rdfs:comment xml:lang="en">A temperature inversion (temperature rising with height) in the atmosphere, encountered upon vertical ascent through a sloping front (or frontal zone).</rdfs:comment>
  </owl:Class>

  <owl:Class rdf:about="#Inversion">
    <rdfs:subClassOf rdf:resource="&atmo;#MeteorologicalPhenomena" />
    <rdfs:subClassOf>
      <owl:Restriction>
        <owl:onProperty rdf:resource="&phys;#hasPhysicalProperty" />
        <owl:allValuesFrom rdf:resource="&thermo;#Temperature" />
      </owl:Restriction>
    </rdfs:subClassOf>
    <rdfs:comment xml:lang="en">In meteorology, a departure from the usual decrease or increase with altitude of the value of an atmospheric quantity; also, the layer through which this departure occurs (the inversion layer), or the lowest altitude at which the departure is found (the base of the inversion).</rdfs:comment>
  </owl:Class>

  <owl:Class rdf:about="#AbsoluteInstability">
    <rdfs:subClassOf rdf:resource="&state;#Instability" />
    <rdfs:comment>state of a layer of atmosphere when it has superadiabatic lapse rate of temperature</rdfs:comment>
    <rdfs:label>Absolute Instability</rdfs:label>
  </owl:Class>

<!-- Realms -->
  <owl:Class rdf:about="#InversionLayer">
    <rdfs:subClassOf rdf:resource="&atmo;#AtmosphereLayer" />
    <owl:equivalentClass rdf:resource="#TemperatureInversionLayer"/>
    <rdfs:subClassOf>
      <owl:Restriction>
        <owl:onProperty rdf:resource="&atmo;#hasMeteorologicalPhenomena" />
        <owl:allValuesFrom rdf:resource="#Inversion" />
      </owl:Restriction>
    </rdfs:subClassOf>
  </owl:Class>
  <owl:Class rdf:about="#TemperatureInversionLayer"/>

  <owl:Class rdf:about="#FreeConvectiveLayer">
    <rdfs:subClassOf rdf:resource="&atmo;#AtmosphereLayer" />
    <rdfs:subClassOf>
      <owl:Restriction>
        <owl:onProperty rdf:resource="&atmo;#hasMeteorologicalPhenomena" />
        <owl:allValuesFrom rdf:resource="#FreeInstability" />
      </owl:Restriction>
    </rdfs:subClassOf>
  </owl:Class>

<!-- Processes -->
  <owl:Class rdf:about="#DryAdiabaticProcess">
    <rdfs:subClassOf rdf:resource="&thermo;#Adiabatic" />
    <rdfs:label>Dry Adiabatic Process</rdfs:label>
    <rdfs:comment>1. An adiabatic process in a hypothetical atmosphere in which no moisture is present. 2. An adiabatic process in which no condensation of its water vapor occurs and no liquid water is present.</rdfs:comment>
  </owl:Class>

  <owl:Class rdf:about="#PseudoAdiabaticProcess">
    <rdfs:subClassOf rdf:resource="&phys;#PhysicalProcess" />
    <rdfs:subClassOf>
      <owl:Restriction>
        <owl:onProperty rdf:resource="&sol;#approximates" />
        <owl:allValuesFrom rdf:resource="&thermo;#Adiabatic" />
      </owl:Restriction>
    </rdfs:subClassOf>
    <rdfs:comment xml:lang="en">A moist-adiabatic process in which the liquid water that condenses is assumed to be removed as soon as it is formed, by idealized instantaneous precipitation.</rdfs:comment>
  </owl:Class>

</rdf:RDF>
