<?xml version="1.0" encoding="UTF-8"?>

<!DOCTYPE rdf:RDF [
  <!ENTITY trans "http://sweet.jpl.nasa.gov/2.0/physTransport.owl">
  <!ENTITY fludyn "http://sweet.jpl.nasa.gov/2.0/physFluidDynamics.owl">
  <!ENTITY inst "http://sweet.jpl.nasa.gov/2.0/physFluidInstability.owl">
  <!ENTITY state "http://sweet.jpl.nasa.gov/2.0/chemState.owl">
  <!ENTITY phys "http://sweet.jpl.nasa.gov/2.0/phys.owl">
  <!ENTITY ener "http://sweet.jpl.nasa.gov/2.0/physEnergy.owl">
  <!ENTITY dynam "http://sweet.jpl.nasa.gov/2.0/physDynamics.owl">
  <!ENTITY vect "http://sweet.jpl.nasa.gov/2.0/mathVector.owl">
  <!ENTITY units "http://sweet.jpl.nasa.gov/2.0/sciUnits.owl">
  <!ENTITY res "http://sweet.jpl.nasa.gov/2.0/sciResearch.owl">
  <!ENTITY owl "http://www.w3.org/2002/07/owl#">
  <!ENTITY rdf "http://www.w3.org/1999/02/22-rdf-syntax-ns#">
  <!ENTITY rdfs "http://www.w3.org/2000/01/rdf-schema#">
  <!ENTITY xsd "http://www.w3.org/2001/XMLSchema#">
]>

<rdf:RDF xml:base="&trans;"
         xmlns:res="&res;"
         xmlns:phys="&phys;"
         xmlns:ener="&ener;"
         xmlns:dynam="&dynam;"
         xmlns:vect="&vect;"
         xmlns:state="&state;"
         xmlns:trans="&trans;"
         xmlns:units="&units;"
         xmlns:fludyn="&fludyn;"
         xmlns:inst="&inst;"
         xmlns:owl="&owl;"
         xmlns:rdf="&rdf;"
         xmlns:rdfs="&rdfs;"
 	 xmlns:xsd="&xsd;">

<!-- Ontology Information -->
  <owl:Ontology rdf:about="" owl:versionInfo="2.0">
     <owl:imports rdf:resource="&fludyn;"/>
     <owl:imports rdf:resource="&inst;"/>
     <owl:imports rdf:resource="&phys;"/>
     <owl:imports rdf:resource="&ener;"/>
     <owl:imports rdf:resource="&dynam;"/>
     <owl:imports rdf:resource="&units;"/>
     <owl:imports rdf:resource="&vect;"/>
     <owl:imports rdf:resource="&res;"/>
     <owl:imports rdf:resource="&state;"/>
  </owl:Ontology>

<!-- Phenomena -->
  <owl:Class rdf:about="#Advection">
    <rdfs:subClassOf rdf:resource="&phys;#PhysicalPhenomena"/>
    <rdfs:subClassOf>
      <owl:Restriction>
        <owl:onProperty rdf:resource="&state;#hasState" />
        <owl:allValuesFrom rdf:resource="&state;#Fluid" />
      </owl:Restriction>
    </rdfs:subClassOf>
    <rdfs:subClassOf>
      <owl:Restriction>
        <owl:onProperty rdf:resource="&phys;#hasPhysicalProperty" />
        <owl:allValuesFrom rdf:resource="#Transport" />
      </owl:Restriction>
    </rdfs:subClassOf>
    <rdfs:label>Advection</rdfs:label>
    <rdfs:comment>The process of transport solely by the mass motion (velocity field); also, the rate of change of the value of the advected property at a given point.</rdfs:comment>
  </owl:Class>

  <owl:Class rdf:about="#BolusAdvection">
    <rdfs:subClassOf rdf:resource="#Advection"/>
  </owl:Class>

  <owl:Class rdf:about="#Buoyancy">
    <rdfs:subClassOf rdf:resource="&phys;#PhysicalPhenomena"/>
    <rdfs:comment xml:lang="en">That property of an object that enables it to float on the surface of a liquid, or ascend through and remain freely suspended in a compressible fluid such as the atmosphere.</rdfs:comment>
  </owl:Class> 

  <owl:Class rdf:about="#Convection">
    <rdfs:subClassOf rdf:resource="&ener;#EnergyTransfer"/>
    <rdfs:comment xml:lang="en">In general, mass motions within a fluid resulting in transport and mixing of the properties of that fluid.  Convection, along with conduction and radiation, is a principal means of energy transfer.</rdfs:comment>
  </owl:Class>

  <owl:Class rdf:about="#Convective">
    <rdfs:subClassOf rdf:resource="&phys;#PhysicalPhenomena" />
    <rdfs:subClassOf>
      <owl:Restriction>
        <owl:onProperty rdf:resource="&phys;#hasPhysicalProcess" />
        <owl:allValuesFrom rdf:resource="#Convection" />
      </owl:Restriction>
    </rdfs:subClassOf>
  </owl:Class>

  <owl:Class rdf:about="#Deposition">
    <rdfs:subClassOf rdf:resource="&phys;#PhysicalProcess"/>
    <rdfs:comment xml:lang="en">Processes by which traces gases or particles are transferred from atmosphere to a surface.</rdfs:comment>
  </owl:Class>

  <owl:Class rdf:about="#SlantWiseConvection">
    <rdfs:subClassOf rdf:resource="#Convection" />
    <rdfs:comment xml:lang="en">A form of convection driven by a combination of gravitational and centrifugal forces.</rdfs:comment>
  </owl:Class>

  <owl:Class rdf:about="#VorticityAdvection">
    <rdfs:subClassOf rdf:resource="#Advection" />
    <rdfs:subClassOf>
      <owl:Restriction>
        <owl:onProperty rdf:resource="&phys;#hasPhysicalProperty" />
        <owl:allValuesFrom rdf:resource="&vect;#Vorticity" />
      </owl:Restriction>
    </rdfs:subClassOf>
    <rdfs:comment xml:lang="en">Advection of vorticity by the total wind or force.</rdfs:comment>
  </owl:Class>

<!-- Properties -->
  <owl:Class rdf:about="#BuoyancyFlux">
    <rdfs:subClassOf rdf:resource="#Flux" />
    <rdfs:subClassOf>
      <owl:Restriction>
        <owl:onProperty rdf:resource="&phys;#hasPhysicalProperty" />
        <owl:someValuesFrom rdf:resource="#Buoyancy" />
      </owl:Restriction>
    </rdfs:subClassOf>
    <rdfs:comment xml:lang="en">The vertical kinematic flux of virtual potential temperature, which when multiplied by the buoyancy parameter yields a flux that is proportional to buoyancy.</rdfs:comment>
  </owl:Class>

  <owl:Class rdf:about="#BuoyancyVelocity">
    <rdfs:subClassOf rdf:resource="&dynam;#Velocity" />
    <rdfs:subClassOf>
      <owl:Restriction>
        <owl:onProperty rdf:resource="&phys;#hasPhysicalProcess" />
        <owl:allValuesFrom rdf:resource="#Convection" />
      </owl:Restriction>
    </rdfs:subClassOf>
    <rdfs:subClassOf>
      <owl:Restriction>
        <owl:onProperty rdf:resource="&phys;#hasPhysicalProperty" />
        <owl:allValuesFrom rdf:resource="#Buoyancy" />
      </owl:Restriction>
    </rdfs:subClassOf>
    <rdfs:comment xml:lang="en">A vertical velocity scale for convective boundary layers, that is related to the buoyant driving force for convection and the depth of the mixed layer.</rdfs:comment>
  </owl:Class>

  <owl:Class rdf:about="#ConvectiveMassFlux">
    <rdfs:subClassOf rdf:resource="#MassFlux" />
    <rdfs:subClassOf>
      <owl:Restriction>
        <owl:onProperty rdf:resource="&phys;#hasPhysicalPhenomena" />
        <owl:someValuesFrom rdf:resource="#Convection" />
      </owl:Restriction>
    </rdfs:subClassOf>
    <rdfs:comment xml:lang="en">An average vertical transport of mass for a field, e.g., of cumulus clouds or thermals.
    </rdfs:comment>
  </owl:Class>

  <owl:Class rdf:about="#CounterGradientFlux">
    <rdfs:subClassOf rdf:resource="#Flux" />
  </owl:Class>

  <owl:Class rdf:about="#Diffusivity">
    <rdfs:subClassOf rdf:resource="&phys;#PhysicalProperty"/>
    <rdfs:subClassOf>
      <owl:Restriction>
        <owl:onProperty rdf:resource="&phys;#hasPhysicalProcess" />
        <owl:allValuesFrom rdf:resource="#Diffusion" />
      </owl:Restriction>
    </rdfs:subClassOf>
    <rdfs:comment>(Also called coefficient of diffusion.) The ratio of the flux of a conservative property through a specified surface by turbulence to the gradient of the mean property normal to the surface.</rdfs:comment>
    <rdfs:label>Diffusivity</rdfs:label>
  </owl:Class>

  <owl:Class rdf:about="#DifferentialFlux">
    <rdfs:subClassOf rdf:resource="#Flux"/>
  </owl:Class>

  <owl:Class rdf:about="#EddyDiffusivity">
    <rdfs:subClassOf rdf:resource="#Diffusivity" />
    <rdfs:subClassOf>
      <owl:Restriction>
        <owl:onProperty rdf:resource="&phys;#hasPhysicalProperty" />
        <owl:someValuesFrom rdf:resource="&fludyn;#Eddy" />
      </owl:Restriction>
    </rdfs:subClassOf>
    <rdfs:comment xml:lang="en">The exchange coefficient for the diffusion of a conservative property by eddies in a turbulent flow.</rdfs:comment>
  </owl:Class>

  <owl:Class rdf:about="#EddyFlux">
    <rdfs:subClassOf rdf:resource="#Flux" />
    <rdfs:subClassOf>
      <owl:Restriction>
        <owl:onProperty rdf:resource="&phys;#hasPhysicalPhenomena" />
        <owl:someValuesFrom rdf:resource="&fludyn;#Eddy" />
      </owl:Restriction>
    </rdfs:subClassOf>
    <rdfs:comment xml:lang="en">The rate of transfer of a conservative fluid property through a surface by turbulent eddies.
    </rdfs:comment>
  </owl:Class>

  <owl:Class rdf:about="#Flux">
    <rdfs:subClassOf rdf:resource="&phys;#PhysicalProperty"/>
    <rdfs:subClassOf rdf:resource="&vect;#Vector"/>
    <rdfs:subClassOf>
      <owl:Restriction>
        <owl:onProperty rdf:resource="&phys;#hasPhysicalProcess" />
        <owl:allValuesFrom rdf:resource="#Transport" />
      </owl:Restriction>
    </rdfs:subClassOf>
    <rdfs:comment xml:lang="en">The rate of flow of some quantity, often used in reference to the flow of some form of energy.
    </rdfs:comment>
  </owl:Class>

  <owl:Class rdf:about="#FluxDensity">
    <rdfs:subClassOf rdf:resource="#Flux" />
    <owl:equivalentClass rdf:resource="#Intensity"/>
    <rdfs:subClassOf>
      <owl:Restriction>
        <owl:hasValue rdf:resource="&units;#watt_perMeterSquared"/>
        <owl:onProperty rdf:resource="&units;#hasDefaultUnit"/>
      </owl:Restriction>
    </rdfs:subClassOf>
  </owl:Class>
  <owl:Class rdf:about="#Intensity"/>

  <owl:Class rdf:about="#MassFlux">
    <rdfs:subClassOf rdf:resource="#Flux"/>
    <rdfs:subClassOf>
      <owl:Restriction>
        <owl:onProperty rdf:resource="&phys;#hasPhysicalProperty" />
        <owl:allValuesFrom rdf:resource="&phys;#Mass" />
      </owl:Restriction>
    </rdfs:subClassOf>
  </owl:Class>

  <owl:Class rdf:about="#Transport">
    <rdfs:subClassOf rdf:resource="&phys;#PhysicalProperty" />
  </owl:Class>

  <owl:Class rdf:about="#TurbulentFlux">
    <rdfs:subClassOf rdf:resource="#Flux" />
    <rdfs:subClassOf>
      <owl:Restriction>
        <owl:onProperty rdf:resource="&phys;#hasPhysicalPhenomena" />
        <owl:someValuesFrom rdf:resource="&inst;#Turbulence" />
      </owl:Restriction>
    </rdfs:subClassOf>
    <rdfs:comment xml:lang="en">Transport of a quantity by quasi-random eddies or swirls; the covariance between a velocity component and any variable.</rdfs:comment>
  </owl:Class>

  <owl:ObjectProperty rdf:about="#hasFlux">
    <rdfs:range rdf:resource="#Flux"/>
  </owl:ObjectProperty>

<!-- Processes -->
  <owl:Class rdf:about="#Diffusion">
    <rdfs:subClassOf rdf:resource="&phys;#PhysicalProcess"/>
    <owl:equivalentClass rdf:resource="#Diffuse"/>
  </owl:Class>
  <owl:Class rdf:about="#Diffuse"/>

  <owl:Class rdf:about="#EddyDiffusion">
    <rdfs:subClassOf rdf:resource="#Diffusion" />
    <rdfs:subClassOf>
      <owl:Restriction>
        <owl:onProperty rdf:resource="&phys;#hasPhysicalProperty" />
        <owl:someValuesFrom rdf:resource="&fludyn;#Eddy" />
      </owl:Restriction>
    </rdfs:subClassOf>
  </owl:Class>

  <owl:Class rdf:about="#FickianDiffusion">
    <rdfs:subClassOf rdf:resource="#Diffusion" />
  </owl:Class>

  <owl:Class rdf:about="#TurbulentDiffusion">
    <rdfs:subClassOf rdf:resource="#Diffusion" />
    <rdfs:subClassOf>
      <owl:Restriction>
        <owl:onProperty rdf:resource="&phys;#hasPhysicalPhenomena" />
        <owl:someValuesFrom rdf:resource="&inst;#Turbulence" />
      </owl:Restriction>
    </rdfs:subClassOf>
    <rdfs:comment xml:lang="en">Diffusion or dispersion due to the effects of turbulent motions.</rdfs:comment>
  </owl:Class>

<!-- Knowledge -->
  <owl:Class rdf:about="#Parcel">
    <rdfs:subClassOf rdf:resource="&res;#Sample"/>
    <rdfs:comment xml:lang="en">An imaginary volume of fluid to which may be assigned various thermodynamic and kinematic quantities.</rdfs:comment>
  </owl:Class>

</rdf:RDF>
